Compound Angles Solutions
*************************
1. Given, :math:`\sin\alpha = \frac{3}{5}` and :math:`\cos\beta = \frac{9}{41}`

   Therefore, :math:`\cos\alpha = \frac{4}{5}` and :math:`\sin\beta = \frac{40}{41}`

   :math:`\sin(\alpha - \beta) = \sin\alpha\cos\beta - \cos\alpha\sin\beta`

   :math:`= \frac{3}{5}\frac{9}{41} - \frac{4}{5}\frac{40}{41}`

   :math:`= \frac{27 - 160}{205} = -\frac{133}{205}`

   :math:`\cos(\alpha + \beta) = \cos\alpha\cos\beta - \sin\alpha\sin\beta`

   :math:`= \frac{4}{5}\frac{9}{41} - \frac{3}{5}\frac{40}{41}`

   :math:`= \frac{36 - 120}{205} = -\frac{84}{205}`

2. Given, :math:`\sin\alpha = \frac{45}{53}` and :math:`\sin\beta = \frac{33}{65}`

   Thus, :math:`\cos\alpha = \frac{28}{53}` and :math:`\cos\beta = \frac{56}{65}`

   :math:`\sin(\alpha - \beta) = \sin\alpha\cos\beta - \cos\alpha\sin\beta`

   :math:`= \frac{45}{53}\frac{56}{65} - \frac{28}{53}\frac{33}{65}`

   :math:`= \frac{2520 - 924}{3445} = \frac{1596}{3445}`

   :math:`\sin(\alpha + \beta) = \sin\alpha\cos\beta + \cos\alpha\sin\beta`

   :math:`= \frac{45}{53}\frac{56}{65} + \frac{28}{53}\frac{33}{65}`

   :math:`= \frac{2520 + 924}{3445} = \frac{3444}{3445}`

3. Given, :math:`\sin\alpha = \frac{15}{17}` and :math:`\cos\beta = \frac{12}{13}`

   :math:`\cos\alpha = \frac{8}{17}` and :math:`\sin\beta = \frac{5}{13}`

   :math:`\tan\alpha = \frac{15}{8}` and :math:`\tan\beta = \frac{5}{12}`

   :math:`\sin(\alpha + \beta) = \sin\alpha\cos\beta + \cos\alpha\sin\beta`

   :math:`= \frac{15}{17}\frac{12}{13} + \frac{8}{17}\frac{5}{13}`

   :math:`= \frac{220}{221}`

   :math:`\cos(\alpha - \beta) = \cos\alpha\cos\beta + \sin\alpha\sin\beta`

   :math:`= \frac{8}{17}\frac{12}{13} + \frac{15}{17}\frac{5}{13}`

   :math:`= \frac{171}{221}`

   :math:`\tan(\alpha + \beta) = \frac{\tan\alpha + \tan\beta}{1 - \tan\alpha\tan\beta}`

   :math:`= \frac{\frac{15}{8} + \frac{5}{12}}{1 - \frac{15}{8}\frac{5}{12}}`

   :math:`= \frac{220}{21}`

4. L.H.S. :math:`= \cos(45^{\circ} - A)\cos(45^{\circ} - B) - \sin(45^{\circ} - A)\sin(45^{\circ} - B)`

   :math:`= [(\cos 45^\circ\cos A + \sin45^\circ\sin A)(\cos 45^\circ\cos B + \sin45^\circ\sin B) - (\sin45^\circ\cos A -
   \cos45^\circ\sin A)(\sin45^\circ\cos B - \cos45^\circ\sin B)]`

   Substituting valus for :math:`\sin45^\circ` and :math:`\cos45^\circ`

   :math:`=\left[\left(\frac{\cos A}{\sqrt{2}} + \frac{\sin A}{\sqrt{2}}\right)\left(\frac{\cos B}{\sqrt{2}} + \frac{\sin
   B}{\sqrt{2}}\right)\right] - \left[\left(\frac{\cos A}{\sqrt{2}} - \frac{\sin A}{\sqrt{2}}\right)\left(\frac{\cos B}{\sqrt{2}} -
   \frac{\sin B}{\sqrt{2}}\right)\right]`

   :math:`= \left[\frac{\cos A\cos B}{2} + \frac{\cos A\sin B}{2} + \frac{\sin A\cos B}{2} + \frac{\sin A\sin B}{2}\right] -
   \left[\frac{\cos A\cos B}{2} - \frac{\cos A\sin B}{2} - \frac{\sin A\cos B}{2} + \frac{\sin A\sin B}{2}\right]`

   :math:`= \sin A\cos B + \cos A\sin B = \sin(A + B)`

5. L.H.S. :math:`= \sin(45^{\circ} + A)\cos(45^\circ - B) + \cos(45^{\circ} + A)\sin(45^\circ - B)`

   :math:`= [(\sin45^\circ\cos A + \cos45^\circ\sin A)(\cos45^\circ\cos B + \sin45^\circ\sin B) + (\cos45^\circ\cos A -
   \sin45^\circ\sin A)(\sin45^\circ\cos B - \cos45^\circ)\sin B]`

   :math:`= \left[\left(\frac{\cos A}{\sqrt{2}} + \frac{\sin A}{\sqrt{2}}\right)\left(\frac{\cos B}{\sqrt{2}} + \frac{\sin
   B}{\sqrt{2}}\right) + \left(\frac{\cos A}{\sqrt{2}} - \frac{\sin A}{\sqrt{2}}\right)\left(\frac{\cos B}{\sqrt{2}} - \frac{\sin
   B}{\sqrt{2}}\right)\right]`

   :math:`= \left[\frac{\cos A\cos B}{2} + \frac{\cos A\sin B}{2} + \frac{\sin A\cos B}{2} + \frac{\sin A\sin B}{2} +
   \frac{\cos A\cos B}{2} - \frac{\cos A\sin B}{2} - \frac{\sin A\cos B}{2} + \frac{\sin A\sin B}{2}\right]`

   :math:`= \cos A\cos B + \sin A\sin B = \cos(A - B)`

6. L.H.S. :math:`= \frac{\sin(A - B)}{\cos A\cos B} + \frac{\sin(B - C)}{\cos B\cos C} + \frac{\sin(C - A)}{\cos C\cos A}`

   :math:`= \frac{\sin A\cos B - \cos A\sin B}{\cos A\cos B} + \frac{\sin B\cos C - \cos B\sin C}{\cos B\cos C} + \frac{\sin C\cos
   A - \cos C\sin A}{\cos C\cos A}`

   :math:`= \tan A - \tan B + \tan B - \tan C + \tan C - \tan A = 0 =` R.H.S.

7. L.H.S. :math:`= \sin 105^\circ + \cos 105^\circ`

   :math:`= \sin(60^\circ + 45^\circ) + \cos(60^\circ + 45^\circ)`

   :math:`=\sin60^\circ\cos45^\circ + \cos60^\circ\sin45^\circ + \cos60^\circ\cos45^\circ - \sin60^\circ\sin45^\circ`

   :math:`=\cos45^\circ(\sin60^\circ + \cos60^\circ + \cos60^\circ - \sin 60^\circ)[\because \sin45^\circ = \cos45^\circ]`

   :math:`= \cos45^\circ =` R.H.S.

8. Given, :math:`\sin 75^\circ - \sin 15^\circ = \cos 105^\circ + \cos 15^\circ`

   :math:`\Rightarrow \sin75^\circ -\sin15^\circ = \cos(90^\circ + 15^\circ) + \sin(90^\circ - 15^\circ)`

   :math:`\Rightarrow \sin75^\circ -\sin15^\circ = \cos90^\circ\cos15^\circ - \sin90^\circ\sin15^\circ + \sin(90^\circ - 15^\circ)`

   :math:`\Rightarrow \sin75^\circ -\sin15^\circ = -\sin15^\circ + \sin75^\circ [\because \cos90^\circ = 0~\&~\sin90^\circ = 1]`

   Thus, we have proven the equality.

9. L.H.S. :math:`= \cos\alpha\cos(\gamma - \alpha) - \sin\alpha\sin(\gamma - \alpha)`

   :math:`= \cos\alpha(\cos\gamma\cos\alpha + \sin\gamma\sin\alpha) - \sin\alpha(\sin\gamma\cos\alpha - \sin\alpha\cos\gamma)`

   :math:`= \cos^2\alpha\cos\gamma + \sin\gamma\sin\alpha\cos\alpha - \sin\alpha\sin\gamma\cos\alpha - \sin^2\alpha\cos\gamma`

   :math:`= \cos\gamma(\sin^2\alpha + \cos^2\alpha) = \cos\gamma =` R.H.S.

10. L.H.S. :math:`= \cos(\alpha + \beta)\cos\gamma - \cos(\beta + \gamma)\cos\alpha`

    :math:`= \cos\alpha\cos\beta\cos\gamma - \sin\alpha\sin\beta\cos\gamma - \cos\alpha\cos\beta\cos\gamma +
    \cos\alpha\sin\beta\sin\gamma`

    :math:`= \sin\beta(\cos\alpha\sin\gamma - \sin\alpha\cos\gamma)`

    :math:`= \sin\beta\sin(\gamma - \alpha) =` R.H.S.

11. L.H.S. :math:`= \sin(n + 1)A\sin(n - 1)A + \cos(n + 1)A\cos(n - 1)A`

    :math:`= \cos(n + 1 - (n - 1))A = \cos 2A =` R.H.S.

12. L.H.S. :math:`= \sin(n + 1)A\sin(n + 2)A + \cos(n + 1)A\cos(n + 2)A`

    :math:`= \cos(n + 1 - (n + 1)) = \cos A =` R.H.S.

13. :math:`\cos 15^\circ = \cos(45^\circ - \cos 30^\circ)`

    :math:`= \cos45^\circ\cos30^\circ + \sin45^\circ\sin30^\circ`

    :math:`= \frac{1}{\sqrt{2}}\frac{\sqrt{3}}{2} + \frac{1}{\sqrt{2}}\frac{1}{2}`

    :math:`= \frac{\sqrt{3} + 1}{2\sqrt{2}}`

    :math:`\sin 105^\circ = \sin(60^\circ + 45^\circ)`

    :math:`= \sin60^\circ\cos^45\circ + \cos60^\circ\sin45^\circ`

    :math:`= \frac{\sqrt{3}}{2}\frac{1}{\sqrt{2}} + \frac{1}{2}\frac{1}{\sqrt{2}}`

    :math:`= \frac{\sqrt{3} + 1}{2\sqrt{2}} =` R.H.S.

14. :math:`\tan 105^\circ = \tan(60^\circ + 45^\circ)`

    :math:`= \frac{\tan60^\circ + \tan 45^\circ}{1 - \tan60^\circ\tan 45^\circ}`

    :math:`= \frac{\sqrt{3} + 1}{1 - \sqrt{3}}`

15. :math:`\frac{\tan 495^\circ}{\cot 855^\circ} = \frac{\tan(360^\circ + 135^\circ)}{\cot(720^\circ + 135^\circ)}`

    :math:`= \frac{\tan 135^\circ}{\cot 135^\circ} = \tan^2135^\circ = (-1)^2 = 1`

16. :math:`\sin(\pi + \theta) = -\sin\theta \therefore \sin(n\pi + \theta) = (1)^n\sin\theta`

    :math:`\sin\left(n\pi + (-1)^n \frac{\pi}{4}\right) = (-1)^n\sin\left((-1)^n\frac{\pi}{4}\right)`

    :math:`= (-1)^n(-1)^n\sin \frac{\pi}{4}~[\because \sin(-\theta) = -\sin\theta]`

    :math:`= (-1)^{2n}\sin \frac{\pi}{4} = \frac{1}{\sqrt{2}}`

17. L.H.S. :math:`= \sin 15^\circ = \sin(60^\circ - 45^\circ)`

    :math:`= \sin60^\circ\cos45^\circ - \cos60^\circ\sin45^\circ`

    :math:`= \frac{\sqrt{3}}{2}\frac{1}{\sqrt{2}} - \frac{1}{2}\frac{1}{\sqrt{2}}`

    :math:`= \frac{\sqrt{3} - 1}{2\sqrt{2}} =` R.H.S.

18. L.H.S. :math:`= \cos 75^\circ = \cos(45^\circ + 30^\circ)`

    :math:`= \cos45^\circ\cos30^\circ - \sin45^\circ\sin30^\circ`

    :math:`= \frac{1}{\sqrt{2}}\frac{\sqrt{3}}{2} - \frac{1}{\sqrt{2}}\frac{1}{2}`

    :math:`= \frac{\sqrt{3} - 1}{2\sqrt{2}} =` R.H.S.

19. L.H.S. :math:`= \tan 75^\circ = \tan(45^\circ + 30^\circ)`

    :math:`= \frac{\tan45^\circ + \tan30^\circ}{1 - \tan45^\circ\tan30^\circ}`

    :math:`= \frac{1 + \frac{1}{\sqrt{3}}}{1 - 1.\frac{1}{\sqrt{3}}}`

    :math:`= \frac{\frac{\sqrt{3} + 1}{\sqrt{3}}}{\frac{\sqrt{3} - 1}{\sqrt{3}}}`

    :math:`= \frac{\sqrt{3} + 1}{\sqrt{3} - 1} = \frac{(\sqrt{3} + 1)^2}{3 - 1} = 2 + \sqrt{3} =` R.H.S.

20. L.H.S. :math:`= \tan 15^\circ = \tan(45^\circ - 30^\circ)`

    :math:`= \frac{\tan45^\circ - \tan30^\circ}{1 + \tan45^\circ\tan30^\circ}`

    :math:`= \frac{1 - \frac{1}{\sqrt{3}}}{1 + 1.\frac{1}{\sqrt{3}}}`

    :math:`= \frac{\frac{\sqrt{3} - 1}{\sqrt{3}}}{\frac{\sqrt{3} + 1}{\sqrt{3}}}`

    :math:`= \frac{\sqrt{3} - 1}{\sqrt{3} + 1} = \frac{(\sqrt{3} - 1)^2}{3 - 1} = 2 - \sqrt{3} =` R.H.S.

21. :math:`\cos 1395^\circ = \cos(3*360^\circ + 315^\circ) = \cos315^\circ = \cos(270^\circ + 45^\circ)`

    :math:`= \cos45^\circ = \frac{1}{\sqrt{2}}`

22. :math:`\tan(-330^\circ) = -\tan(330^\circ) = -\tan(270^\circ + 60^\circ) = =\cot 60^\circ = \frac{1}{\sqrt{3}}`

23. Given, :math:`\sin 300^\circ \cosec 1050^\circ - \tan(-120^\circ)`

    :math:`= \sin (270^\circ + 30^\circ)\cosec(720^\circ + 270^\circ + 60^\circ) + \tan(90^\circ + 30^\circ)`

    :math:`= -cos 30^\circ. \frac{1}{-cos 60^\circ} - \cot 30^\circ`

    :math:`= \frac{\sqrt{3}}{2}.\frac{2}{1} - \sqrt{3} = 0`

24. Given, :math:`\tan\left(\frac{11\pi}{12}\right)`

    :math:`= \tan\left(\pi - \frac{\pi}{12}\right) = -\tan15^\circ`

    Using the value computed in 20 for :math:`\tan15^\circ` we have :math:`\sqrt{3} - 2` as the answer.

25. We know that :math:`tan(-\theta) = -\tan\theta,` thus

    :math:`\tan \left((-1)^n\frac{\pi}{4}\right) = (-1)^n\tan\frac{\pi}{4} = (-1)^n`

26. Given, :math:`\cos 18^\circ - \sin 18^\circ = \sqrt{2}\sin 27^\circ`

    :math:`\frac{1}{\sqrt{2}}\cos\18^\circ - \frac{1}{\sqrt{2}}\sin18^\circ = \sin 27^\circ`

    L.H.S. :math:`= \sin45^\circ\cos18^\circ - \cos45^\circ\sin18^\circ`

    :math:`= \sin(45^\circ - 18^\circ) = \sin 27^\circ =` R.H.S.

27. L.H.S. :math:`=\tan 70^\circ = \tan(50^\circ + 20^\circ)`

    :math:`= \frac{\tan 50^\circ + \tan 20^\circ}{1 - \tan50^\circ\tan20^\circ}`

    :math:`\tan70^\circ - \tan70^\circ\tan50^\circ\tan20^\circ = \tan 50^\circ + \tan 20^\circ`

    :math:`\tan70^\circ = \tan70^\circ\tan50^\circ\tan20^\circ + \tan 50^\circ + \tan 20^\circ`

    :math:`= \tan(90^\circ - 20^\circ)\tan50^\circ\tan20^\circ + \tan 50^\circ + \tan 20^\circ`

    :math:`= \cot20^\circ\tan50^\circ\tan20^\circ + \tan 50^\circ + \tan 20^\circ`

    :math:`= \tan 50^\circ + \tan 50^\circ + \tan 20^\circ = 2\tan50^\circ + \tan20^\circ =` R.H.S.

28. L.H.S. :math:`= \frac{\cos\left(\frac{\pi}{4} + x\right)\cos\left(\frac{\pi}{4} - x\right)}{\sin\left(\frac{\pi}{4} +
    x\right)\sin\left(\frac{\pi}{4} - x\right)}`

    :math:`= \frac{\cos^2\frac{\pi}{4} - \sin^2x}{\sin^2\frac{\pi}{4} - \sin^2x} = \frac{\frac{1}{2} - \sin^2x}{\frac{1}{2} -
    \sin^2x} = 1 =` R.H.S.

29. L.H.S. :math:`= \cos(m + n)\theta.\cos(m - n)\theta - \sin(m + n)\theta\sin(m - n)\theta`

    :math:`= \cos(m + n + m - n)\theta = \cos2m\theta =` R.H.S.

30. L.H.S. :math:`= \frac{\tan(\theta + \phi) + \tan(\theta - \phi)}{1 - \tan(\theta + \phi)\tan(\theta - \phi)}`

    :math:`= \tan(\theta + \phi + \theta - \phi) = \tan 2\theta =` R.H.S.

31. Given :math:`\cos 9^\circ + \sin 9^\circ = \sqrt{2}\sin 54^\circ`

    :math:`\frac{1}{\sqrt{2}}\cos9^\circ + \frac{1}{\sqrt{2}}\sin9^\circ = \sin54^\circ`

    L.H.S. :math:`= \sin45^\circ\cos9^\circ + \cos45^\circ\sin9^\circ`

    :math:`= \sin(45^\circ + 9^\circ) = \sin 54^\circ =` R.H.S.

32. L.H.S. :math:`= \frac{\cos 20^\circ - \sin 20^\circ}{\cos 20^\circ + \sin 20^\circ}`

    Dividing both numerator and denominaor with :math:`\cos20^\circ,` we get

    :math:`= \frac{1 - \tan20^\circ}{1 + \tan20^\circ} = \frac{\tan 45^\circ - \tan20^\circ}{1 -
    \tan45^\circ\tan20^\circ}~[\because \tan45^\circ = 1]`

    :math:`= \tan(45^\circ - 20^\circ) = \tan 25^\circ =` R.H.S.

33. L.H.S. :math:`= \frac{\tan A + \tan B}{\tan A - \tan B}`

    :math:`= \frac{\frac{\sin A}{\cos A} + \frac{\sin B}{\cos B}}{\frac{\sin A}{\cos A} - \frac{\sin B}{\cos B}}`

    :math:`= \frac{\sin A\cos B + \sin B\cos A}{\sin A\cos B - \sin B\cos A} = \frac{\sin(A + B)}{\sin (A - B)} =` R.H.S.

34. L.H.S. :math:`= \frac{1}{\tan 3A - \tan A} - \frac{1}{\cot 3A - \cot A}`

    :math:`= \frac{1}{\tan 3A - \tan A} - \frac{1}{\frac{1}{\tan 3A} - \frac{1}{\tan A}}`

    :math:`= \frac{1}{\tan 3A - \tan A} - \frac{\tan A\tan 3A}{\tan A - \tan 3A}`

    :math:`= \frac{1 + \tan A \tan 3A}{\tan 3A - \tan A} = \frac{1}{\tan(3A - A)} = \cot 2A =` R.H.S.

35. This is similar to previous problema and can be solved likewise.

36. L.H.S. :math:`= \frac{\sin 3\alpha}{\sin\alpha} + \frac{\cos 3\alpha}{cos\alpha}`

    :math:`= \frac{\sin3\alpha\cos\alpha + \cos3\alpha\sin\alpha}{\sin\alpha\cos\alpha}`

    :math:`= \frac{\sin(3\alpha + \alpha)}{\sin\alpha\cos\alpha}`

    :math:`=2\frac{2\sin 4\alpha}{\sin2\alpha}~[\because \sin\alpha\cos\alpha = \frac{1}{2}\sin2\alpha]`

    :math:`= 2\frac{2\sin2\alpha\cos2\alpha}{\sin2\alpha} = 4\cos2\alpha =` R.H.S.

37. L.H.S. :math:`= \frac{\tan\left(\frac{\pi}{4} + A \right) - \tan\left(\frac{\pi}{4} - A\right)}{\tan\left(\frac{\pi}{4} + A\right) +
    \tan\left(\frac{\pi}{4} - A\right)}`

    :math:`= \frac{\frac{1 + \tan A}{1 - \tan A} - \frac{1 - \tan A}{1 + \tan A}}{\frac{1 + \tan A}{1 - \tan A} + \frac{1 - \tan
    A}{1 + \tan A}}`

    :math:`= \frac{(1 + \tan A)^2 - (1 - \tan A)^2}{(1 + \tan A)^2 + (1 - \tan A)^2}`

    :math:`= \frac{4\tan A}{2 + 2\tan^2A} = \frac{2\tan A}{\sec^2A} = 2\sin A\cos A = \sin 2A`

38. Given, :math:`\tan 40^\circ + 2 \tan 10^\circ = \tan 50^\circ`

    R.H.S. :math:`= \tan 50^\circ = \tan(40^\circ + 10^\circ)`

    :math:`= \frac{\tan 40^\circ + \tan 10^\circ}{1 - \tan 40^\circ\tan 10^\circ}`

    :math:`\tan50^\circ - \tan50^\circ\tan40^\circ\tan10^\circ = \tan 40^\circ + \tan 10^\circ`

    :math:`\tan50^\circ - \cot40^\circ\tan40^\circ\tan10^\circ = tan40^\circ + \tan10^\circ`

    :math:`\tan50^\circ = \tan 40^\circ + 2 \tan 10^\circ`

39. R.H.S. :math:`= \tan(\alpha + \beta)\tan(\alpha - \beta)`

    :math:`= \frac{\sin(\alpha + \beta)}{\cos(\alpha + \beta)}\frac{\sin(\alpha -\beta)}{\cos(\alpha - \beta)}`

    :math:`= \frac{\sin\alpha\cos\beta + \cos\alpha\sin\beta}{\cos\alpha\cos\beta - \sin\alpha\sin\beta}\frac{\sin\alpha\cos\beta -
    \cos\alpha\sin\beta}{\cos\alpha\cos\beta + \sin\alpha\sin\beta}`

    :math:`= \frac{\sin^2\alpha\cos^2\beta - \sin^2\beta\cos^2\alpha}{\cos^2\alpha\cos^2\beta - \sin^2\alpha\sin^2\beta}`

    
