************************************
Inverse Circular Functions Solutions
************************************
1. Let :math:`\tan^{-1}(-1) = \theta` then :math:`\tan\theta = -1.` Also, :math:`-\frac{\pi}{2}< \theta < \frac{\pi}{2}`

   The only value in this range which satisfied this equation is :math:`-\frac{\pi}{4}.`

2. Let :math:`\cot^{-1}(-1) = \theta,` then :math:`\cot\theta = -1` and :math:`0<\theta<\pi`

   :math:`\Rightarrow \theta = \frac{3\pi}{4}`

3. Let :math:`\sin^{-1}\left(-\frac{\sqrt{3}}{2}\right) = \theta` then :math:`\sin\theta = -\frac{\sqrt{3}}{2}`

   Also, :math:`-\frac{\pi}{2}\leq \theta\leq \frac{\pi}{2} \Rightarrow \theta = -\frac{\pi}{3}`

4. :math:`\sin\left[\frac{\pi}{3} -\sin^{-1}\left(-\frac{1}{2}\right)\right]`

   :math:`=\sin\left[\frac{\pi}{3} -\{-\sin^{-1}\frac{1}{2}\}\right]`

   :math:`= \sin\left[\frac{\pi}{3} + \frac{\pi}{6}\right] = 1`

5. :math:`\sin\left[\cos^{-1}\left(-\frac{1}{2}\right)\right] = \sin\left[\pi - \cos^{-1}\frac{1}{2}\right]`

   :math:`= \sin\frac{2\pi}{3} = \frac{\sqrt{3}}{2}`

6. :math:`\sin\left[\tan^{-1}(-\sqrt{3}) + \cos^{-1}\frac{-\sqrt{3}}{2}\right]`

   :math:`= \sin\left[-\frac{\pi}{3} + \pi- \frac{\pi}{6}\right]`

   :math:`= \sin\frac{\pi}{2} = 1`

7. Given expression is :math:`\tan\left[\frac{1}{2}\cos^{-1}\frac{\sqrt{5}}{3}\right]`

   Let :math:`\cos^{-1}\frac{\sqrt{5}}{3} = 2\theta` then :math:`\cos2\theta = \frac{\sqrt{5}}{3}`

   :math:`\Rightarrow \frac{1 - \tan^2\theta}{1 + \tan^2\theta} = \frac{\sqrt{5}}{3}`

   By componendo and dividendo :math:`\frac{2\tan^2\theta}{2} = \frac{3 - \sqrt{5}}{3 + \sqrt{5}}`

   :math:`\Rightarrow \tan\theta = \pm\left(\frac{3 - \sqrt{5}}{2}\right)`

   Given :math:`0 \leq 2\theta \leq \pi \Rightarrow 0\leq \theta \leq \frac{\pi}{2}`

   i.e. :math:`\theta` lies in first quadrant. :math:`\Rightarrow \tan\theta = \frac{3 - \sqrt{5}}{2}`

8. Given expression is :math:`\sin^{-1}\left(\sin\frac{2\pi}{3}\right)`

   Let :math:`\sin^{-1}\left(\sin\frac{2\pi}{3}\right) = \theta`

   then :math:`\sin\theta = \sin\frac{2\pi}{3}` and :math:`-\frac{\pi}{2}\leq\theta\leq \frac{\pi}{2}`

   :math:`=\sin\left(\pi - \frac{\pi}{3}\right) = \sin\frac{\pi}{3} \Rightarrow \theta = \frac{\pi}{3}`

   :math:`\sin^{-1}\left(\sin\frac{2\pi}{3}\right) = \frac{\pi}{3}`

9. Let :math:`\sin^{-1}\frac{\sqrt{3}}{2} = \theta \Rightarrow \sin\theta = \frac{\sqrt{3}}{2}`

   :math:`\Rightarrow \theta = \frac{\pi}{3}` :math:`-\frac{\pi}{2}\leq\theta\leq \frac{\pi}{2}`

10. Let :math:`\tan^{-1}\frac{-1}{\sqrt{3}} =\theta`

    then :math:`\tan\theta = \frac{-1}{\sqrt{3}} =\tan\left(\frac{-\pi}{3}\right)`

    :math:`\Rightarrow \theta = -\frac{\pi}{3}`

11. Let :math:`\cot^{-1}(-\sqrt{3}) = \theta \Rightarrow \cot\theta = -\sqrt{3}`

    :math:`\cot\theta = \cot\left(\pi - \frac{\pi}{6}\right)`

    :math:`\theta = \frac{5\pi}{6}`

12. Let :math:`\cot^{-1}\cot\frac{5\pi}{4} = \theta \Rightarrow \cot\theta = \cot\left(\pi + \frac{\pi}{4}\right)`

    :math:`\cot\theta = \cot\frac{\pi}{4} \Rightarrow \theta = \frac{\pi}{4}`

13. Let :math:`\tan^{-1}\left(\tan\frac{3\pi}{4}\right) = \theta`

    :math:`\Rightarrow \tan\theta = \tan\frac{3\pi}{4} = \tan\left(\pi - \frac{\pi}{4}\right)`

    :math:`\Rightarrow \theta = -\frac{\pi}{4}`

14. :math:`\sin^{-1}\frac{1}{2} + \cos^{-1}\frac{1}{2} = \frac{\pi}{6} + \frac{\pi}{3} = \frac{\pi}{2}`

15. Let :math:`\tan^{-1} = \theta \Rightarrow \tan\theta = \frac{3}{4} \Rightarrow \cos\theta = \frac{4}{5}`

16. :math:`\cos\left[\cos^{-1}\left(\frac{\sqrt{3}}{2}\right) + \frac{\pi}{6}\right]`

    :math:`=\cos\left[\frac{\pi}{6} + \frac{\pi}{6}\right] = \cos \frac{\pi}{3} = \frac{1}{2}`

17. L.H.S. :math:`= 2\tan^{-1}\frac{1}{3} + \tan^{-1}\frac{1}{7}`

    :math:`= \tan^{-1}\frac{2*\frac{1}{3}}{1 - \frac{1}{9}} + \tan^{-1}\frac{1}{7}`

    :math:`= \tan^{-1}\frac{3}{4} + \tan^{-1}\frac{1}{7}`

    :math:`= \tan^{-1}\frac{\frac{3}{4} + \frac{1}{7}}{1 - \frac{3}{28}} = \tan^{-1}1 = \frac{\pi}{4} =` R.H.S.

18. L.H.S. :math:`= \tan^{-1}\frac{1}{3} + \tan^{-1}\frac{1}{7} + \tan^{-1}\frac{1}{5} + \tan^{-1}\frac{1}{8}`

    :math:`= \tan^{-1}\frac{\frac{1}{3} + \frac{1}{7}}{1 - \frac{1}{21}} + \tan^{-1}\frac{\frac{1}{5} + \frac{1}{8}}{1 -
    \frac{1}{40}}`

    :math:`= \tan^{-1}\frac{1}{2} + \tan^{-1}\frac{1}{3} = \tan^{-1}1 = \frac{\pi}{4} =` R.H.S.

19. L.H.S. :math:`= \sin^{-1}\frac{4}{5} + \sin^{-1}\frac{5}{13} + \sin^{-1}\frac{16}{65}`

    :math:`= \sin^{-1}\left(\frac{4}{5}\sqrt{1 - \frac{25}{169}} + \frac{5}{13}\sqrt{1 - \frac{16}{25}}\right) +
    \sin^{-1}\frac{16}{65}`

    :math:`= \sin^{-1}\left(\frac{48}{65} + \frac{15}{65}\right) + \sin^{-1}\frac{16}{65} = \sin^{-1}\frac{64}{65} +
    \sin^{-1}\frac{16}{65}`

    :math:`= \sin^{-1}\left(\frac{63}{65}.\sqrt{1 - \frac{16^2}{65^2}} + \frac{16}{65}\sqrt{1 - \frac{63^2}{65^2}}\right)`

    :math:`\sin^{-1}\frac{63^2 + 16^2}{65^2} = \sin^{-1} = \frac{\pi}{2} =` R.H.S.

20. We have to prove that :math:`4\tan^{-1}\frac{1}{5} - \tan^{-1}\frac{1}{70} + \tan^{-1}\frac{1}{99} = \frac{\pi}{4}`

    :math:`\Rightarrow 4\tan^{-1}\frac{1}{5} = \frac{\pi}{4} + \tan^{-1}\frac{1}{70} - tan^{-1}\frac{1}{99}`

    L.H.S. :math:`= 4\tan^{-1}\frac{1}{5} = 2\tan^{-1}\frac{2.\frac{1}{5}}{1 - \frac{1}{25}} = 2\tan^{-1}\frac{5}{12}`

    :math:`= \tan^{-1}\frac{2.\frac{5}{12}}{1 - \frac{25}{144}} = \tan^{-1}\frac{120}{119}`

    :math:`\tan^{-1}\frac{1}{70} - \tan^{-1}\frac{1}{99} = \tan^{-1}\frac{\frac{1}{70} - \frac{1}{99}}{1 +
    \frac{1}{70}.\frac{1}{99}}`

    :math:`= \tan^{-1}\frac{1}{239}`

    R.H.S. :math:`= \tan^{-1}1 + \tan^{-1}\frac{1}{239} = \tan^{-1}\frac{120}{119}`

    Thus, L.H.S. = R.H.S.

21. We have to prove that :math:`\cot^{-1}9 + \cosec^{-1}\frac{\sqrt{41}}{4} = \frac{\pi}{4}`

    :math:`\cot^{-1}9 = \tan^{-1}\frac{1}{9}`

    Let :math:`\cosec^{-1}\frac{\sqrt{41}}{4} = \theta \Rightarrow \cosec\theta = \frac{\sqrt{41}}{4}`

    Since we have to consider principal values only :math:`-\frac{\pi}{2}\leq \theta\leq \frac{\pi}{2}` and :math:`\theta \neq 0`

    As :math:`\cosec\theta` is +ve here, :math:`\theta` lies between :math:`0` and :math:`\pi/2,` hence :math:`\tan\theta` must be
    positive.

    :math:`\Rightarrow \tan\theta = \frac{4}{5}`

    :math:`\tan^{-1}\frac{1}{9} + \tan^{-1}\frac{4}{5} = \tan^{-1}\frac{\frac{1}{9} + \frac{4}{5}}{1 - \frac{1}{9}\frac{4}{5}}`

    :math:`=\tan^{-1}\frac{41}{45}.\frac{45}{41} = \tan^{-1}1 = \frac{\pi}{4} =` R.H.S.
