Multiple and Submultiple Angles Solutions
*****************************************
1. Let us solve these one by one.

   i. Given, :math:`\cos A = \frac{3}{5}`

      :math:`\Rightarrow \sin A = \sqrt{1 - \cos^2A} = \sqrt{1 - \frac{9}{25}} = \sqrt{\frac{16}{25}} = \frac{4}{5}`

      :math:`\sin 2A = 2\sin A\cos A = 2.\frac{4}{5}.\frac{3}{5} = \frac{24}{25}`

   ii. Given, :math:`\sin A = \frac{12}{13}`

       :math:`\Rightarrow \cos A = \sqrt{1 - \sin^2A} = \sqrt{1 - \frac{144}{169}} = \sqrt{\frac{25}{169}} = \frac{5}{13}`

       :math:`\sin 2A = 2\sin A\cos A = 2.\frac{12}{13}.\frac{5}{13} = \frac{120}{169}`

   iii. Given, :math:`\tan A = \frac{16}{63} = \frac{\text{perpendicular}}{\text{base}}`

        :math:`\text{hypotenuse} = \sqrt{p^2 + b^2} = \sqrt{16^2 + 63^2} = 65`

        :math:`\sin A = \frac{16}{65}, \cos A = \frac{63}{65}`

        :math:`\sin 2A = 2\sin A\cos A = 2.\frac{16}{65}.\frac{63}{65} = \frac{2016}{4225}`

2. Let us solve these one by one.

   i. Given, :math:`\cos A = \frac{15}{17}`

      :math:`\Rightarrow \sin A = \sqrt{1 - \cos^2A}` :math:`= \sqrt{1 - \frac{225}{289}} = \sqrt{\frac{64}{289}} = \frac{8}{17}`

      :math:`\cos 2A = \cos^2A - \sin^2A = \frac{225 - 64}{289} = \frac{161}{289}`

   ii. Given, :math:`\sin A = \frac{4}{5}`

       :math:`\Rightarrow \cos A = \sqrt{1 - \sin^2A}` :math:`= \sqrt{1 - \frac{16}{25}} = \frac{3}{5}`

       :math:`\cos2A = \cos^2A - \sin^2A = \frac{9 - 16}{25} = -\frac{7}{25}`

   iii. Give, :math:`\tan A = \frac{5}{12} = \frac{\text{perpendicular}}{\text{base}}`

        :math:`\text{hypotenuse} = \sqrt{p^2 + b^2} = \sqrt{25 + 144} = 13`

        :math:`\sin A = \frac{5}{13}, \cos A = \frac{12}{13}`

        :math:`\cos^2A = \cos^2A - \sin^2A = \frac{119}{169}`

3. Given, :math:`\tan A = \frac{b}{a},` thus :math:`\text{hypotenuse} = \sqrt{b^2 + a^2}`

   :math:`a\cos 2A+ b\sin 2A = a(\cos^2A - \sin^2A) + 2b\sin A\cos A`

   :math:`= a\left(\frac{a^2}{a^2 + b^2} - \frac{b^2}{a^2 + b^2}\right) + 2b.\frac{ab}{a^2 + b^2}`

   :math:`= a\left(\frac{a^2 - b^2 + 2b^2}{a^2 + b^2}\right) = a`

4. We have to prove that :math:`\frac{\sin 2A}{1 + \cos 2A} = \tan A`

   L.H.S. :math:`= \frac{\sin 2A}{1 + \cos 2A} = \frac{2\sin A\cos A}{1 + \cos^2A - \sin^2A}`

   :math:`= \frac{2\sin A\cos A}{2\cos^2A}[\because 1 - \sin^2A = \cos^2A]`

   :math:`= \tan A =` R.H.S.

5. We have to prove that :math:`\frac{\sin 2A}{1 - \cos 2A} = \cot A`

   L.H.S. :math:`= \frac{\sin 2A}{1 - \cos 2A} = \frac{2\sin A\cos A}{1 -(\cos^2A - \sin^2A)}`

   :math:`= \frac{2\sin A\cos A}{2\sin^2A} = \cot A =` R.H.S.

6. We have to prove that :math:`\frac{1 - \cos 2A}{1 + \cos 2A} = \tan^2A`

   L.H.S. :math:`= \frac{1 - (\cos^2A - \sin^2A)}{1 + \cos^2A - \sin^2A}`

   :math:`= \frac{2\sin^2A}{2\cos^2A} = \tan^2A =` R.H.S.

7. We have to prove that :math:`\tan A + \cot A = 2\cosec 2A`

   L.H.S. :math:`= \frac{\sin A}{\cos A} + \frac{\cos A}{\sin A} = \frac{\sin^2A + \cos^2A}{\sin A\cos A}`

   :math:`= \frac{2}{2\sin A\cos A} = \frac{2}{\sin 2A} = 2\cosec 2A =` R.H.S.

8. We have to prove that :math:`\tan A - \cot A = -2\cot2A`

   L.H.S. :math:`= \frac{\sin A}{\cos A} - \frac{\cos A}{\sin A} = \frac{\sin^2A - \cos^2A}{\sin A\cos A}`

   :math:`= \frac{-\cos2A}{\frac{\sin2A}{2}} = -2\cot2A =` R.H.S.

9. We have to prove that :math:`\cosec 2A + \cot 2A = \cot A`

   L.H.S. :math:`= \frac{1}{\sin 2A} + \frac{\cos 2A}{\sin 2A} = \frac{1 + \cos 2A}{\sin 2A} = \frac{2\cos^2A}{2\sin A\cos A}`

   :math:`= \cot A =` R.H.S.
