Properties of Triangles' Solutions Part 2
*****************************************
51. The diagram is given below:

   .. image:: _static/images/18_8.png
      :alt: Problem 51
      :align: center

   From figure, :math:`\angle ADC = 90^\circ + B`

   By applying :math:`m:n` rule in triangle :math:`ABC,` we get

   :math:`(1 + 1)\cot(90^\circ + B) = 1.\cot90^\circ - 1.\cot(A-90^\circ)`

   :math:`-2\tan B = 0 - \cot[-(90^\circ - A)]`

   :math:`-2\tan B = \tan A \Rightarrow \tan A + 2\tan B = 0`

52. Given, :math:`\cot A + \cot B + \cot C = \sqrt{3}`

    Squaring, :math:`\cot^2A + \cot^2B + \cot^2C + 2\cot A\cot B + 2\cot B\cot C + 2\cot C\cot A = 3`

    Since :math:`A + B + C = \pi \Rightarrow A + B = \pi - C`

    :math:`\cot(A + B) = \cot(\pi - C)`

    :math:`\frac{\cot A\cot B - 1}{\cot A + \cot B} = -\cot C`

    :math:`\cot A\cot B + \cot B\cot C + \cot C\cot A = 1`

    :math:`\Rightarrow \cot^2A + \cot^2B + \cot^2C + 2\cot A\cot B + 2\cot B\cot C + 2\cot C\cot A = 3(\cot A\cot B + \cot B\cot C +
    \cot C\cot A)`

    :math:`\frac{1}{2}[(\cot A - \cot B)^2 + (\cot B - \cot C)^2 + (\cot C - \cot A)^2] = 0`

    :math:`\Rightarrow \cot A = \cot B = \cot C`

    :math:`\Rightarrow A = B = C` i.e. triangle is equilateral.

53. Given, :math:`(a^2 + b^2)\sin(A - B) = (a^2 - b^2)\sin(A + B)`

    :math:`(\sin^2A + \sin^2B)\sin(A - B) = (\sin^2A - \sin^2B)\sin(A + B)`

    :math:`[\because \sin^2A - \sin^2B = \sin(A + B)\sin(A - B)]`

    :math:`\Rightarrow (\sin^2A + \sin^2B)\sin(A - B) = \sin^2(A + B)\sin(A - B)`

    :math:`\Rightarrow \sin(A - B)[\sin^2A + \sin^2B - \sin^2C] = 0`

    Either :math:`\sin(A - B) = 0` or :math:`\sin^2A + \sin^2B - \sin^2C = 0`

    :math:`A = B` or :math:`a^2 + b^2 - c^2 = 0`

    Thus, triangle is either isosceles or right angled.

54. R.H.S. :math:`= c(\cos A\cos\theta + \sin A\sin\theta) + a(\cos C\cos\theta - \sin C\sin\theta)`

    :math:`= \cos\theta(c\cos A + a\cos C) + \sin\theta(c\sin A - a\sin C)`

    :math:`=b\cos\theta + \sin\theta\left(c.\frac{a}{2R} - a.\frac{c}{2R}\right)`

    :math:`= b\cos\theta =` L.H.S.

55. The diagram is given below:

    .. image:: _static/images/18_9.png
       :alt: Problem 51
       :align: center

    :math:`\frac{b}{\sin(B + \theta)} = \frac{a}{2\sin(A - \theta)}`

    :math:`\frac{c}{\sin[\pi -(B + \theta)]} = \frac{a}{2\sin\theta}`

    :math:`\Rightarrow b\sin(A - \theta) = c\sin\theta`

    :math:`\Rightarrow \sin B(\sin A\cos\theta - \cos A\sin\theta) = \sin C\sin\theta = (\sin A\cos B + \sin B \cos A)\sin\theta`

    :math:`\Rightarrow \cot\theta = 2\cot A + \cot B`

56. The diagram is given below:

    .. image:: _static/images/18_10.png
       :alt: Problem 56
       :align: center

    :math:`\Delta ABC = \Delta ABD + \Delta ACD`

    :math:`\frac{1}{2}bc\sin A = \frac{1}{2}AD.c\sin\frac{A}{2} + \frac{1}{2}AD.b\sin\frac{A}{2}`

    :math:`\Rightarrow AD = \frac{2bc}{b + c}\cos\frac{A}{2}`

57. The diagram is given below:

    .. image:: _static/images/18_11.png
       :alt: Problem 57
       :align: center

    :math:`\angle ACB = \pi - (\alpha + \beta + \gamma)`

    :math:`\sin ACB = \sin(\alpha + \beta + \gamma)`

    In :math:`\triangle ABC`

    :math:`\frac{AB}{\sin ACB} = \frac{AC}{\sin\gamma}`

    :math:`AC = \frac{a\sin\gamma}{\sin(\alpha + \beta + \gamma)}`

    In :math:`\triangle ACD`

    :math:`\frac{CD}{\sin\alpha} = \frac{AC}{\sin\beta}`

    :math:`CD = \frac{a\sin\alpha\sin\gamma}{\sin\beta\sin(\alpha + \beta + \gamma)}`

58. Given, :math:`2\cos A = \frac{\sin B}{\sin C}`

    :math:`2\cos A\sin C = \sin B = \sin[\pi - (A + C)] = \sin(A + C)`

    :math:`2\cos A\sin C = \sin A\cos C + \cos A\sin C`

    :math:`\cos A\sin C = \sin A\cos C\Rightarrow \tan A = \tan C`

    :math:`\Rightarrow A = C`

    Thus, the triangle is isosceles.

59. Let such angles be :math:`A` and :math:`B.` Then,

    :math:`\cos A = \frac{1}{a}` and :math:`\cos B = \frac{1}{b}`

    :math:`\Rightarrow \sin A\cos A = \sin B\cos B`

    :math:`\sin 2A = \sin 2B` or :math:`\sin 2A = \sin[\pi - 2B]`

    :math:`A = B` or :math:`A + B = \frac{\pi}{2} \Rightarrow C = \frac{\pi}{2}`

    Thus, the triangle is either isosceles or right angled.

60. Given :math:`a\tan A + b\tan B = (a + b)\tan \frac{A + B}{2}`

    :math:`\Rightarrow a\left(\frac{\sin A}{\cos A} - \frac{\sin \frac{A + B}{2}}{\cos\frac{A + B}{2}}\right) =
    b\left(\frac{\sin\frac{A + B}{2}}{\cos \frac{A + B}{2}} - \frac{\sin B}{\cos B}\right)`

    :math:`\Rightarrow a.\frac{\sin\frac{A - B}{2}}{\cos A\cos \frac{A + B}{2}} = b.\frac{\sin\frac{A - B}{2}}{\cos B\cos\frac{A +
    B}{2}}`

    :math:`\Rightarrow \tan A = \tan B \Rightarrow A = B`

    Thus, the triangle is isosceles.

61. Given, :math:`\frac{\tan A - \tan B}{\tan A + \tan B} = \frac{c - b}{c}`

    :math:`\Rightarrow \frac{\frac{\sin A}{\cos A} - \frac{\sin B}{\cos B}}{\frac{\sin A}{\cos A} + \frac{\sin B}{\cos B}} =
    \frac{\sin C - \sin B}{\sin C}`

    :math:`\Rightarrow \frac{\sin A\cos B - \sin B\cos A}{\sin A\cos B + \sin B\cos A} = \frac{\sin (A + B) - \sin B}{\sin (A + B)}`

    :math:`\Rightarrow \frac{\sin A\cos B - \sin B\cos A}{\sin(A + B)} = \frac{\sin(A + B) - \sin B}{\sin(A + B)}`

    :math:`\Rightarrow \sin A\cos B - \sin B\cos A = \sin A\cos B + \sin B\cos A - \sin B`

    :math:`\Rightarrow \sin B = 2\sin B\cos A \Rightarrow \cos A = \frac{1}{2} \Rightarrow A = 60^\circ.`

62. We know that :math:`\cos C = \frac{a^2 + b^2 - c^2}{2ab}`

    Given, :math:`c^4 - 2(a^2 + b^2)c^2 + a^4 + a^2b^2 + b^4 = 0`

    :math:`\Rightarrow a^4 + b^4 + c^4 - 2a^2c^2 - 2b^2c^2 + 2a^2b^2 = a^2b^2`

    :math:`(a^2 + b^2 -c^2)^2 = a^2b^2 \Rightarrow a^2 + b^2 + c^2 = \pm ab`

    :math:`\Rightarrow \cos C = \pm\frac{1}{2} \Rightarrow A = 60^\circ` or :math:`120^\circ`

63. Given, :math:`\frac{\cos A + 2\cos C}{\cos A + 2\cos B} = \frac{\sin B}{\sin C}`

    :math:`\Rightarrow \cos A(\sin C - \sin B) = 2\sin B\cos B - 2\sin C\cos C = \sin 2B - \sin 2C`

    :math:`\Rightarrow 2\cos A.\cos\frac{B + C}{2}\sin\frac{C - B}{2} = 2\cos(B + C)\sin(B - C)`

    :math:`\cos A.\cos\frac{B + C}{2}\sin\frac{C - B}{2} = -2\cos A.\sin\frac{B - C}{2}.\cos\frac{B - C}{2}`

    If :math:`B = C` then above it :math:`0 = 0` i.e. triangle is isosceles.

    If :math:`A = 90^\circ` then above is :math:`0 =0` i.e. triangle is right angled.

64. :math:`\because \tan\frac{A}{2}, \tan\frac{B}{2}, \tan\frac{C}{2}` are in A.P.

    :math:`\tan\frac{A}{2} - \tan\frac{B}{2} = \tan\frac{B}{2} - \tan \frac{C}{2}`

    :math:`\frac{\sin\left(\frac{A}{2} - \frac{B}{2}\right)}{\cos\frac{A}{2}\cos\frac{B}{2}} = \frac{\sin\left(\frac{B}{2} -
    \frac{C}{2}\right)}{\cos\frac{B}{2}\cos\frac{C}{2}}`

    :math:`\sin\left(\frac{A}{2} - \frac{B}{2}\right)\cos\frac{C}{2} = \sin\left(\frac{B}{2} - \frac{C}{2}\right)\cos\frac{A}{2}`

    :math:`\sin\left(\frac{A}{2} - \frac{B}{2}\right)\sin\left(\frac{A}{2} + \frac{B}{2}\right) = \sin\left(\frac{B}{2} -
    \frac{C}{2}\right)\sin\left(\frac{B}{2} + \frac{C}{2}\right)`

    :math:`\Rightarrow \cos B - \cos A = \cos C - \cos B`

    Thus, :math:`\cos A, \cos B, \cos C` are in A.P.

65. Given, :math:`a\cos^2\frac{C}{2} + c\cos^2\frac{A}{2} = \frac{3b}{2}`

    :math:`a.\frac{s(s - c)}{ab} + c.\frac{s(s - a)}{bc} = \frac{3b}{2}`

    :math:`\frac{s}{b}[2s - a - c] = \frac{3b}{2}`

    :math:`2s = 3b \Rightarrow a + c = 2b`

    We have to prove that :math:`\cot\frac{A}{2} + \cot\frac{C}{2} = 2\cot\frac{B}{2}`

    L.H.S. :math:`= \frac{s(s - a)}{\Delta} + \frac{s(s - c)}{\Delta}`

    :math:`= \frac{s}{\Delta}(2s - a - c) = \frac{2s(s - b)}{\Delta} = 2\cot\frac{B}{2} =` R.H.S.

66. Given, :math:`a^2, b^2, c^2` are in A.P.

    :math:`\Rightarrow b^2 - a^2 = c^2 - b^2`

    :math:`\Rightarrow \sin^2B - \sin^2A = \sin^2C - \sin^2B`

    :math:`\Rightarrow \sin(B + A)\sin(B - A) = \sin(C + B)\sin(C - B)`

    :math:`\Rightarrow \sin C\sin(B - A) = \sin A\sin(C - B)`

    :math:`\Rightarrow \frac{\sin A\cos B - \cos B\sin A}{\sin A\sin B} = \frac{\sin B\cos C - \sin C\cos B}{\sin B\sin C}`

    :math:`\Rightarrow \cot B - \cot A = \cot C - \cot B`

    :math:`\therefore \cot A, \cot B, \cot C` are in A.P.

67. Since :math:`A, B, C` are in A.P. :math:`\Rightarrow 2B = A + C \Rightarrow A + B + C = 3B = 180^\circ \Rightarrow B = 60^\circ`

    Given, :math:`2b^2 = 3c^2`

    :math:`2.\sin^2B = 3.\sin^2C \Rightarrow \sin C = \pm\frac{1}{\sqrt{2}}`

    :math:`\sin C\neq -\frac{1}{\sqrt{2}}` because :math:`C < 120^\circ`

    :math:`\sin C = \frac{1}{\sqrt{2}} \Rightarrow C = 45^\circ`

    :math:`\Rightarrow A = 75^\circ`

68. Given, :math:`\tan\frac{A}{2}, \tan\frac{B}{2}, \tan\frac{C}{2}` are in H.P.

    :math:`\Rightarrow \cot \frac{A}{2}, \cot\frac{B}{2}, \cot\frac{C}{2}` are in A.P.

    :math:`\cot\frac{B}{2} - \cot\frac{A}{2} = \cot\frac{C}{2}- \cot\frac{B}{2}`

    :math:`\frac{s(s - b) - s(s - a)}{\Delta} = \frac{s(s - c) - s(s - b)}{\Delta}`

    :math:`a - b = b - c`

    :math:`a, b, c` are in A.P.

69. Given, :math:`\frac{\sin A}{\sin C} = \frac{\sin(A - B)}{\sin(B - C)}`

    :math:`\frac{\sin A}{\sin C} = \frac{\sin A\cos B - \sin B \cos A}{\sin B\cos C - \sin C\cos B}`

    :math:`\sin A\sin C\cos C + \sin B\sin C\cos A = 2\sin A\sin C\cos B`

    :math:`\sin B\sin(A + C) = 2\sin A\sin C\cos B`

    :math:`\sin^2B = 2\sin A\sin C\cos B`

    :math:`\cos B = \frac{b^2}{2ac} = \frac{a^2 + c^2 - b^2}{2ac}`

    :math:`\Rightarrow c^2 + a^2 = 2b^2`

    Thus, :math:`a^2, b^2, c^2` are in A.P.

70. Given, :math:`2\sin B = \sin A + \sin C`

    :math:`4\sin\frac{B}{2}\cos\frac{B}{2} = 2\sin\frac{A + C}{2}\cos\frac{A - C}{2} = 2\cos\frac{B}{2}\cos\frac{A - C}{2}`

    :math:`2\sin\frac{B}{2} = 3\cos\frac{A + C}{2} = \cos\frac{A - C}{2}`

    :math:`3\sin\frac{A}{2}\sin\frac{C}{2} = \cos\frac{A}{2}\cos\frac{C}{2}`

    :math:`3\tan\frac{A}{2}\tan\frac{C}{2} = 1`

71. Given, :math:`a^2, b^2, c^2` are in A.P.

    :math:`b^2 - a^2 = c^2 - b^2`

    :math:`\sin^2B - \sin^2A = \sin^2C - \sin^2B`

    :math:`\sin(A + B)\sin(A - B) = \sin(B + C)\sin(B - C)`

    :math:`\sin C\sin(A - B) = \sin A\sin(B - C)`

    :math:`\cos B -\cot A\sin B = \sin B\cot C - \cos B`

    :math:`2\cos B = \sin B(\cot A + \cot C)`

    :math:`2\cot B = \cot A + \cot C`

    :math:`\therefore \cot A, \cot B, \cot C` are in A.P.

    :math:`\therefore \tan A,\tan B, \tan C` are in H.P.

72. We have proven in previous problem that :math:`\therefore \cot A, \cot B, \cot C` are in A.P.

73. Since :math:`A, B, C` are in A.P. :math:`\Rightarrow 2B = A + C \Rightarrow A + B + C = 3B = 180^\circ \Rightarrow B =
    60^\circ`

    :math:`b:c = \sqrt{3}:\sqrt{2} \Rightarrow \sin C = \frac{\sqrt{3}}{2}.\sqrt{\frac{2}{3}} = \frac{1}{\sqrt{2}}`

    :math:`\Rightarrow C = 45^\circ \Rightarrow A = 75^\circ`

74. Let the sides are :math:`a, b, c` then :math:`2b = a + c.` Also, let :math:`a` to be greatest and :math:`c` to be smallest
    side.

    Then, :math:`A = 90 + C` then :math:`90 + C + B + C = 180 \Rightarrow B = 90 -2C`

    :math:`\frac{a}{\sin(90 + C)} = \frac{b}{\sin(90 - 2C)} = \frac{c}{\sin C} = 2R`

    :math:`4R\cos2C = 2R\cos C + 2R\sin C`

    :math:`2\cos 2C = \cos C + \sin C`

    Squaring, we get

    :math:`4(1 - \sin^22C) = 1 + \sin 2C \Rightarrow \sin2C = \frac{3}{4}` when :math:`1 + \sin 2C \neq 0`

    When :math:`1 + \sin 2C = 0 \Rightarrow C = \frac{3\pi}{4}` which is not possible.

    :math:`\because \sin 2C = \frac{3}{4} \Rightarrow \cos 2C = \frac{\sqrt{7}}{4}`

    Now :math:`\sin C` and :math:`\cos C` can be found and ratio can be evaluated.

75. :math:`\because a, b, c` are in A.P.:math:`2b = a + c \Rightarrow a = 2b - c`

    :math:`\cos A = \frac{b^2 + c^2 - a^2}{2bc} = \frac{b^2 + c^2 -4b^2 -c^2 +4bc}{2bc}`

    :math:`= \frac{4bc - 3b^2}{2bc} =\frac{4c - 3b}{2c}`

76.
