Properties of Triangles' Solutions Part 3
*****************************************
101. The diagram is given below:

   .. image:: _static/images/18_15.png
      :alt: Problem 101
      :align: center

   Let :math:`BD = DE = EC = x.` Also let,

   :math:`\angle BAD = \alpha, \angle DAE = \beta, EAC = \gamma, CEA = \theta`

   Given, :math:`\tan\alpha = t_1, \tan\beta = t_2, \tan\gamma = t_3`

   Applying :math:`m:n` rule in :math:`\triangle ABC,` we get

   :math:`(2x + x)\cot\theta = 2x\cot(\alpha + beta) - x\cot\gamma`

   From :math:`\triangle ADC,` we get

   :math:`2x\cot\theta = x\cot\beta - x\cot\gamma`

   :math:`\Rightarrow \frac{3}{2} = \frac{2(\alpha + \beta) - \cot\gamma}{\cot\beta - \cot\gamma}`

   :math:`\Rightarrow 3\cot\beta - 3\cot\gamma = 4\cot(\alpha + \beta) - 2\cot\gamma`

   :math:`3\cot\beta - \cot\gamma = \frac{4(\cot\alpha\cot\beta - 1)}{\cot\alpha + \cot\beta}`

   :math:`3\cot^2\beta - \cot\beta\cot\gamma + 3\cot\alpha\cot\beta - \cot\alpha\cot\gamma = 4\cot\alpha\cot\beta - 4`

   :math:`4 + 4\cot^2\beta = \cot^2\beta + \cot\alpha\cot\beta + \cot\beta\cot\gamma + \cot\alpha\cot\gamma`

   :math:`4(1 + \cot^2\beta) = (\cot\beta + \cot\alpha)(\cot\beta + \cot\gamma)`

   :math:`4\left(1 + \frac{1}{t_2^2}\right) = \left(\frac{1}{t_1} + \frac{1}{t_2}\right)\left(\frac{1}{t_2} + \frac{1}{t_3}\right)`

102. The diagram is given below:

   .. image:: _static/images/18_16.png
      :alt: Problem 102
      :align: center

   Let the medians be :math:`AD, BE` and :math:`CF` meet at :math:`O.` From question,

   :math:`\angle BOC=\alpha, \angle COA = \beta, \angle AOB = \gamma`

   Let :math:`AD = p_1, BE=p_2, CF = p_3`

   :math:`AO:OD = 2:1 \Rightarrow AO = \frac{2}{3}p_1`

   Similalrly, :math:`OB = \frac{2}{3}p_2, OC = \frac{2}{3}p_3`

   Applying cosine rule in :math:`\triangle AOC,`

   :math:`\cos\beta = \frac{OA^2 + OC^2 - AC^2}{2.OA.OC} = \frac{\frac{4}{9}p_1^2 + \frac{4}{9}p_3^2 -
   b^2}{2.\frac{2}{3}p_1\frac{2}{3}p_3}`

   :math:`\cos\beta = \frac{4p_1^2 + 4p_3^2 - 9b^2}{8p_1p_3}`

   :math:`\Delta AOC = \frac{1}{2}.OA.OC.\sin\beta`

   :math:`\frac{1}{3}\Delta = \frac{1}{2}\frac{2}{3}p_1\frac{2}{3}p_3\sin\beta` where :math:`\Delta` is area of triangle :math:`ABC.`

   :math:`\sin\beta = \frac{3\Delta}{2p_1p_3}`

   :math:`\Rightarrow \cos\beta = \frac{4p_1^2 + 4p_3^2 - 9b^2}{12\Delta}`

   :math:`\because AD` is mean of :math:`\triangle ABC`

   :math:`\therefore AB^2 + AC^2 = 2BD^2 + 2AD^2`

   :math:`\Rightarrow b^2 + c^2 = 2\frac{a^2}{4} + 2p_1^2`

   :math:`p_1^2 = \frac{2b^2 + 2c^2 - a^2}{4}`

   Similarly, :math:`p_2^2 = \frac{2c^2 + 2a^2 - b^2}{4}`

   and :math:`p_3^2 = \frac{2a^2 + 2b^2 - c^2}{4}`

   :math:`\Rightarrow \cos\beta = \frac{(2b^2 + 2c^2 - a^2) + (2a^2 + 2b^2 - c^2) - 9b^2}{12\Delta}`

   :math:`= \frac{a^2 + c^2 - 5b^2}{12\Delta}`

   Similarly, :math:`\cos\alpha = \frac{b^2 + c^2 - 5a^2}{12\Delta}`

   Similarly, :math:`\cos\gamma = \frac{a^2 + b^2 - 5c^2}{12\Delta}`

   :math:`\cos\alpha + \cos\beta + \cos\gamma = \frac{-3(a^2 + b^2 + c^2)}{12\Delta}`

   :math:`= -\frac{a^2 + b^2 + c^2}{4\Delta}`

   :math:`\cot A + \cot B + \cot C = \frac{b^2 + c^2 - a^2}{2bc\sin A} + \frac{c^2 + a^2 - b^2}{2ca\sin B} + \frac{a^2 + b^2 -
   c^2}{2ab\sin C}`

   :math:`= \frac{a^2 + b^2 + c^2}{4\Delta}`

   :math:`\Rightarrow \cot\alpha + \cot\beta + \cot\gamma + \cot A + \cot B + \cot C = 0`

103. The diagram is given below:

    .. image:: _static/images/18_17.png
       :alt: Problem 103
       :align: center

   Let :math:`AD` be the perpendicular from :math:`A` on :math:`BC.` When :math:`AD` is extended it meets the circumscrbing circle
   at :math:`E.` Given, :math:`DE=\alpha.`

   Since angles in the same segment are equal, :math:`\therefore \angle AEB = \angle ACB = \angle C`

   and :math:`\angle AEC = \angle ABC = \angle B`

   From right angled :math:`\triangle BDE, \tan C = \frac{BD}{DE}`

   From right angled :math:`\triangle CDE, \tan B = \frac{CD}{DE}`

   :math:`\tan B + \tan C = \frac{a}{\alpha}`

   Similarly, :math:`\tan C + \tan A = \frac{b}{\beta}`

   and :math:`\tan A + \tan B = \frac{c}{\gamma}`

   Adding, we get

   :math:`\frac{a}{\alpha} + \frac{b}{\beta} + \frac{c}{\gamma} = 2(\tan A + \tan B + \tan C)`

104. The diagram is given below:

    .. image:: _static/images/18_18.png
       :alt: Problem 104
       :align: center

    Let :math:`H` be the orthocenter of triangle :math:`ABC.`

    From question, :math:`HA = p, HB = q, HC = r.`

    From figure, :math:`\angle HBD = \angle EBC = 90^\circ - C`

    :math:`\angle HCD = \angle FCB = 90^\circ - B`

    :math:`\therefore \angle BHC = 180^\circ - (\angle HBD + \angle HCD)`

    :math:`= 180^\circ - [90^\circ - C + 90^\circ - B] = B + C = \pi - A`

    Similarly, :math:`\angle AHC = \pi - B` and :math:`\angle AHB = \pi - C`

    Now :math:`\Delta BHC + \Delta CHA + \Delta AHB = \Delta ABC`

    :math:`\Rightarrow \frac{1}{2}[qr\sin BHC + rp\sin CHA + pq \sin AHB] = \Delta`

    :math:`\Rightarrow \frac{1}{2}[qr\sin A + rp\sin B + pq\sin C] = \Delta`

    :math:`\Rightarrow aqr + brp + cpq = abc`

105. The diagram is given below:

     .. image:: _static/images/18_19.png
        :alt: Problem 105
        :align: center

     Let :math:`O` be the center of unit circle and :math:`A` be the center of circle whose arc :math:`BPC` divides the unit circle
     in two equal parts.

     i.e area of the curve :math:`ABPCA = \frac{1}{2}` area of the unit circle :math:`= \frac{\pi}{2}`

     Let the radius of this new circle be :math:`r.`

     Then, :math:`AC = AB = AP = r`

     :math:`\because OB = OC = 1 \therefore \angle OCA = \angle OAC = \theta`

     Applying sine rule in :math:`\triangle AOC,`

     :math:`\frac{r}{\sin(\pi -2\theta)} = \frac{1}{\sin\theta}`

     :math:`r = 2\cos\theta`

     Now area of :math:`ABPCA = 2[` Are of sector :math:`ACP +` Area of sector :math:`OAC -` Are of :math:`\triangle OAC]`

     :math:`= 2\left[\frac{1}{2}r^2\theta + \frac{1}{2}1^2(\pi - 2\theta) - \frac{1}{2}\sin(\pi -2\theta)\right]`

     :math:`=\theta. 4\cos^2\theta + \pi - 2\theta - \sin2\theta [\because r = 2\cos\theta]`

     :math:`= 2\theta\cos2\theta - \sin2\theta + \pi`

     :math:`\Rightarrow \frac{\pi}{2} = 2\theta\cos2\theta - \sin2\theta + \pi`

     :math:`\Rightarrow \frac{\pi}{2} = \sin2\theta - 2\theta\cos2\theta`

106. The diagram is given below:

     .. image:: _static/images/18_20.png
        :alt: Problem 106
        :align: center

     Let :math:`EF` be the perpendicular bisector of :math:`BC` and :math:`O` the center of the square. From question,

     Let :math:`BF = FC = a \Rightarrow BC = EF = 2a` and :math:`OE=OF = a`

     Let :math:`OP = x \Rightarrow OQ = x`

     :math:`\Rightarrow PF = a - x, QF = a + x`

     From right angled :math:`\triangle BPF,`

     :math:`\tan B = \frac{PF}{BF} = \frac{a - x}{x}`

     From right angled :math:`\triangle QFC,`

     :math:`\tan C = \frac{a + x}{a}`

     :math:`\Rightarrow (\tan B - \tan C)^2 = \frac{4x^2}{a^2}`

     In triangle :math:`ABC,`

     :math:`\tan A = \tan[\pi - (B + C)] = -\tan(B + C) = -\frac{2a^2}{x^2}`

     :math:`\Rightarrow \tan A(\tan B - \tan C)^2 + 8 = 0`

107. The diagram is given below:

     .. image:: _static/images/18_21.png
        :alt: Problem 107
        :align: center

     :math:`\because CD` is internal bisector of :math:`\angle C`

     :math:`\therefore \frac{AD}{DB} = \frac{b}{a}`

     :math:`\Rightarrow BD = \frac{ac}{a + b}`

     Since angles of the same segment are equal.

     :math:`\therefore \angle ABE = \angle ACE = \frac{C}{2}`

     and :math:`\angle BEC = \angle BAC = A`

     Applying sine rule in :math:`\triangle BEC,`

     :math:`\frac{CE}{\sin CBE} = \frac{BC}{\sin BEC} \Rightarrow CE = \frac{a\sin\left(a + \frac{C}{2}\right)}{\sin A}`

     Applying sine rule in :math:`\triangle BDE,`

     :math:`\frac{DE}{\sin\frac{C}{2}} = \frac{BD}{\sin A}\Rightarrow DE = \frac{ac\sin\frac{C}{2}}{(a + b)\sin A}`

     :math:`\Rightarrow \frac{CE}{DE} = \frac{a\sin\left(B + \frac{C}{2}\right)}{ac\sin\frac{C}{2}}(a + b)`

     :math:`\Rightarrow \frac{CE}{DE} = \frac{(a + b)\sin\left(B + \frac{C}{2}\right)}{c\sin \frac{C}{2}}`

     Now, :math:`\frac{\sin\left(B + \frac{C}{2}\right)}{\sin\frac{C}{2}} = \frac{\sin\left(B +
     \frac{C}{2}\right).2\cos\frac{C}{2}}{2\sin\frac{C}{2}\cos\frac{C}{2}}`

     :math:`= \frac{\sin(B + C)+ \sin B}{\sin C} = \frac{\sin A + \sin B}{\sin C} = \frac{a + b}{c}`

     Thus, :math:`\frac{CE}{DE} = \frac{(a + b)^2}{c^2}`

108. The diagram is given below:

     .. image:: _static/images/20_1.png
        :alt: Problem 108
        :align: center

     :math:`\because AD` is the interna; bisector of angle :math:`A,`

     :math:`\frac{BD}{DC} = \frac{BA}{AC} = \frac{c}{b}`

     :math:`\Rightarrow \frac{BD}{c} = \frac{DC}{b} = \frac{BD + DC}{b + c}`

     :math:`\Rightarrow \frac{BD}{c} = \frac{a}{b + c}`

     Similarly, :math:`\frac{BF}{a} = \frac{c}{a + b}`

     Now :math:`\frac{\Delta BDF}{\Delta ABC} = \frac{BD.BF.\sin B}{a.c.\sin B} = \frac{ac}{(a + b)(b + c)}`

     Similarly, :math:`\frac{\Delta CDE}{\Delta ABC} = \frac{ab}{(a + c)(b + c)}`

     and :math:`\frac{\Delta AEF}{\Delta ABC} = \frac{bc}{(a + b)(a + c)}`

     :math:`\therefore \frac{\Delta DEF}{\Delta ABC} = \frac{\Delta ABC - (\Delta BDF + \Delta CDE + \Delta AEF)}{\Delta ABC}`

     :math:`= 1 - \frac{ac}{(a + b)(b + c)} - \frac{ab}{(a + c)(b + c)} - \frac{bc}{(a + b)(a + c)}`

     :math:`= \frac{2abc}{(a + b)(b + c)(c + a)}`

     :math:`\Delta DEF = \frac{2.\Delta .abc}{(a + b)(b + c)(c + a)}`

109. The diagram is given below:

     .. image:: _static/images/20_2.png
        :alt: Problem 109
        :align: center

     :math:`\because A + B + C = \pi \Rightarrow 3\alpha + 3\beta + 3\gamma = \pi \Rightarrow \alpha + \beta + \gamma =
     \frac{\pi}{3}`

     Clearly, :math:`\angle ADB = 60^\circ`

     Applying sine rule in :math:`\triangle ADB,`

     :math:`\frac{AR}{\sin\beta} = \frac{c}{\sin[\pi - (\alpha + \beta)]}`

     :math:`AR = \frac{c\sin \beta}{\sin(\alpha + \beta)} = \frac{2R\sin C\sin\beta}{\sin(\alpha + \beta)}`

     :math:`= \frac{2R\sin3\gamma\sin\beta}{\sin(60^\circ - \gamma)}`

     :math:`= \frac{2R(3\sin\gamma - 4\sin^3\gamma)\sin\beta}{\sin(60^\circ - \gamma)}.\frac{\cos(30^\circ -
     \gamma)}{cos(30^\circ - \gamma}`

     :math:`= \frac{4R\sin\beta\sin\gamma.(3 - 4\sin^2\gamma).\cos(30^\circ - \gamma)}{\sin(09^\circ - 2\gamma) + \sin 30^\circ}`

     :math:`= \frac{4R\sin\beta\sin\gamma\cos(30^\circ - \gamma)(3 - 4\sin^2\gamma)}{\cos2\gamma + \frac{1}{2}}`

     :math:`= \frac{8R\sin\beta\sin\gamma\cos(30^\circ - \gamma)(3 - 4\sin^2\gamma)}{2\cos2\gamma + 1}`

     :math:`= \frac{8R\sin\beta\sin\gamma\cos(30^\circ - \gamma)(3 - 4\sin^2\gamma)}{2(1 - 2\sin^2\gamma) + 1}`

     :math:`= 8R\sin\beta\sin\gamma\cos(30^\circ - \gamma)`
