Properties of Triangles' Solutions Part 1
*****************************************
1. Let :math:`a = 8` cm, :math:`b = 10` cm and :math:`c = 12` cm. So the smallest angle will be :math:`A` and greatest angle will
   be :math:`C.` So from cosine rule,

   :math:`\cos A = \frac{b^2 + c^2 - a^2}{2bc} = \frac{100 + 144 - 64}{2.10.12} = \frac{3}{4}`

   :math:`\cos C = \frac{a^2 + b^2 - c^2}{2ab} = \frac{64 + 100 - 144}{2.8.10} = \frac{1}{8}`

   :math:`\cos 2A = 2\cos^2A - 1 = 2.\frac{9}{16} - 1 = \frac{1}{8} = \cos C`

   Thus, we see that greatest angle is double to that of smallest angle.

#. Let :math:`\frac{b + c}{11} = \frac{c + a}{12} = \frac{a + b}{13}, = k`

   :math:`\therefore b + c = 11k, c + a = 12k, a + b = 13k \Rightarrow a + b + c = 18k`

   :math:`\therefore a = 7k, b = 6k, c = 5k`

   :math:`\frac{\cos A}{7} = \frac{b^2 + c^2 - a^2}{2bc} = \frac{36k^2 + 25k^2 - 49k^2}{2.6.7.7k^2} = \frac{1}{35}`

   :math:`\frac{\cos B}{19} = \frac{c^2 + a^2 - b^2}{2ca} = \frac{25k^2 + 49k^2 - 36k^2}{2.5.7.19.k^2} = \frac{1}{35}`

   :math:`\frac{\cos C}{25} = \frac{a^2 + b^2 - c^2}{2ab} = \frac{49k^2 + 36k^2 - 25k^2}{2.7.6.25.k^2} = \frac{1}{35}`

#. Given, :math:`\Delta = a^2 - (b - c)^2 \Rightarrow \Delta = a^2 - b^2 - c^2 + 2bc`

   :math:`\Rightarrow b^2 + c ^2 - a^2 = 2bc - \Delta \Rightarrow 2bc\cos A = 2bc - \frac{1}{2}bc\sin A`

   :math:`\Rightarrow 4\cos A + \sin A = 4 \Rightarrow 4\left(1 - 2\sin^2\frac{A}{2}\right) + 2\sin\frac{A}{2}\cos\frac{A}{2} = 4`

   :math:`2\sin\frac{A}{2}\left(\cos\frac{A}{2} - 4\sin\frac{A}{2}\right) = 0`

   :math:`\Rightarrow` either :math:`\sin\frac{A}{2} = 0` or :math:`\cos\frac{A}{2} - 4\sin\frac{A}{2} = 0`

   :math:`A = 0` is not possible. :math:`\therefore \tan\frac{A}{2} = \frac{1}{4}`

   :math:`\tan A = \frac{2\tan\frac{A}{2}}{1 - \tan^2\frac{A}{2}} = \frac{8}{15}.`

#. Since :math:`A, B, C` are in A.P. :math:`\therefore 2B = A + C`

   :math:`\because A + B + C = 180^\circ \Rightarrow B = 60^\circ`

   :math:`\cos B = \frac{c^2 + a^2 - b^2}{2ca} \Rightarrow \frac{1}{2} = \frac{c^2 + a^2 - b^2}{2ac} \Rightarrow a^2 - ac + c^2 =
   b^2`

   :math:`\Rightarrow \frac{a + c}{\sqrt{a^2 - ac + a^2}} = \frac{a + c}{b}`

   :math:`= \frac{k(\sin A + \sin C)}{k\sin B} = \frac{2\sin\frac{A + C}{2}\cos\frac{A - C}{2}}{\sin B}`

   :math:`= \frac{2\sin B\cos \frac{A - C}{2}}{\sin B} = 2\cos\frac{A - C}{2}`

#. :math:`\Delta = \frac{1}{2}.a.p_1 \therefore \frac{1}{p_1} = \frac{a}{\Delta}`

   Similarly, :math:`\frac{1}{p_2} = \frac{b}{\Delta}, \frac{1}{p_3} = \frac{c}{\Delta}`

   L.H.S. :math:`= \frac{a + b - c}{2\Delta} = \frac{(a + b)^2 - c^2}{2\Delta(a + b + c)}`

   :math:`= \frac{2ab + a^2 + b^2 - c^2}{2\Delta(a + b + c)} = \frac{2ab + 2ab\cos C}{2\Delta(a + b + c)}`

   :math:`= \frac{ab(1 + \cos C)}{\Delta(a + b + c)} = \frac{2ab\cos^2\frac{C}{2}}{\Delta(a + b + c)}`

#. :math:`\because :\tan\theta = \frac{2\sqrt{ab}}{a - b}\sin\frac{C}{2}`

   :math:`\Rightarrow (a - b)^2\tan^2\theta = 4ab\sin^2\frac{C}{2} \Rightarrow (a - b)^2(\sec^2\theta - 1) = 4ab\sin^2\frac{C}{2}`

   :math:`(a - b)^2\sec^2\theta = a^2b^2 -2ab\left(1 - 2\sin^2\frac{C}{2}\right)`

   :math:`(a - b)^2\sec^2\theta = a^2 + b^2 - 2ab\cos C = c^2[\because \cos C = \frac{a^2 + b^2 - c^2}{2ab}]`

   :math:`\Rightarrow c = (a - b)\sec\theta.`

#. :math:`\Delta ABC = \frac{1}{2}bc\sin A = \frac{1}{2}6.3.\sin C = 9\sin C`

   :math:`\tan^2\frac{A - B}{2} = \frac{1 - \cos(A - B)}{1 + \cos(A - B)} = \frac{1}{9}`

   :math:`\tan\frac{A - B}{2} = \pm\frac{1}{3}`

   :math:`\because 0 < \frac{A - B}{2} < 90^\circ \therefore \tan\frac{A - B}{2} = \frac{1}{3}`

   :math:`\tan\frac{A - B}{2} = \frac{a - b}{a + b}\cot\frac{C}{2} \Rightarrow \cot\frac{C}{2} = 1`

   :math:`\Rightarrow C = 90^\circ`

   Thus, required area :math:`= 8\sin90^\circ = 9`

#. The diagram is given below:

   .. image:: _static/images/18_1.png
      :alt: Problem 8
      :align: center

   From question, :math:`\angle A = 75^\circ, \angle C = 60^\circ \Rightarrow \angle B = 45^\circ`

   Also given, :math:`\frac{\Delta BAD}{\Delta BCD} = \sqrt{3} = \frac{c.x.\sin\theta}{a.x.\sin(45^\circ - \theta)}` where
   :math:`BD = x`

   :math:`\Rightarrow \frac{c\sin\theta}{a\sin(45^\circ - \theta)} = \sqrt{3}`

   :math:`\Rightarrow \frac{\sin C\sin\theta}{\sin A\sin(45^\circ - \theta)} = \sqrt{3}`

   :math:`\Rightarrow \frac{\frac{\sqrt{3}}{2}\sin\theta}{\frac{\sqrt{3} + 1}{2\sqrt{2}}\sin(45^\circ - \theta)} = \sqrt{3}`

   :math:`\Rightarrow \sqrt{2}\sin\theta = (\sqrt{3} + 1)\sin(45^\circ - \theta)`

   :math:`\Rightarrow \sqrt{2}\sin\theta = (\sqrt{3} + 1)\left(\frac{1}{\sqrt{2}}\cos\theta - \frac{1}{\sqrt{2}}\sin\theta\right)`

   :math:`\Rightarrow 2\sin\theta = (\sqrt{3} + 1)(\cos\theta - \sin\theta)`

   :math:`\tan\theta = \frac{1}{\sqrt{3}} \Rightarrow \theta = 30^\circ`

#. We find the largest angle which is opposite to side :math:`7,` if any angle can be obtuse angle then this one can.

   :math:`\cos \theta = \frac{3^2 + 5^2 - 7^2}{2.3.5} = -\frac{15}{30} = -\frac{1}{2}`

   :math:`\Rightarrow \theta = 120^\circ`

#. Given :math:`\angle A = 45^\circ, \angle B = 75^\circ \Rightarrow \angle = 60^\circ`

   We know that :math:`\frac{a}{\sin A} = \frac{b}{\sin B} = \frac{c}{\sin C} = k`

   :math:`a = \frac{1}{\sqrt{2}}k, b = \frac{\sqrt{3} + 1}{2\sqrt{2}}k, c = \frac{\sqrt{3}k}{2}`

   :math:`a + c\sqrt{2} = \frac{1}{\sqrt{\sqrt{2}}}k + \frac{\sqrt{3}}{\sqrt{2}}k = \frac{1 + \sqrt{3}}{\sqrt{2}}k`

   :math:`2b = \frac{\sqrt{3} + 1}{\sqrt{2}}`

   :math:`\Rightarrow a + \sqrt{2}c = 2b`

#. The diagram is given below:

   .. image:: _static/images/18_2.png
      :alt: Problem 11
      :align: center

   :math:`\Delta BCD + \Delta ACD = \Delta ABC`

   :math:`\Rightarrow \frac{1}{2}3CD\sin30^\circ + \frac{1}{2}4CD\sin60^\circ = \frac{1}{2}3.4`

   :math:`\frac{3}{4}CD + \sqrt{3}CD = 6 \Rightarrow CD = \frac{24}{3 + 4\sqrt{3}}`

#. The smallest angle will be opposite to smallest side i.e. :math:`4` cm. Similarly, greatest angle will be opposite to greatest
   side i.e. :math:`6` cm.

   Let :math:`a = 4` cm, :math:`b = 5` cm and :math:`c = 6` cm. Also, let opposite angles are :math:`A, B` and :math:`C.`

   :math:`\cos A = \frac{b^2 + c^2 - a^2}{2bc} = \frac{45}{60} = \frac{3}{4}`

   :math:`\cos C = \frac{a^2 + b^2 - c^2}{2ab} = \frac{5}{40} = \frac{1}{8}`

   :math:`\cos 2A = 2\cos^2A - 1 = 2.\frac{9}{16} - 1 = \frac{1}{8} = \cos C`

#. The diagram is given below:

   .. image:: _static/images/18_3.png
      :alt: Problem 13
      :align: center

   :math:`\angle A + \angle B + \angle C = 180^\circ = 10\angle B + \angle B + \angle B \Rightarrow \angle B = 15^\circ`

   :math:`\Rightarrow \angle A = 150^\circ`

   Let :math:`AB = AC = x`

   :math:`\therefore \cos 150^\circ = \frac{x^2 + x^2 - a^2}{2.x.x}`

   :math:`\Rightarrow -\sqrt{3}x^2 = 2x^2 - a^2 \Rightarrow x = \sqrt{\frac{1}{2 + \sqrt{3}}}a`

#. Let angles are :math:`A = 2k, B=3k, C=7k \therefore 2k + 3k + 7k = 180^\circ \Rightarrow k = 15^\circ`

   :math:`\frac{a}{\sin A} = \frac{b}{\sin B} = \frac{c}{\sin C} = l`

   :math:`\sin A = \frac{1}{2}, \sin B= \frac{1}{\sqrt{2}}, \sin C = \frac{\sqrt{2 + \sqrt{3}}}{2}`

   Now the ratios of sides can be proven.

#. Clearly, the sides are in the ratio of :math:`7:6:5`

   :math:`\therefore \cos A = \frac{6^2 + 5^2 - 7^2}{2.6.5} = \frac{1}{5}`

   :math:`\cos B = \frac{7^2 + 5^2 - 6^2}{2.7.5} = \frac{19}{35}`

   :math:`\cos C = \frac{7^2 + 6^2 - 5^2}{2.7.6} = \frac{5}{7}`

   :math:`\therefore \cos A:\cos B:\cos C = 7:19;25`

#. :math:`\tan \frac{C}{2} = \tan\frac{\pi - (A + B)}{2} = \cot\frac{A + B}{2} = \frac{1 -
   \tan\frac{A}{2}\tan\frac{B}{2}}{\tan\frac{A}{2} + \tan\frac{B}{2}}`

   :math:`= \frac{1 - \frac{5}{6}.\frac{20}{37}}{\frac{5}{6} + \frac{20}{37}}`

   :math:`= \frac{\frac{122}{222}}{\frac{305}{222}} = \frac{122}{305} = \frac{2}{5}`

   :math:`\sin A = \frac{2\tan\frac{A}{2}}{1 + \tan^2\frac{A}{2}} = \frac{2.\frac{5}{6}}{1 + \frac{25}{36}}`

   :math:`= \frac{60}{61}`

   :math:`\sin B = \frac{2\tan\frac{B}{2}}{1 + \tan^2\frac{B}{2}} = \frac{2.\frac{20}{37}}{1 + \frac{400}{1369}}`

   :math:`= \frac{1480}{1769}`

   :math:`\sin B = \frac{2\tan\frac{C}{2}}{1 + \tan^2\frac{C}{2}} = \frac{2\frac{2}{5}}{1 + \frac{4}{25}}`

   :math:`= \frac{20}{29}`

   :math:`a + c = k(\sin A + \sin C)[\frac{a}{\sin A} = \frac{b}{\sin B} = \frac{c}{\sin C} = k]`

   :math:`= k\left(\frac{60}{61} + \frac{20}{29}\right) = \frac{1740 + 1220}{1769} = \frac{2960}{1769} = 2b.`

#. It is much easier to prove this problem in reverse.

   Given, :math:`\frac{1}{a + c} + \frac{1}{b + c} = \frac{3}{a + b + c}`

   Upon solving :math:`a^2 + b^2 - c^2 = ab`

   :math:`\Rightarrow \frac{a^2 + b^2 - c^2}{2ab} = \frac{1}{2} = \cos60^\circ = \cos C`

#. Let the sides be :math:`a, b, c.` We know that :math:`\Delta = \frac{1}{2}a.\alpha` because area = :math:`\frac{1}{2}\times` base :math:`\times` altitude

   :math:`\Delta = \frac{1}{2}\alpha \Rightarrow \alpha = \frac{2\Delta}{a} \Rightarrow \frac{1}{\alpha} = \frac{a}{2\Delta}`

   :math:`\frac{1}{\alpha^2} + \frac{1}{\beta^2} + \frac{1}{\gamma^2} = \frac{a^2 + b^2 + c^2}{4\Delta^2}`

   :math:`\frac{\cot A + \cot B + \cot C}{\Delta} = \frac{\cos A}{\Delta\sin A} + \frac{\cos B}{\Delta\sin B} + \frac{\cos
   C}{\Delta\sin C}`

   :math:`\Delta = \frac{1}{2}bc\sin A \Rightarrow \sin A = \frac{2\Delta}{bc}`

   :math:`\therefore \frac{\cos A}{\Delta\sin A} = \frac{bc\cos A}{2\Delta^2} = \frac{b^2 + c^2 - a^2}{4\Delta^2}`

   :math:`\therefore \frac{\cos A}{\Delta\sin A} + \frac{\cos B}{\Delta\sin B} + \frac{\cos
   C}{\Delta\sin C} = \frac{a^2 + b^2 + c^2}{4\Delta^2}`

   Hence proven.

#. Given, :math:`\frac{a}{b} = 2 + \sqrt{3} = \tan75^\circ = \frac{\sin75^\circ}{\cos75^\circ}`

   :math:`\frac{\sin A}{\sin B} = \frac{\sin(90^\circ + 15^\circ)}{\sin(75^\circ - 15^\circ)}`

   :math:`\Rightarrow A = 105^\circ, B= 15^\circ` which satisfied :math:`A + B + C = 180^\circ`

#. :math:`\cos C = \frac{1}{2} = \frac{a^2 + b^2 - c^2}{2ab} \Rightarrow (1 + \sqrt{3}^2) + 4 - c^2 = 2(1 + \sqrt{3})`

   :math:`\Rightarrow c^2 = 6 \Rightarrow c = \sqrt{6}`

   :math:`\cos A = \frac{b^2 + c^2 - a^2}{2bc} = \frac{4 + 6 - (1 + \sqrt{3})^2}{4\sqrt{6}}`

   :math:`= \frac{6 + 2\sqrt{3}}{\sqrt{6}} = \sqrt{6} + \sqrt{2} \Rightarrow A = 75^\circ`

   Thus, :math:`\angle B = 45^\circ`

#. Greatest angle will be opposite to greatest side i.e. :math:`\sqrt{x^2 + xy + y^2}`

   :math:`\cos\theta = \frac{x^2 + y^2 - x^2 - xy - y^2}{2.x.y} = -\frac{1}{2} \Rightarrow \theta = 120^\circ`

#. Given sides are :math:`2x + 3, x^2 + 3x + 3` and :math:`x^2 + 2x.` Since lengths of sides is a positive quantity, therefore
   :math:`x^2 + 2x > 0 \Rightarrow x > 0`

   This leads to the fact that :math:`x^2 + 3x + 3` will be greatest side.

   :math:`\cos\theta = \frac{(2x + 3)^2 + (x^2 + 2x)^2 - (x^2 + 3x + 3)^2}{2(2x + 3)(x^2 + 2x)}`

   :math:`= \frac{4x^2 + 12x + 9 + x^4 + 4x^3 + 4x^2 - x^4 - 9x^2 - 9 - 6x^3 - 6x^2 - 18x}{4x^3 + 14x^2 + 12x}`

   :math:`= \frac{-2x^3 -7x^2 - 6x}{2(2x^3 + 7x^2 + 6x)} = -\frac{1}{2} = \cos120^\circ`

#. Given, :math:`3a = b + c.` We know that :math:`s = \frac{a + b + c}{2} \Rightarrow s = 2a`

   :math:`\cot\frac{B}{2}\cot\frac{C}{2} = \frac{s(s - b)}{\Delta}.\frac{s(s - c)}{\Delta}`

   :math:`=\frac{s^2(s - b)(s - c)}{s(s - a)(s - b)(s - c)} = \frac{s}{s - a} = 2`

#. We have to prove that :math:`a\sin\left(\frac{A}{2} + B\right) = (b + c)\sin\frac{A}{2}`

   :math:`\frac{b + c}{a} = \frac{k(\sin B + \sin C)}{\sin A}`

   :math:`= \frac{2\sin\frac{B + c}{2}\cos\frac{B - C}{2}}{2\sin\frac{A}{3}\cos\frac{A}{2}}`

   :math:`= \frac{\cos\left(\frac{B}{2} - \frac{C}{2}\right)}{\sin\frac{A}{2}}`

   :math:`= \frac{\cos\left[\frac{B}{2} - \left\{\frac{\pi}{2} - \left(\frac{A + B}{2}\right)\right\}\right]}{}\sin\frac{A}{2}`

   :math:`= \frac{\sin\left(\frac{A}{2} + B\right)}{\sin\frac{A}{2}}`

#. Numerator of L.H.S. :math:`= \frac{s(s - a)}{\Delta} + \frac{s(s - b)}{\Delta} + \frac{s(s - c)}{\Delta}`

   :math:`= \frac{s(s - a + s - b + s - c)}{\Delta} = \frac{s^2}{\Delta} = \frac{(a + b + c)^2}{4\Delta}`

   Denominator of R.H.S. :math:`= \frac{\cos A}{\sin A} + \frac{\cos B}{\sin B} + \frac{\cos C}{\sin C}`

   :math:`= \frac{b^2 + c^2 - a^2}{2bc\sin A} + \frac{c^2 + a^2 - b^2}{2ca\sin B} + \frac{a^2 + b^2 - c^2}{2ab\sin C}`

   [ :math:`\Delta = \frac{1}{2}bc\sin A = \frac{1}{2}ca\sin B = \frac{1}{2}ab\sin C` ]

   :math:`= \frac{a^2 + b^2 + c^2}{4\Delta}`

   L.H.S. :math:`= \frac{(a + b + c)^2}{a^2 + b^2 + c^2}`

#. First term of L.H.S. :math:`= \frac{b^2 - c^2}{a^2}\sin2A = \frac{b^2 - c^2}{a^2}2\sin A\cos A`

   :math:`= \frac{b^2 - c^2}{a^2}.2\frac{a}{K}.\frac{b^2 + c^2 - a^2}{2bc}`

   :math:`= \frac{1}{Kabc}[(b^2 - c^2)(b^2 + c^2 - a^2)] = \frac{1}{Kabc}[b^4 - c^4 -a^2(b^2 - c^2)]`

   Similarly, second term :math:`= \frac{1}{Kabc}[c^4 - a^4 - b^2(c^2 - a^2)]`

#. First term of L.H.S :math:`= a^3\cos(B - C) = a^2[a\cos(B - C)]`

   :math:`= Ra^2[2\sin A\cos(B - C)] = Ra^2[2\sin(B + C)\cos(B - C)] = Ra^2[\sin2B + \sin2C]`

   :math:`=Ra^2[2\sin B\cos B + 2\sin C\cos C] = a^2[b\cos B + c\cos C]`

   Similarly, second term :math:`= b^2[a\cos A + c\cos C]`

   and third term :math:`= c^2[a\cos A + b\cos B]`

   Adding, :math:`ab[a\cos B + b\cos A] + ca[c\cos A + a\cos C] + bc[b\cos C + c\cos B]`

   :math:`= 3abc =` R.H.S.

#. L.H.S. :math:`= \frac{\cos^2\frac{B - C}{2}}{K^2[\sin B + \sin C]^2} + \frac{\sin^2\frac{B - C}{2}}{K^2[\sin B - \sin C]^2}`

   :math:`= \frac{1}{K^2}\left(\frac{\cos^2\frac{B - C}{2}}{4\sin^2\frac{B + C}{2}\cos^2\frac{B - C}{2}} + \frac{\sin^\frac{B -
   C}{2}}{4\cos^2\frac{B + C}{2}\sin^2\frac{B - C}{2}}\right)`

   :math:`= \frac{1}{4k^2}\left(\frac{1}{\sin^2\frac{B + C}{2}} + \frac{1}{\cos^2\frac{B + C}{2}}\right)`

   :math:`= \frac{1}{4K^2}\left(\frac{1}{\cos^2\frac{A}{2}} + \frac{1}{\sin^2\frac{A}{2}}\right)`

   :math:`= \frac{1}{k^2}.\frac{1}{4\sin^2\frac{A}{2}\cos^2\frac{A}{2}} = \frac{1}{a^2}`

#. First term of L.H.S. :math:`= \frac{a}{\cos B\cos C} = \frac{2R\sin A}{\cos B\cos C}`

   :math:`= \frac{2R\sin(B + C)}{\cos B\cos C} = 2R(\tan B + \tan C)`

   Similarly, second term :math:`= 2R(\tan C + \tan A)` and third term :math:`= 2R(\tan A + \tan B)`

   L.H.S. :math:`= 4R[\tan A + \tan B + \tan C]`

   :math:`= 4R.\tan A\tan B\tan C[\because A + B + C = \pi \therefore \tan A + \tan B + \tan C = \tan A\tan B\tan C]`

   :math:`= 2.a\tan B\tan C\sec A =` R.H.S.

#. We have to prove that :math:`(b - c)\cos\frac{A}{2} = a\sin\frac{B - C}{2}`

   :math:`\frac{b - c}{a} = \frac{\sin B - \sin C}{\sin A} = \frac{2\cos\frac{B + C}{2}\sin \frac{B -
   C}{2}}{2\sin\frac{A}{2}\cos\frac{A}{2}}`

   :math:`= \frac{2\sin\frac{A}{2}\sin\frac{B - C}{2}}{2\sin\frac{A}{2}\cos\frac{A}{2}} = \frac{\sin\frac{B - C}{2}}{\cos\frac{A}{3}}`

#. We have to prove that :math:`\tan\left(\frac{A}{2} + B\right) = \frac{c + b}{c - b}\tan \frac{A}{2}`

   :math:`\frac{c + b}{c - b} = \frac{\sin C + \sin B}{\sin C - \sin B}`

   :math:`= \frac{2\sin\frac{B + C}{2}\cos\frac{C - B}{2}}{2\cos\frac{B + C}{2}\sin\frac{C - B}{2}}`

   :math:`= \frac{\tan\frac{B + C}{2}}{\tan\frac{C - B}{2}} = \frac{\cot\frac{A}{2}}{\tan\frac{\pi - B - A - B}{2}}`

   :math:`= \frac{\tan\left(\frac{A}{2} + B\right)}{\tan\frac{A}{3}}`

#. We have to prove that :math:`\tan\frac{A - B}{2} = \frac{a - b}{a + b}\cot\frac{C}{2}`

   :math:`\frac{a - b}{a + b} = \frac{\sin A - \sin B}{\sin A + \sin B} = \frac{2\cos\frac{A + B}{2}\sin\frac{A -
   B}{2}}{2\sin\frac{A + B}{2}\cos\frac{A - B}{2}}`

   :math:`= \frac{\tan\frac{A - B}{2}}{\tan \frac{A + B}{2}} = \frac{\tan\frac{A - B}{2}}{\cot\frac{C}{2}}`

#. L.H.S. :math:`= (b + c)\cos A + (c + a)\cos B + (a + b)\cos C`

   :math:`= (a\cos B + b\cos A) + (b\cos C + c\cos B) + (a\cos C + c\cos A)`

   :math:`= c + a + b =` R.H.S.

#. First term of L.H.S. :math:`= \frac{\cos^2B - \cos^2C}{b + c} = \frac{1}{k}\left[\frac{(\cos B + \cos C)(\cos B - \cos C)}{\sin
   B + \sin C}\right]`

   :math:`= \frac{1}{k}\left[\frac{2\cos\frac{B+C}{2}\cos\frac{B - C}{2}.2\sin\frac{B + C}{2}\sin\frac{C - B}{2}}{2\sin\frac{B +
   C}{2}\cos\frac{B - C}{3}}\right]`

   :math:`= \frac{1}{k}\left[2\cos\frac{B + C}{2}\sin\frac{C - B}{2}\right] = \frac{1}{k}[\sin C - \sin B]`

   Similarly second term :math:`= \frac{1}{k}[\sin A - \sin C]` and third term :math:`= \frac{1}{k}[\sin B - \sin A]`

   Thus, L.H.S. = R.H.S. = 0
