Transformation Formulae Solutions
*********************************
1. Given, :math:`\frac{\sin 75^\circ - \sin 15^\circ}{\cos 75^\circ + \cos 15^\circ}`

   :math:`= \frac{2\cos \frac{75^\circ + 15^\circ}{2}\sin \frac{75^\circ - 15^\circ}{2}}{2\cos \frac{75^\circ + 15^\circ}{2}\cos
   \frac{75^\circ - 15^\circ}{2}}`

   :math:`= \frac{2\cos 45^\circ\sin30^\circ}{2\cos45^\circ\cos30^\circ} = \tan30^\circ = \frac{1}{\sqrt{3}}`

2. Given, :math:`\frac{(\cos \theta - \cos 2\theta)(\sin 8\theta + \sin 2\theta)}{(\sin 5\theta - \sin\theta)(\cos
   4\theta - \cos 6\theta)} = \frac{2\sin2\theta\sin\theta.2\sin5\theta\cos3\theta}{2\cos3\theta\sin2\theta.2\sin5\theta\sin\theta}`

   :math:`= 1`

3. We have to prove, :math:`\frac{\sin7\theta - \sin5\theta}{\cos7\theta + \cos5\theta} = \tan\theta`

   L.H.S. :math:`= \frac{2\cos6\theta\sin\theta}{2\cos6\theta\cos\theta} = \tan\theta`

4. We have to prove, :math:`\frac{\cos6\theta - \cos4\theta}{\sin6\theta + \sin4\theta} = -\tan\theta`

   L.H.S. :math:`= \frac{2\sin5\theta\sin(-\theta)}{2\sin5\theta\cos\theta} = -\tan\theta`

5. We have to prove, :math:`\frac{\sin A + \sin 3A}{\cos A + \cos 3A} = \tan 2A`

   L.H.S. :math:`= \frac{2\sin2A\cos(-A)}{2\cos2A\cos(-A)} = \tan 2A`

6. We have to prove, :math:`\frac{\sin 7A - \sin A}{\sin 8A - \sin 2A} = \cos 4A\sec 5A`

   L.H.S. :math:`= \frac{2\cos4A\sin3A}{2\cos5A\sin3A} = \cos4A\sec5A`

7. We have to prove, :math:`\frac{\cos 2B + \cos 2A}{\cos 2B - \cos 2A} = \cot(A + B)\cot(A - B)`

   L.H.S. :math:`= \frac{2\cos(A + B)\cos(A - B)}{2\sin(A + B)\sin(A - B)} = \cot(A + B)\cot(A - B)`

8. We have to prove, :math:`\frac{\sin 2A + \sin 2B}{\sin 2A - \sin 2B} = \frac{\tan(A + B)}{\tan(A - B)}`

   L.H.S. :math:`= \frac{\2\sin(A + B)\cos(A - B)}{2\cos(A + B)\sin(A - B)}`

   :math:`= \frac{\tan(A + B)}{\tan(A - B)}`

9. We have to prove, :math:`\frac{\sin A + \sin 2A}{\cos A - \cos 2A} = \cot \frac{A}{2}`

   L.H.S. :math:`= \frac{2\sin\frac{3A}{2}\cos\frac{A}{2}}{2\sin\frac{3A}{2}\sin\frac{A}{2}}`

   :math:`= \cot\frac{A}{2}`

10. We have to prove, :math:`\frac{\sin 5A - \sin 3A}{\cos 3A + \cos 5A} = \tan A`

    L.H.S. :math:`= \frac{2\cos4A\sin A}{2\cos4A\cos A} = \tan A`

11. We have to prove, :math:`\frac{\cos 2B - \cos 2A}{\sin 2B + \sin 2A} = \tan(A - B)`

    L.H.S. :math:`= \frac{2\sin(A + B)\sin(A - B)}{2\sin(A + B)\cos(A - B)} = \tan(A - B)`

12. We have to prove, :math:`\cos (A + B) + \sin(A - B) = 2\sin(45^\circ + A)\cos(45^\circ + B)`

    L.H.S. :math:`= \cos A\cos B - \sin A\sin B + \sin A\cos B - \cos A\sin B`

    :math:`= (\sin A + \cos A)(\cos B - \sin B)`

    :math:`= 2(\frac{1}{\sqrt{2}}\sin A + \frac{1}{\sqrt{2}}\cos A)(\frac{1}{\sqrt{2}}\cos B - \frac{1}{\sqrt{2}}\sin B)`

    :math:`= 2(\sin A\cos 45^\circ + \sin 45^\circ\sin A)(\cos 45^\circ\cos B - \sin 45^\circ\sin B)`

    :math:`= 2\sin(45^\circ + A)\cos(45^\circ + B)`

13. We have to prove, :math:`\frac{\cos 3A - \cos A}{\sin 3A - \sin A} + \frac{\cos 2A - \cos 4A}{\sin 4A - \sin 2A} = \frac{\sin A}{\cos
    2A\cos 3A}`

    L.H.S. :math:`= \frac{-2\sin 2A\sin A}{2\cos 2A\sin A} + \frac{2\sin 3A\sin A}{2\cos 3A\sin A}`

    :math:`= \frac{-\sin 2A}{\cos 2A} + \frac{\sin 3A}{\cos 3A}`

    :math:`= \frac{\cos 2A\sin 3A - \sin 2A\cos 3A}{\cos 2A\cos 3A} = \frac{\sin(3A - 2A)}{\cos 2A\cos 3A}`

    :math:`= \frac{\sin A}{\cos 3A\cos 3A}`

14. Given, :math:`\frac{\sin (4A - 2B) + \sin (4B - 2A)}{\cos (4A - 2B) + \cos (4B - 2A)} = \tan(A + B)`
    L.H.S. :math:`= \frac{2\sin(A + B)\cos3(A - B)}{2\cos(A + B)\cos3(A - B)} = \tan(A + B)`

15. We have to prove, :math:`\frac{\tan 5\theta + \tan 3\theta}{\tan 5\theta - \tan 3\theta} = 4\cos 2\theta\cos 4\theta`

    L.H.S. :math:`= \frac{\frac{\sin5\theta}{\cos5\theta} + \frac{\sin4\theta}{\cos3\theta}}{\frac{\sin5\theta}{\cos5\theta} -
    \frac{\sin4\theta}{\cos3\theta}}`

    :math:`= \frac{\sin5\theta\cos3\theta + \sin3\theta\cos5\theta}{\sin5\theta\cos3\theta - \sin3\theta\cos5\theta}`

    :math:`= \frac{\sin8\theta}{\sin2\theta} = \frac{2\sin4\theta\cos\theta}{\sin2\theta}`

    :math:`= \frac{4\sin2\theta\cos2\theta\cos4\theta}{\sin2\theta} = 4\cos2\theta\cos4\theta`

16. We have to prove, :math:`\frac{\cos 3\theta + 2\cos5\theta + \cos 7\theta}{\cos\theta + 2\cos3\theta + \cos 5\theta} = \cos 2\theta - \sin
    2\theta\tan 3\theta`

    Adding first and last terms of numerator and denominator, we have

    L.H.S. :math:`= \frac{2\cos5\theta\cos2\theta + 2\cos5\theta}{2\cos3\theta\cos2\theta + 2\cos3\theta}`

    :math:`= \frac{\cos5\theta(\cos2\theta + 1)}{\cos3\theta(\cos2\theta + 1)}`

    :math:`= \frac{\cos3\theta\cos2\theta - \sin3\theta\sin2\theta}{\cos3\theta}`

    :math:`= \cos2\theta - \sin2\theta\tan3\theta`

17. We have to prove, :math:`\frac{\sin A + \sin 3A + \sin 5A + \sin 7A}{\cos A + \cos 3A + \cos 5A + \cos 7A} = \tan 4A`

    Pairing first and fourth term and second and third term in numerator and denominator, we get

    L.H.S. :math:`= \frac{2\sin4A\cos3A + 2\sin4A\cos A}{2\cos4A\cos3A + 2\cos4A\cos A}`

    :math:`= \frac{2\sin4A(\cos 3A + \cos A)}{2\cos4A(\cos 3A + \cos A)}`

    :math:`= \tan 4A`

18. We have to prove, :math:`\frac{\sin (\theta + \phi) - 2\sin\theta + \sin (\theta - \phi)}{\cos (\theta + \phi) - 2\cos \theta +
    \cos(\theta - \phi)} = \tan\theta`

    Pairing first and last term in both numerator and denominator, we get

    L.H.S. :math:`= \frac{2\sin\theta\cos\phi + 2\sin\theta}{2\cos\theta\cos\phi + 2\cos\theta}`

    :math:`= \frac{2\sin\theta(\cos\phi + 1)}{2\cos\theta(\cos\phi + 1)}`

    :math:`= \tan\theta`

19. We have to prove that, :math:`\frac{\sin A + 2\sin 3A + \sin 5A}{\sin 3A + 2\sin 5A + \sin 7A} = \frac{\sin 3A}{\sin 5A}`

    Pairing first and last term in both numerator and denominator, we get

    L.H.S. :math:`= \frac{2\sin3A\cos2A + 2\sin3A}{2\sin5A\cos2A + 2\sin5A}`

    :math:`= \frac{\sin3A(\cos 2A + 1)}{\sin5A(\cos 2A + 1)}`

    :math:`= \frac{\sin 3A}{\sin 5A}`

20. We have to prove that, :math:`\frac{\sin(A - C) + 2\sin A + \sin(A + C)}{\sin (B - C) + 2\sin B + \sin(B + C)} = \frac{\sin
    A}{\sin B}`
    Pairing first and last term in both numerator and denominator, we get

    L.H.S. :math:`= \frac{2\sin A\cos C + 2\sin A}{2\sin B\cos C + 2\sin B}`

    :math:`= \frac{\sin A(\cos C + 1)}{\sin B(\cos C + 1)}`

    :math:`= \frac{\sin A}{\sin B}`

21. We have to prove that, :math:`\frac{\sin A - \sin 5A + \sin 9A - \sin 13A}{\cos A - \cos 5A - \cos 9A + \cos 13 A} = \cot 4A`

    Pairing first and last term and second and third term in both numerator and denominator, we get

    L.H.S. :math:`= \frac{-2\cos7A\sin6A + 2\cos7A\sin 2A}{3\cos7A\cos6A - 2\cos7A\cos2A}`

    :math:`= \frac{2\cos7A(\sin 2A - \sin 6A)}{2\cos 7A(\cos 6A - \cos 2A)}`

    :math:`= \frac{-2\cos 4A\sin 2A}{-2\sin 4A\sin 2A}`

    :math:`= \cot 4A`

22. We have to prove that, :math:`\frac{\sin A + \sin B}{\sin A - \sin B} = \tan \frac{A + B}{2}\cot \frac{A - B}{2}`

    L.H.S. :math:`= \frac{2\sin\frac{A + B}{2}\cos\frac{A - B }{2}}{2\cos\frac{A + B}{2}\sin\frac{A - B}{2}}`

    :math:`= \tan \frac{A + B}{2}\cot \frac{A - B}{2}`

23. We have to prove that, :math:`\frac{\cos A + \cos B}{\cos B - \cos A} = \cot \frac{A + B}{2}\cot \frac{A - B}{2}`

    L.H.S. :math:`= \frac{2\cos\frac{A + B}{2}\cos\frac{A - B}{2}}{2\sin\frac{A + B}{2}\sin\frac{A - B}{2}}`

    :math:`= \cot\frac{A + B}{2}\cot\frac{A - B}{2}`

24. We have to prove that, :math:`\frac{\sin A + \sin B}{\cos A + \cos B} = \tan \frac{A + B}{2}`

    L.H.S. :math:`= \frac{2\sin\frac{A + B}{2}\cos\frac{A - B}{2}}{2\cos\frac{A + B}{2}\cos\frac{A - B}{2}}`

    :math:`= \tan \frac{A + B}{2}`

25. We have to prove that, :math:`\frac{\sin A - \sin B}{\cos B - \cos A} = \cot \frac{A + B}{2}`

    L.H.S. :math:`= \frac{2\cos\frac{A + B}{2}\sin\frac{A - B}{3}}{2\sin\frac{A + B}{2}\sin\frac{A - B}{2}}`

    :math:`= \cot \frac{A + B}{2}`

26. We have to prove that, :math:`\frac{\cos(A + B + C) + \cos(-A + B + C) + \cos(A - B + C) + \cos(A + B - C)}{\sin(A + B +
    C)+\sin(-A + B + C) - \sin(A - B + C) + \sin(A + B - C)} = \cot B`

    L.H.S. :math:`= \frac{2\cos(B + C)\cos A + 2\cos A\cos(B - C)}{2\sin(B + C)\cos A + 2\sin(B - C)\cos A}`

    :math:`= \frac{\cos(B + C) + \cos(B - C)}{\sin(B + C) + \sin(B - C)}`

    :math:`= \frac{2\cos B\cos C}{2\sin B\cos C} = \cot B`

27. We have to prove that, :math:`\cos 3A + \cos 5A + \cos 7A + \cos 15A = 4 \cos 4A\cos 5A \cos 6A`

    Adding first and last and two middle terms together, we gte

    L.H.S. :math:`= 2\cos9A\cos6A + 2\cos6A\cos A`

    :math:`= 2\cos6A(\cos9A + \cos A)`

    :math:`= 4\cos 4A \cos 5A \cos 6A`

28. We have to prove that, :math:`\cos(-A + B + C) + \cos(A - B + C) + \cos(A + B - C) + \cos(A + B + C) = 4\cos A\cos B\cos C`

    Adding first two and last two, we get

    L.H.S. :math:`= 2\cos C\cos (B - A) + 2\cos (A + B)\cos C`

    :math:`= 2\cos C(\cos (B - A) + \cos (A + B))`

    :math:`= 4\cos A\cos B\cos C`

29. We have to prove that, :math:`\sin 50^\circ - \sin 70^\circ + \sin 10^\circ = 0`

    L.H.S. :math:`= -2\cos 60^\circ \sin 10^\circ + \sin 10^\circ`

    :math:`= -\sin10^\circ + \sin10^\circ = 0`

30. We have to prove that, :math:`\sin 10^\circ + \sin 20^\circ + \sin 40^\circ + \sin 50^\circ = \sin 70^\circ + \sin 80^\circ`

    L.H.S. :math:`= \sin 10^\circ + \sin 50^\circ + \sin 20^\circ + \sin 40^\circ`

    :math:`= 2\sin 30^\circ \cos 20^\circ + 2\sin 30^\circ \cos 10^\circ`

    :math:`= 2\sin30^\circ(\cos 20^\circ + \cos 10^\circ)`

    :math:`= \sin 70^\circ + \sin 80^\circ[\because \cos\theta = \sin(90^\circ - \theta)]`

31. We have to prove that, :math:`\sin\alpha + \sin 2\alpha + \sin 4\alpha + \sin 5\alpha = 4\cos \frac{\alpha}{2}\cos
    \frac{3\alpha}{2}\sin 3\alpha`

    L.H.S. :math:`= \sin\alpha + \sin 5\alpha + \sin2\alpha + \sin4\alpha`

    :math:`= 2\sin3\alpha\cos2\alpha + 2\sin3\alpha\cos\alpha`

    :math:`= 2\sin3\alpha(\cos2\alpha + \cos\alpha)`

    :math:`= 4\cos \frac{\alpha}{2}\cos \frac{3\alpha}{2}\sin 3\alpha`

32. Given, :math:`\cos\left[\theta + \left(n - \frac{3}{2}\right)\phi\right] - \cos\left[\theta + \left(n +
    \frac{3}{2}\right)\phi\right]`

    :math:`= 2\sin\left[\theta + n\phi\right]\sin\left[\frac{\phi}{2}\right]`

33. Given, :math:`\sin\left[\theta + \left(n - \frac{3}{2}\right)\phi\right] + \sin\left[\theta + \left(n +
    \frac{3}{2}\right)\phi\right]`

    :math:`= 2\sin\left[\theta + n\phi\right]\cos\left[\frac{\phi}{2}\right]`

34. Given, :math:`2\sin5\theta\sin7\theta`

    Let the angles are :math:`A` and :math:`B` then :math:`\cos C - \cos D = 2\sin \frac{C + D}{2}\cos\frac{D - C}{2}`

    Thus, comparing, we get

    :math:`C + D = 14, D - C = 10`

    :math:`D = 12, C = 2`

    Thus, required expression is :math:`\cos 2\theta - \cos12\theta`

35. Given, :math:`2\cos7\theta\sin5\theta`

    :math:`= \sin 12\theta + \sin 2\theta`

36. Given, :math:`2\cos 11\theta\cos 3\theta`

    :math:`= \cos 14\theta + \cos 8\theta`

37. Given, :math:`2\sin54^\circ\sin66^\circ`

    :math:`=\cos12^\circ - \cos120^\circ`

38. We have to prove that :math:`\sin\frac{\theta}{2}\sin\frac{7\theta}{2} + \sin \frac{3\theta}{2}\sin\frac{11\theta}{2} =\sin
    2\theta\sin 5\theta`

    L.H.S. :math:`= \frac{1}{2}(\cos 3\theta - \cos 4\theta) + \frac{1}{2}(\cos 4\theta - \cos 7\theta)`

    :math:`= \sin2\theta + \sin5\theta`

39. We have to prove that, :math:`\cos 2\theta\cos \frac{\theta}{2} -\cos3\theta\cos\frac{9\theta}{2} =
    \sin5\theta\sin\frac{5\theta}{2}`

    L.H.S. :math:`= \frac{1}{2}\left(\cos\frac{5\theta}{2} + \cos \frac{3\theta}{2}\right) - \frac{1}{2}\left(\cos
    \frac{15\theta}{2} + \cos \frac{3\theta}{2}\right)`

    :math:`= \frac{1}{2}\left(2\sin 5\theta \sin \frac{5\theta}{2}\right)`

    :math:`= \sin5\theta\sin\frac{5\theta}{2}`

40. We have to prove that, :math:`\sin A\sin(A + 2B) - \sin B\sin(B + 2A) = \sin(A - B)\sin(A + B)`

    L.H.S. :math:`= \frac{1}{2}(2\sin A\sin(A + 2B) - 2\sin B\sin(B + 2A))`

    :math:`= \frac{1}{2}(\cos B - \cos(A + B) - \cos A - \cos (A + B))`

    :math:`= \frac{1}{2}2\sin(A - B)\sin(A + B)`

41. We have to prove that, :math:`(\sin 3A + \sin A)\sin A + (\cos 3A - \cos A)\cos A = 0`

    L.H.S. :math:`= 2\sin2A\cos A\sin A - 2\sin2A\sin A\cos A = 0`

42. We have to prove that, :math:`\frac{2\sin(A - C)\cos C - \sin(A - 2C)}{2\sin(B - C)\cos C - \sin(B - 2C)} = \frac{\sin A}{\sin
    B}`

    L.H.S. :math:`= \frac{\sin A + \sin(A - 2C) - \sin(A - 2C)}{\sin B + \sin(B - 2C) - \sin(B - 2C)}`

    :math:`= \frac{\sin A}{\sin B}`

43. We have to prove that, :math:`\frac{\sin A\sin 2A + \sin 3A\sin 6A + \sin4A\sin 13A}{\sin A\cos2A + \sin 3A\cos 6A + \sin
    4A\cos 13A} = \tan 9A`

    L.H.S. :math:`= \frac{\cos A - \cos 3A + \cos 3A - \cos 9A + \cos 9A - \cos 17A}{\sin 3A - \sin A + \sin 9A - \sin 3A + \sin 17A
    - \sin 9A}`

    :math:`= \frac{\cos A - \cos 17A}{\sin 17A - \sin A}`

    :math:`= \frac{2\sin 8A\sin 9A}{2\cos 9A\sin 8A} = \tan 9A`

44. We have to prove that, :math:`\frac{\cos 2A\cos 3A - \cos 2A\cos 7A + \cos A\cos 10A}{\sin 4A\sin 3A - \sin 2A\sin 5A + \sin
    4A\sin 7A} =\cot 6A\cot 5A`

    L.H.S. :math:`= \frac{\cos 5A + \cos A - \cos 9A - \cos 5A + \cos 11A + \cos 9A}{\cos A - \cos 7A - \cos 3A + cos 7A + \cos
    3A - \cos 11A}`

    :math:`= \frac{\cos A + \cos 11A}{\cos A - \cos 11A}`

    :math:`= \frac{\cos 6A\cos 5A}{\sin 6A\sin 5A} = \cot 6A\cot 5A`

45. We have to prove that, :math:`\cos(36^\circ - A)\cos(36^\circ + A) + \cos(54^\circ + A)\cos(54^\circ - A) = \cos 2A`

    L.H.S. :math:`= \frac{1}{2}(\cos (72^\circ)+ \cos 2A) + \frac{1}{2}(\cos 108^\circ + \cos 2A)`

    :math:`= \frac{1}{2}(\sin 18^\circ + - \sin 18^\circ + 2\cos 2A)[\because \sin 18^\circ = \cos(90^\circ - 18^\circ) = \cos
    72^\circ` and :math:`\cos 108^\circ = \cos(90^\circ + 18^\circ) = -\sin 18^\circ]`

    :math:`= \cos 2A`

46. We have to prove that :math:`\cos A\sin(B - C) + \cos B\sin(C - A) + \cos C\sin(A - B) = 0`

    L.H.S. :math:`= \frac{1}{2}[\sin(A + B - C) - \sin(A - B + C) + \sin(B + C - A) - \sin (B - C + A) + \sin(A - B + C) - \sin(C -
    A + B)] = 0`

47. :math:`\sin(45^\circ + A)\sin(45^\circ - A) = \frac{1}{2}\cos 2A`

    L.H.S. :math:`= \frac{1}{2}(2\sin(45^\circ + A)\sin(45^\circ - A)) = \frac{1}{2}[\cos 2A - \cos 90^\circ] = \frac{1}{2}\cos 2A`

48. We have to prove that, :math:`\sin(\beta - \gamma)\cos(\alpha - \delta) + \sin(\gamma - \alpha)\cos(\beta - \delta) +
    \sin(\alpha - \beta)\cos(\gamma - \delta) = 0`

    L.H.S. :math:`= \frac{1}{2}[\sin(\alpha + \beta - \gamma - \delta) + \sin(\beta + \delta - \gamma - \alpha) + \sin(\gamma
    -\alpha + \beta - \delta) + \sin(\gamma - \alpha - \beta + \delta) + \sin(\alpha - \beta + \gamma - \delta) - \sin(\alpha -
    \beta - \gamma + \delta)]`

    :math:`= 0`

49. We have to prove that, :math:`2\cos\frac{\pi}{13}\cos \frac{9\pi}{13} + \cos \frac{3\pi}{13} + \cos \frac{5\pi}{13} = 0`

    L.H.S. :math:`=\cos \frac{10\pi}{13} + \cos \frac{8\pi}{13} + \cos \left(\pi - \frac{10\pi}{13}\right) + \cos \left(\pi -
    \frac{8\pi}{13}\right)`

    :math:`= \cos \frac{10\pi}{13} + \cos \frac{8\pi}{13} - \cos \frac{10\pi}{13} - \cos \frac{8\pi}{13} = 0`

50. We have to prove that, :math:`\cos 55^\circ + \cos65^\circ + \cos 175^\circ = 0`

    L.H.S. :math:`= 2\cos 60^\circ\cos5^\circ + \cos(180^\circ - 5^\circ)`

    :math:`= 2.\frac{1}{2}.\cos5^\circ - \cos 5^\circ = 0`

51. We have to prove that, :math:`\cos 18^\circ -\sin 18^\circ = \sqrt{2}\sin 27^\circ`

    L.H.S. :math:`= \cos18^\circ - \cos(90^\circ - 72^\circ) = \cos 18^\circ - \cos 72^\circ`

    :math:`= 2\sin 45^\circ\sin 27^\circ = \sqrt{2}\sin27^\circ`

52. We have to prove that, :math:`\frac{\sin A + \sin 2A + \sin 4A + \sin 5A}{\cos A + \cos 2A + \cos 4A + \cos 5A} = \tan 3A`

    L.H.S. :math:`= \frac{(\sin 5A + \sin A) + (\sin 4A + \sin 2A)}{(\cos 5A + \cos A) + (\cos 4A + \cos 2A)}`

    :math:`= \frac{2\sin 3A\cos 2A + 2\sin 3A\cos A}{2\cos3A\cos2A + 2\cos 3A\cos A}`

    :math:`= \frac{\sin 3A(\cos 2A + \cos A)}{\cos 3A(\cos 2A + \cos A)} = \tan 3A`
