Trigonometrical Equations and their General Solutions Answers
*************************************************************
1. Given equation is :math:`\sin\theta = -1`

   :math:`\Rightarrow \sin\theta = \sin\left(-\frac{\pi}{2}\right)`

   :math:`\Rightarrow \theta = n\pi + (-1)^n\left(-\frac{\pi}{2}\right)`

   :math:`\theta = n\pi + (-1)^{n +1}\frac{\pi}{2}` where :math:`n\in I.`
2. Given equation is :math:`\cos\theta = -\frac{1}{2}`

   :math:`\cos\theta = \cos\frac{2\pi}{3} \Rightarrow \theta = 2n\pi \pm \frac{2\pi}{3}` where :math:`n\in I.`
3. Given equation is :math:`\tan\theta = -\sqrt{3}`

   :math:`\Rightarrow \tan\theta = \tan\left(-\frac{\pi}{3}\right) \Rightarrow \theta = n\pi + \left(-\frac{\pi}{3}\right)`

   :math:`= n\pi - \frac{\pi}{3}` where :math:`n\in I.`
4. Given equation is :math:`\sec\theta = -\sqrt{2}`

   :math:`\Rightarrow \sec\theta = \sec\frac{3\pi}{4}\Rightarrow \theta = 2n\pi\pm \frac{3\pi}{4}` where :math:`x\in I`
5. Given equation is :math:`\sin8\theta = \sin\theta \Rightarrow \sin9\theta - \sin\theta = 0`

   :math:`\Rightarrow 2\cos5\theta.\sin4\theta = 0`

   Either :math:`\cos5\theta = 0` or :math:`\sin4\theta = 0`

   :math:`\Rightarrow 5\theta = (2n + 1)\frac{\pi}{2}` or :math:`4\theta = n\pi`

   :math:`\theta = \frac{n\pi}{4}, (2n + 1)\frac{\pi}{10}` where :math:`n\in I.`
6. Given equation is :math:`\sin5x = \cos2x`

   :math:`\Rightarrow \cos2x = \cos\left(\frac{\pi}{2} - 5x\right)`

   :math:`2x = 2n\pi \pm \left(\frac{\pi}{2} - 5x\right)`

   :math:`x = (4n + 1)\frac{\pi}{14}, -(4n - 1)\frac{\pi}{6}` where :math:`n\in I`
7. Given equation is :math:`\sin3x = \sin x \Rightarrow \sin3x - \sin x= 0`

   :math:`\Rightarrow \cos2x.\sin x = 0`

   Either :math:`\cos2x = 0` or :math:`\sin x= 0`

   :math:`\Rightarrow 2x = (2n + 1)\frac{\pi}{2}` or :math:`x = n\pi`

   :math:`x = n\pi, (2n + 1)\frac{\pi}{4}` where :math:`n\in I`
8. Given equation is :math:`\sin3x = \cos2x \Rightarrow \cos2x = \cos\left(\frac{\pi}{2} - 3x\right)`

   :math:`\Rightarrow 2x = 2n\pi \pm \left(\frac{\pi}{2} - 3x\right)`

   :math:`x = \frac{2n\pi}{5} + \frac{\pi}{10}, -2n\pi + \frac{\pi}{2}`
9. Given equation is :math:`\sin ax + \cos bx = 0`

   :math:`\Rightarrow \sin ax + \sin\left(\frac{\pi}{2} - bx\right) = 0`

   :math:`\Rightarrow 2\sin\left(\frac{\pi}{4} + \frac{(a - b)x}{2}\right)\cos\left(\frac{(a + b)x}{2} - \frac{\pi}{4}\right) = 0`

   Either :math:`\Rightarrow \sin\left(\frac{\pi}{4} + \frac{(a - b)x}{2}\right) = 0` or :math:`\cos\left(\frac{(a + b)x}{2} -
   \frac{\pi}{4}\right) = 0`

   :math:`\Rightarrow \frac{\pi}{4} + \frac{(a - b)x}{2} = n\pi` or :math:`\frac{(a + b)x}{2} - \frac{\pi}{4} = (2n +
   1)\frac{\pi}{2}`

   :math:`x = \frac{2n\pi - \frac{\pi}{2}}{a - b}, \frac{(2n + 1)\pi + \frac{\pi}{2}}{a + b}`
10. Given :math:`\tan x\tan 4x =1 \Rightarrow \sin x\sin4x = \cos x\cos4x`

    :math:`\Rightarrow \cos x\cos4x - \sin x\sin 4x = 0`

    :math:`\cos 5x = 0 \Rightarrow 5x = (2n + 1)\frac{\pi}{2} \Rightarrow x = \frac{(2n + 1)\pi}{10}`
11. Given equation is :math:`\cos\theta = \sin105^\circ + \cos 105^\circ`

    :math:`\sin105^\circ = \sin(60^\circ + 45^\circ) = \frac{\sqrt{3} + 1}{2\sqrt{2}}`

    :math:`\cos105^\circ = \cos(60^\circ + 45^\circ) = \frac{1 - \sqrt{3}}{2\sqrt{2}}`

    :math:`\Rightarrow \cos\theta = \frac{1}{\sqrt{2}} \Rightarrow \theta = 2n\pi \pm \frac{\pi}{4}`
12. Given equation is :math:`7\cos^2\theta + 3\sin^2\theta = 4`

    :math:`\Rightarrow 4\cos^2\theta + 3 = 4 \Rightarrow \cos\theta = \pm \frac{1}{2}`

    If :math:`\cos\theta = \frac{1}{2}\Rightarrow \theta = 2n\pi\pm\frac{\pi}{3}`

    If :math:`\cos\theta = -\frac{1}{2}\Rightarrow \theta = 2n\pi\pm\frac{2\pi}{3}`
13. Given equation is :math:`3\tan(\theta - 15^\circ) = \tan(\theta + 15^\circ)`

    :math:`\Rightarrow \frac{\tan(\theta + 15^\circ)}{\tan(\theta - 15^\circ)} = \frac{3}{1}`

    Applying componendo and dividendo

    :math:`\Rightarrow \frac{\tan(\theta + 15^\circ) + \tan(\theta - 15^\circ)}{\tan(\theta + 15^\circ) - \tan(\theta - 15^\circ)}
    = \frac{4}{2}`

    :math:`\Rightarrow \frac{\sin(\theta + 15^\circ + \theta - 15^\circ)}{\sin(\theta + 15^\circ - \theta + 15^\circ)} = 2`

    :math:`\Rightarrow \sin2\theta = 2 \Rightarrow 2\theta = n\pi + (-1)^n\frac{\pi}{2} \Rightarrow \theta = \frac{n\pi}{2} +
    (-1)^n\frac{\pi}{4}`
14. Given equation is :math:`\tan x + \cot x = 2 \Rightarrow \tan^2x - 2\tan x + 1 = 0`

    :math:`\Rightarrow (\tan x - 1)^2 = 0 \Rightarrow \tan x = 1 \Rightarrow x = n\pi + \frac{\pi}{4}`
15. Given equation is :math:`\sin^2\theta = \sin^2\alpha \Rightarrow \sin\theta = \pm \sin\alpha`

    :math:`\theta = n\pi \pm\alpha`
16. Given equation is :math:`\tan^2x + \cot^2x = 2`

    :math:`\Rightarrow \tan^4x - 2\tan^2x + 1 = 0 \Rightarrow (\tan^2x - 1)^2 = 0`

    :math:`\tan x = \pm \Rightarrow x = n\pi \pm \frac{\pi}{4}`
17. Given equation is :math:`\tan^2x = 3\cosec^2x - 1`

    :math:`\Rightarrow \tan^2x = 2 + 3\cot^2x \Rightarrow \tan^4x -2\tan^2x - 3 = 0`

    :math:`\Rightarrow (\tan^2x + 1)(\tan^2x - 3) = 0`

    If :math:`\tan^2x + 1 = 0` then :math:`x` will become imaginary.

    :math:`\therefore \tan x = \pm\sqrt{3} \Rightarrow x = n\pi \pm \frac{\pi}{3}`
18. Given equation is :math:`2\sin^2x + \sin^22x = 2`

    :math:`\Rightarrow 2\sin^2x + 4\sin^2x\cos^2x = 2 \Rightarrow \sin^2x + 2\sin^2x(1 - \sin^2x) = 1`

    :math:`\Rightarrow (2\sin^2x - 1)(\sin^2x - 1) = 0`

    :math:`\Rightarrow \sin x = \pm\frac{1}{\sqrt{2}}` or :math:`\sin x = \pm 1`

    :math:`\Rightarrow x = n\pi \pm \frac{\pi}{4}, (2n + 1)\frac{\pi}{2}`
19. Given equation is :math:`7\cos^2 x + 3\sin^2 x = 4`

    :math:`\Rightarrow 4\cos^2 x + 3 = 4 \Rightarrow \cos x = \pm \frac{1}{2}`

    If :math:`\cos x = \frac{1}{2}\Rightarrow x = 2n\pi\pm\frac{\pi}{3}`

    If :math:`\cos x = -\frac{1}{2}\Rightarrow x = 2n\pi\pm\frac{2\pi}{3}`
20. Given equation is :math:`2\cos2x + \sqrt{2\sin x} = 2`

     :math:`\Rightarrow \sqrt{2\sin x} = 2(1 - \cos2x) = 4\sin^2x`

     :math:`\Rightarrow \sqrt{2\sin x}\left(1 - 2\sqrt{2}\sin^{\frac{3}{2}}x\right) = 0`

     Either:math:`\sin x = 0 \Rightarrow x = n\pi` where :math:`n\in I`

     or :math:`\sin^{\frac{3}{2}}x = \frac{1}{2\sqrt{2}} \Rightarrow \sin x = \frac{1}{2}`

     :math:`\Rightarrow x = n\pi + (-1)^n\frac{\pi}{6}`
21. We know that :math:`\tan^2\frac{x}{2} = \frac{1 - \cos x}{1 + \cos x}`

    :math:`\therefore 8\left(\frac{1 - \cos x}{1 + \cos x}\right) = 1 + sec x = \frac{1 + \cos x}{\cos x}`

    :math:`\Rightarrow 8\cos x - 8\cos^2x = (1 + \cos x)^2`

    :math:`\Rightarrow 9\cos^2x - 6\cos x + 1 = 0 \Rightarrow (3\cos x - 1)^2 = 0`

    :math:`\cos x = \frac{1}{3} \Rightarrow x = 2n\pi \pm \cos^{-1}\frac{1}{3}` where :math:`n in I.`

    Check :math:`\frac{x}{2}\neq (2n + 1)\frac{\pi}{2}` and :math:`\cos x \neq = 0` else equation will be meaningless.

    :math:`\Rightarrow x\neq (2n + 1)\pi` and :math:`x\neq (2n + 1)\frac{\pi}{2}`
22. Given equation is :math:`\cos x\cos2x\cos3x = \frac{1}{4}`

    :math:`\Rightarrow (2\cos x\cos3x)2\cos2x = 1 \Rightarrow 2\cos4x\cos2x + 2\cos^22x - 1 = 0`

    :math:`\Rightarrow \cos4x[2\cos2x + 1] = 0`

    If :math:`\cos4x = 0 \Rightarrow x = (2n + 1)\frac{\pi}{8}`

    If :math:`2\cos2x + 1 = 0 \Rightarrow 2x = 2n\pi \pm \frac{2\pi}{3}`

    :math:`x = n\pi \pm \frac{\pi}{3}`
23. Given equation is :math:`\tan x + \tan2x + \tan3x = 0`

    :math:`\Rightarrow \tan x +\tan2x + \frac{\tan x + \tan 2x}{1 - \tan x\tan 2x} = 0`

    :math:`\Rightarrow (\tan x + \tan 2x)\left(1 + \frac{1}{1 - \tan x\tan 2x}\right) = 0`

    If :math:`\tan x + \tan 2x = 0 \Rightarrow \tan x = -\tan 2x \Rightarrow x = n\pi -2x \Rightarrow x = \frac{n\pi}{3}`

    If :math:`1 + \frac{1}{1 - \tan x\tan 2x} = 0` then :math:`\tan x\tan 2x = 2`

    :math:`\frac{\tan^2x}{1 -\tan^2x} = 1 \Rightarrow \tan x = \pm\frac{1}{\sqrt{2}}`

    :math:`x = n\pi \pm\tan^{-1}\frac{1}{\sqrt{2}}`
24. Given equation is :math:`\cot x - \tan x - \cos x + \sin x = 0`

    :math:`\Rightarrow \frac{\cos^2x - \sin^2x}{\cos x\sin x} - (\cos x - \sin x) = 0`

    :math:`\Rightarrow (\cos x - \sin x)\left(\frac{\cos x + \sin x}{\cos x\sin x} - 1\right) = 0`

    If :math:`\cos x - \sin x = 0 \Rightarrow \tan x = 1\Rightarrow x = n\pi + \frac{\pi}{4}`

    If :math:`\frac{\cos x + \sin x}{\cos x\sin x} - 1= 0`

    :math:`\Rightarrow \cos x + \sin x = \cos x\sin x`

    Squaring, we get :math:`1 + \sin2x = \frac{1}{4}\sin^2x`

    :math:`\Rightarrow \sin2x = 2\pm 2\sqrt{2}`

    However, :math:`2 + 2\sqrt{2} > 1` which is not possible.

    :math:`\Rightarrow \sin 2x = 2 - 2\sqrt{2} = \sin\alpha` (let)

    :math:`x = \frac{n\pi}{2} + \frac{(-1)^n\alpha}{2}`
25. Given equation is :math:`2\sin^2x - 5\sin x\cos x - 8\cos^2x = -2`

    Clearly, :math:`\cos x \neq 0` else :math:`\sin^2x = -1` which is not possible.

    Therefore, we can divide both sides by :math:`\cos^2x` which yields

    :math:`2\tan^2x - 5\tan x -8 = -2\sec^2x`

    :math:`\Rightarrow 4\tan^2x - 5\tan x - 6 = 0`

    :math:`\Rightarrow (\tan x - 2)(4\tan x + 3) = 0`

    Thus, :math:`x = n\pi + \tan^{-1}2, b\pi + \tan^{-1}\left(\frac{-3}{4}\right)`

26. Given equation is :math:`(1 - \tan x)(1 + \sin2x) = 1 + \tan x`

    :math:`\Rightarrow (1 - \tan x)\left(1 + \frac{2\tan x}{1 + \tan^2x}\right) = 1 + \tan x`

    :math:`\Rightarrow (1 - \tan x)(1 + \tan x)^2 = (1 + \tan x)(1 + \tan^2x)`

    :math:`\Rightarrow (1 + \tan x)[(1 - \tan x)(1 + \tan x) - (1 + \tan^2x)] = 0`

    :math:`\Rightarrow (1 + \tan x)(-2\tan^2x) = 0`

    If :math:`\tan^2x = 0 \Rightarrow \tan x = 0\Rightarrow x = n\pi`

    If :math:`1 + \tan x = 0 \Rightarrow x = n\pi - \frac{\pi}{4}`

    where :math:`n \in I`

27. Given equation is :math:`2(\cos x + \cos2x) + \sin2x(1 + 2\cos x) = 2\sin x`

    :math:`\Rightarrow 4\cos\frac{3x}{2}\cos\frac{x}{2} + 2\sin\frac{5x}{2}\cos\frac{x}{2} - 2\sin\frac{x}{2}\cos\frac{x}{2} = 0`

    :math:`\Rightarrow 2\cos\frac{x}{2}\left[2\cos\frac{3x}{2} + \sin\frac{5x}{2} - \sin\frac{x}{2}\right] = 0`

    :math:`\Rightarrow 2\cos\frac{x}{2}\left[2\cos\frac{3x}{2} + 2\cos\frac{3x}{2}\sin x\right] = 0`

    :math:`\Rightarrow 4\cos\frac{x}{2}\cos\frac{3x}{2}[1 + \sin x] = 0`

    If :math:`\cos\frac{x}{2} = 0 \Rightarrow x = (2n + 1)\pi`

    If :math:`\cos\frac{3x}{2} = 0 \Rightarrow x = (2n + 1)\frac{\pi}{3}`

    If :math:`1 + \sin x = 0 \Rightarrow x = n\pi + (-1)^{n + 1}\frac{\pi}{2}`

    So the values in the given range are :math:`x = -\pi, -\frac{\pi}{2}, -\frac{\pi}{3}, \frac{\pi}{3}, \pi`

28. Given equation is :math:`4\cos^2x\sin x - 2\sin^2x = 3\sin x`

    :math:`\Rightarrow \sin x[4\cos^2x - 2\sin x - 3] = 0`

    :math:`\Rightarrow \sin x[4 - 4\sin^2x - 2\sin x - 3] = 0`

    :math:`\Rightarrow \sin x[4\sin^2x + 2\sin x - 1] = 0`

    If :math:`\sin x = 0 \Rightarrow x = n\pi`

    If :math:`4\sin^2x + 2\sin x - 1 = 0`

    :math:`\sin x = \frac{-1\pm\sqrt{5}}{4}`

    If :math:`\sin x = \frac{-1 + \sqrt{5}}{4} \Rightarrow \sin x = \sin\frac{\pi}{10} \Rightarrow x = n\pi + (-1)^n\frac{\pi}{10}`

    If :math:`\sin x = \frac{-1 - \sqrt{5}}{4}\Rightarrow \sin x = -\sin54^\circ = \sin\left(\frac{-3\pi}{10}\right)`

    :math:`\Rightarrow x = n\pi + (-1)^{n + 1}\frac{3\pi}{10}`

29. Given equation is :math:`2 + 7\tan^2x = 3.25\sec^2x`

    :math:`\Rightarrow 8 + 28\tan^2x = 13\sec^2x = 13 + 13\tan^2x`

    :math:`\Rightarrow 15\tan^2x = 5 \Rightarrow \tan x = \pm \frac{1}{\sqrt{3}}`

    :math:`\Rightarrow x = n\pi \pm \frac{\pi}{6}`

30. Given equation is :math:`\cos 2x + \cos 4x = 2\cos x`

    :math:`\Rightarrow \cos4x + \cos2x - 2\cos x = 0`

    :math:`\Rightarrow 2\cos3x\cos x - \cos x = 0`

    :math:`2\cos x[\cos 3x - 1] = 0`

    If :math:`\cos x = 0 \Rightarrow x = (2n + 1)\frac{\pi}{2}`

    If :math:`\cos 3x - 1 = 0\Rightarrow 3x = 2n\pi \Rightarrow x = \frac{2n\pi}{3}`

31. Given equation is :math:`3\tan x + \cot x = 5\cosec x`

    :math:`\Rightarrow \frac{3\sin x}{\cos x} + \frac{\cos x}{\sin x} = \frac{5}{\sin x}`

    :math:`\Rightarrow \sin x(3\sin^2x + \cos^2x) = 5\sin x\cos x`

    :math:`\Rightarrow \sin x(2\sin^2x - 5\cos x + 1) = 0`

    :math:`\Rightarrow \sin x(2\cos^2x + 5\cos x - 3) = 0`

    :math:`\Rightarrow \sin x(2\cos x + 3)(2\cos x - 1) = 0`

    :math:`\sin x\neq 0` because that will make :math:`\cosec x` and :math:`\cot x \infty.`

    :math:`2\cos x + 3 \neq 0` because :math:`-1\leq \cos x\leq 1`

    :math:`\therefore 2\cos x - 1 = 0\Rightarrow \cos x = \frac{1}{2} \Rightarrow x = 2n\pi \pm \frac{\pi}{3}`

32. Given equation is :math:`2\sin^2x = 3\cos x`

    :math:`\Rightarrow 2\cos^2x + 3\cos x - 2 = 0`

    :math:`\Rightarrow (2\cos x - 1)(\cos x + 2) = 0`

    :math:`\cos x \neq 2 \because -1\leq \cos x\leq 1`

    :math:`\therefore 2\cos x - 1 = 0\Rightarrow x = 2n\pi \pm \frac{\pi}{3}~\forall~n\in I`

    :math:`0\leq x \leq 2\pi \therefore x = \frac{\pi}{3}, \frac{5\pi}{3}`

33. Given equation is :math:`\sin^2x - \cos x = \frac{1}{4}`

    :math:`\Rightarrow 4\sin^2x - 4\cos x = 1 \Rightarrow 4 - 4\cos^2x - 4\cos x = 1`

    :math:`\Rightarrow 4\cos^2x + 4\cos x -3 = 0`

    :math:`\Rightarrow (2\cos x + 3)(2\cos x - 1) = 0`

    :math:`\cos x \neq 2 \because -1\leq \cos x\leq 1`

    :math:`\therefore 2\cos x - 1 = 0\Rightarrow x = 2n\pi \pm \frac{\pi}{3}~\forall~n\in I`

    :math:`0\leq x \leq 2\pi \therefore x = \frac{\pi}{3}, \frac{5\pi}{3}`

34. Given equation is :math:`3\tan^2x - 2\sin x = 0`

    :math:`\Rightarrow 3\sin^2x - 2\sin x\cos^2x = 0`

    :math:`\Rightarrow 3\sin^2x - 2\sin x + 2\sin^3x = 0`

    :math:`\Rightarrow \sin x(2\sin^2x + 3\sin x - 2) = 0`

    :math:`\Rightarrow \sin x(\sin x + 2)(2\sin x - 1) = 0`

    :math:`\sin x\neq -2 \because -1\leq \sin x\leq 1`

    If :math:`\sin x = 0 \Rightarrow x = n\pi`

    If :math:`2\sin x - 1 = 0 \Rightarrow x = n\pi + (-1)^n\frac{\pi}{6}`

35. Given equation is :math:`\sin x + \sin5x = \sin 3x`

    :math:`\Rightarrow \sin5x - \sin3x + \sin x = 0`

    :math:`\Rightarrow 2\cos4x\sin x + \sin x = 0`

    :math:`\sin x(2\cos 4x + 1) = 0`

    If :math:`\sin x = 0\Rightarrow x = n\pi~\forall~x\in I`

    If :math:`2\cos4x + 1 = 0 \Rightarrow 4x = 2n\pi \pm\frac{2\pi}{3}`

    :math:`x = \frac{n\pi}{2}\pm \frac{\pi}{6}~\forall~x\in I`

    Thus, :math:`x = 0, \pi` and :math:`x = \frac{\pi}{6}, \frac{\pi}{3}, \frac{2\pi}{3}, \frac{5\pi}{6}`

36. Given equation is :math:`\sin6x = \sin4x - \sin2x`

    :math:`\Rightarrow \sin6x + \sin2x - \sin4x = 0`

    :math:`\Rightarrow 2\sin4x\cos2x - \sin4x = 0`

    :math:`\Rightarrow \sin4x(2\cos2x - 1) = 0`

    If :math:`\sin4x = 0 \Rightarrow x = \frac{n\pi}{4}`

    If :math:`2\cos2x - 1 = 0 \Rightarrow \cos2x = \frac{1}{2}\Rightarrow 2x = 2n\pi \pm \frac{\pi}{3}`

    :math:`\Rightarrow x = n\pi \pm \frac{\pi}{6}`

37. Given equation is :math:`\cos6x + \cos 4x + \cos 2x + 1 = 0`

    :math:`\Rightarrow 2\cos5x\cos x + 2\cos^2x = 0`

    :math:`\Rightarrow 2\cos x(\cos5x + \cos x) = 0`

    :math:`\Rightarrow 4\cos x\cos2x\cos3x = 0`

    If :math:`\cos x = 0 \Rightarrow x = 2n\pi \pm\frac{\pi}{2}`

    If :math:`\cos2x = 0 \Rightarrow x = n\pi \pm \frac{\pi}{4}`

    If :math:`\cos3x = 0 \Rightarrow x = \frac{2n\pi}{3}\pm\frac{\pi}{6}`

38. Given equation is :math:`\cos x + \cos 2x + \cos 3x = 0`

    :math:`\Rightarrow (\cos x + \cos3x) + \cos 2x = 0`

    :math:`\Rightarrow 2\cos2x\cos x + \cos 2x = 0`

    :math:`\Rightarrow \cos2x(2\cos x + 1) = 0`

    If :math:`\cos 2x = 0 \Rightarrow x = (2n + 1)\frac{\pi}{4}`

    If :math:`2\cos x + 1 = 0 \Rightarrow x = 2n\pi\pm\frac{2\pi}{3}`

39. Given equation is :math:`\cos3x + \cos2x = \sin\frac{3x}{2} +  \sin\frac{x}{2}`

    :math:`\Rightarrow 2\cos\frac{5x}{2}\cos\frac{x}{2} - 2\sin x\cos\frac{x}{2} = 0`

    :math:`\Rightarrow 2\cos\frac{x}{2}\left[\cos\frac{5x}{2} - \sin x\right] = 0`

    If :math:`\cos\frac{x}{2} = 0 \Rightarrow \frac{x}{2} = \left(n + \frac{1}{2}\right)\pi`

    :math:`x = (2n + 1)\pi`

    If :math:`\cos\frac{5x}{2} = \sin x = \cos\left(\frac{\pi}{2} - x\right)`

    :math:`\Rightarrow \frac{5x}{2} = 2n\pi \pm \left(\frac{\pi}{2} - x\right)`

    :math:`\Rightarrow x = (4n + 1)\pi/7, (4n - 1)\pi/3`

    Thus, between :math:`0` and :math:`2\pi` the values of :math:`x` are :math:`\frac{\pi}{7}, \frac{5\pi}{7}, \pi, \frac{9\pi}{7},
    \frac{13\pi}{7}.`

40. Given equation is :math:`\tan x+ \tan2x + \tan3x = \tan x.\tan2x.\tan3x`

    :math:`\Rightarrow \tan x + \tan2x = \tan3x(\tan x\tan2x - 1)`

    :math:`\Rightarrow \frac{\tan x + \tan 2x}{1 - \tan x\tan2x} = -\tan3x`

    :math:`\Rightarrow \tan(x + 2x) = -\tan3x \Rightarrow 2\tan 3x = 0`

    :math:`\Rightarrow 3x = n\pi \Rightarrow x = \frac{n\pi}{3}`

41. Given equation is :math:`\tan x + \tan 2x + \tan x\tan 2x = 1`

    :math:`\Rightarrow \tan x + \tan2x = 1 - \tan x\tan 2x`

    :math:`\Rightarrow \frac{\tan x + \tan2x}{1 - \tan x\tan2x} = 1`

    :math:`\Rightarrow \tan 3x = \tan\frac{\pi}{4}`

    :math:`3x = n\pi + \frac{\pi}{4} \Rightarrow x = (4n + 1)\frac{\pi}{12}`

42. Given equation is :math:`\sin2x + \cos2x + \sin x + \cos x + 1 = 0`

    :math:`\Rightarrow 2\sin x\cos x + 2\cos^2x - 1 + \sin x + \cos x + 1 = 0`

    :math:`\Rightarrow \sin x(2\cos x + 1) + \cos x(2\cos x + 1) = 0`

    :math:`\Rightarrow (2\cos x + 1)(\sin x + \cos x) = 0`

    If :math:`\cos x = -\frac{1}{2} \Rightarrow x = 2n\pi\pm\frac{2\pi}{3}`

    If :math:`\sin x + \cos x = 0 \Rightarrow \tan x = -1 \Rightarrow x = n\pi - \frac{\pi}{4}`

43. We have to prove that :math:`\sin x + \sin 2x + \sin 3x = \cos x + \cos 2x + \cos 3x`

    :math:`\Rightarrow (\sin x + \sin 3x) + \sin 2x = (\cos x + \cos3x) + \cos 2x`

    :math:`\Rightarrow 2\sin2x\cos x + \sin 2x = 2\cos2x\cos x + \cos 2x`

    :math:`\Rightarrow \sin2x(2\cos x + 1) = \cos2x(2\cos x + 1)`

    :math:`\Rightarrow (2\cos x + 1)(\sin2x - \cos2x) = 0`

    If :math:`2\cos x + 1 = 0 \Rightarrow x = 2n\pi \pm \frac{2\pi}{3}`

    If :math:`\sin 2x - \cos2x = 0 \Rightarrow \tan2x = 1 = \tan\frac{\pi}{4} \Rightarrow x = \frac{n\pi}{2}+\frac{\pi}{8}`

44. Given equation is :math:`\cos6x + \cos4x = \sin3x + \sin x`

    :math:`\Rightarrow 2\cos5x\cos x = 2\sin2x\cos x`

    :math:`\Rightarrow \cos x(\cos5x - \sin2x) = 0`

    If :math:`x = 0 \Rightarrow x = 2n\pi\pm\frac{\pi}{2}`

    If :math:`\cos5x = \sin2x \Rightarrow \cos5x = \cos\left(\frac{\pi}{2} - 2x\right)`

    :math:`\Rightarrow 5x = 2n\pi\pm \left(\frac{\pi}{2} - 2x\right)`

    Taking +ve sign :math:`7x = 2n\pi + \frac{\pi}{2} \Rightarrow x = (4n + 1)\frac{\pi}{14}`

    Taling -ve sign :math:`3x = 2n\pi - \frac{\pi}{2} \Rightarrow x = (4n - 1)\frac{\pi}{6}`

45. Given equation is :math:`\sec4x - \sec2x = 2`

    :math:`\Rightarrow \cos2x - \cos4x = 2\cos2x\cos4x` where :math:`\cos2x, \cos4x\neq 0`

    :math:`\Rightarrow \cos2x - \cos4x = \cos6x + \cos 2x`

    :math:`\Rightarrow \cos6x + \cos4x = 0 \Rightarrow 2\cos5x\cos x = 0`

    If :math:`\cos 5x = 0 \Rightarrow 5x = 2n\pi\pm\frac{\pi}{2}\Rightarrow x = \frac{2n\pi}{5}\pm\frac{\pi}{10}`

    If :math:`\cos x = 0 \Rightarrow x = 2n\pi\pm\frac{\pi}{2}`

46. Given equation is :math:`\cos2x = (\sqrt{2} + 1)\left(\cos x - \frac{1}{\sqrt{2}}\right)`

    :math:`\Rightarrow (2\cos^2x - 1) = \frac{\sqrt{2} + 1}{\sqrt{2}}\left(\sqrt{2}\cos x - 1\right)`

    :math:`\Rightarrow (\sqrt{2}\cos x - 1)\left(\sqrt{2}\cos x + 1 - 1 - \frac{1}{\sqrt{2}}\right) = 0`

    :math:`\Rightarrow (\sqrt{2}\cos x - 1)(2\cos x - 1) = 0`

    If :math:`\sqrt{2}\cos x - 1 = 0 \Rightarrow x = 2n\pi \pm \frac{\pi}{4}`

    If :math:`2\cos x - 1 = 0 \Rightarrow x = 2n\pi\pm\frac{\pi}{3}`

47. Given equation is :math:`5\cos2x + 2\cos^2\frac{x}{2} + 1 = 0`

    :math:`\Rightarrow 10\cos^2x - 5 + \cos x + 2 = 0[\because \cos2x = 2\cos^2x - 1]`

    :math:`\Rightarrow 10\cos^2x + \cos x - 3 = 0`

    :math:`\Rightarrow (2\cos x -1)(5\cos x + 3) = 0`

    If :math:`\cos x = 1/2 \Rightarrow x = \frac{\pi}{3} [\because -\pi \leq x\leq \pi]`

    If :math:`5\cos x + 3 = 0 \Rightarrow x = \pi - \cos^{-1}\frac{3}{5}`

48. Given equation is :math:`\cot x - \tan x = sec x`

    :math:`\Rightarrow \cos x(\cos^2x - \sin^2x) = \sin x\cos x`

    :math:`\Rightarrow \cos x(2\sin^2x + \sin x - 1) = 0`

    :math:`\Rightarrow \cos x(2\sin x - 1)(\sin x + 1) = 0`

    :math:`\cos x\neq 0` and :math:`\sin \neq -1` because that will render original equation meaningless.

    :math:`\therefore 2\sin x - 1= 0 \Rightarrow x = n\pi + (-1)^n\frac{\pi}{6}`

49. Given equation is :math:`1 + \sec x = \cot^2\frac{x}{2}`

    :math:`\Rightarrow \frac{1 + \cos x}{\cos x} = \frac{\cos^2\frac{x}{2}}{\sin^2\frac{x}{2}}`

    :math:`\Rightarrow 2\sin^2\frac{x}{2}\cos^2\frac{x}{2} = \cos x\cos^2\frac{x}{2}`

    :math:`\Rightarrow \cos^2\frac{x}{2}\left(2\sin^2\frac{x}{2} - \cos x\right) = 0`

    :math:`\Rightarrow \cos^2\frac{x}{2}\left(1 - 2\cos x\right) = 0`

    If :math:`\cos\frac{x}{2} = 0 \Rightarrow \frac{x}{2} = n\pi + \frac{pi}{2} \Rightarrow x = (2n + 1)\pi`

    If :math:`1 - 2\cos x =  0\Rightarrow x = 2n\pi \pm \frac{\pi}{3}`

50. Given equation is :math:`\cos3x\cos^3x + \sin3x\sin^3x = 0`

    :math:`\Rightarrow (4\cos^3x - 3\cos x)\cos^3x + (3\sin x - 4\sin^3x)\sin^3x = 0`

    :math:`\Rightarrow 3(\sin^4x - \cos^4x) - 4(\sin^6x - \cos^6x) = 0`

    :math:`\Rightarrow 3(\sin^2x - \cos^2x) - 4(\sin^2x - \cos^2x)(\sin^4x + \cos^4x + \sin^2x\cos^2x) = 0`

    :math:`\Rightarrow \cos2x[-3 + 4\{\sin^2x(\sin^2x + \cos^2x) + \cos^4x\}] = 0`

    :math:`\Rightarrow \cos 2x[4\cos^4x - 4\cos^2x + 1] = 0`

    :math:`\Rightarrow \cos2x(2\cos^2x - 1)^2 = 0`

    :math:`\Rightarrow \cos^32x = 0`

    :math:`\Rightarrow \cos 2x = 0`

    :math:`2x = n\pi + \frac{\pi}{2} \Rightarrow x = (2n + 1)\frac{\pi}{4}`

51. Given equation is :math:`\sin^3x + \sin x\cos x + \cos^3x = 1`

    :math:`\Rightarrow \sin^3x + \cos^3x + \sin x\cos x - 1 = 0`

    :math:`\Rightarrow (\sin x + \cos x)(\sin^2x - \sin x\cos x + \cos^2x) + (\sin x\cos x - 1) = 0`

    :math:`\Rightarrow (1 - \sin x\cos x)(\sin x + \cos x - 1) = 0`

    If :math:`1 - \sin x\cos x = 0 \Rightarrow \sin 2x = 2` which is not possible.

    :math:`\therefore \sin x + \cos x - 1 = 0 \Rightarrow \frac{1}{\sqrt{2}}\sin x + \frac{1}{\sqrt{2}}\cos x = \frac{1}{\sqrt{2}}`

    :math:`\Rightarrow \cos\left(x - \frac{\pi}{4}\right) = \cos\frac{\pi}{4}`

    :math:`\Rightarrow x - \pi/4 = 2n\pi \pm \pi/4 = 2n\pi, 2n\pi + \pi/2`

52. Given equation is :math:`\sin 7x + \sin4x + \sin x = 0`

    :math:`\Rightarrow 2\sin4x\cos3x + \sin4x = 0`

    :math:`\Rightarrow \sin4x(2\cos3x + 1) = 0`

    If :math:`\sin4x = 0 \Rightarrow x = n\pi/4 \Rightarrow x = \pi/4~\forall 0\leq x\leq\pi/2`

    If :math:`\cos3x = -1/2 \Rightarrow x = \frac{2\pi}{9}, \frac{4\pi}{9}~\forall 0\leq x\leq\pi/2`

53. Given equation is :math:`\sin x + \sqrt{3}\cos x = \sqrt{2}`

    Dividing both sides by :math:`2` [we arrive at this no. by squaring and adding coefficients of :math:`\sin x` and :math:`\cos x`
    and then taking square root]

    :math:`\Rightarrow \frac{1}{2}\sin x + \frac{\sqrt{3}}{2}\cos x = \frac{1}{\sqrt{2}}`

    :math:`\Rightarrow \sin\frac{\pi}{6}\sin x + \cos\frac{\pi}{6}\cos x = \cos\frac{\pi}{4}`

    :math:`\Rightarrow \cos\left(x - \frac{\pi}{6}\right) = \cos\frac{\pi}{4}`

    :math:`\Rightarrow x - \frac{\pi}{6} = 2n\pi\pm\frac{\pi}{4}`

    :math:`\Rightarrow x = 2n\pi\pm\frac{5\pi}{12}, 2n\pi-\frac{\pi}{12}`

54. We have to find minimum value of :math:`27^{\cos2x}.81^{\sin2x}`

    :math:`27^{\cos2x}.81^{\sin2x} = 3^{3\cos2x + 4\sin2x}`

    It will be minimum when :math:`3\cos2x + 4\sin2x` will be minimum.

    Dividing and multiplying with :math:`5,` we get

    :math:`5\left(\frac{3}{5}\cos2x + \frac{4}{5}\sin2x\right)`

    :math:`\Rightarrow 5\cos(2x - y)` where :math:`\tan y = \frac{4}{3}`

    For minimum value :math:`\cos(2x - y) = -1 = \cos\pi \Rightarrow 2x - y = 2n\pi\pm\pi`

    :math:`x = \frac{2n\pi\pm\pi + \tan^{-1}\frac{4}{3}}{2}, n \in I`

    Minimum value will be :math:`3^{-5} = \frac{1}{243}`

55. Given :math:`3\cos 2x = 1 \Rightarrow \cos2x = \frac{1}{3}`

    :math:`\Rightarrow \tan^2x = \frac{1 - \cos2x}{1 + \cos2x} = \frac{1}{2}`

    Given :math:`32\tan^8x = 2\cos^2y - 3\cos y`

    :math:`\Rightarrow 32.\frac{1}{2^4} = 2\cos^2y - 3\cos y`

    :math:`\Rightarrow 2\cos^2y - 3\cos y - 2 = 0`

    :math:`(2\cos y + 1)(\cos y - 2) = 0`

    :math:`\because \cos y \neq 2 \Rightarrow 2\cos y + 1 = 0`

    :math:`\Rightarrow y = 2n\pi\pm\frac{2\pi}{3}`

56. Given equation is :math:`(1 - \tan x)(1 + \tan x)sec^2x + 2^{\tan^2x} = 0`

    :math:`\Rightarrow (1 - \tan^2x)(1 + \tan^2x) + 2^{\tan^2x} = 0`

    :math:`\Rightarrow 1 + 2^{\tan^2x} = \tan^4x`

    Clearly, :math:`\tan^2x = 3` is the solution of the above equation.

    :math:`\Rightarrow \tan x = \pm\sqrt{3} \Rightarrow x = n\pi\pm\frac{\pi}{3}`

    Values of :math:`x` in the given interval are :math:`\pm\frac{\pi}{3}.`

57. Given equation is :math:`e^{\cos x} = e^{-\cos x} + 4.`

    :math:`\Rightarrow e^{2\cos x} - 4e^{\cos x} - 1= 0`

    :math:`\Rightarrow e^{\cos x} = 2\pm\sqrt{5}`

    If :math:`e^{\cos x} = 2 + \sqrt{5}` then :math:`\cos x > 1` which is not possible.

    If :math:`e^{\cos x} = 2 - \sqrt{5}` then :math:`\cos x` is an imaginary number. Thus, no solutions for given equation are
    possible.

58. Given equation is :math:`(1 + \tan x)(1 + \tan y) = 2`

    :math:`\Rightarrow 1 + \tan x + \tan y + \tan x\tan y = 2`

    :math:`\Rightarrow \tan x + \tan y = 1 - \tan x\tan y`

    :math:`\Rightarrow \frac{\tan x + \tan y}{1 - \tan x\tan y} = 1`

    :math:`\Rightarrow \tan(x + y) = \tan\frac{\pi}{4}`

    :math:`\Rightarrow x + y = n\pi\pm\frac{\pi}{4}`

59. Given equation is :math:`\tan(\cot x) = \cot(\tan x)`

    :math:`\Rightarrow \tan(\cot x) = \tan\left(\frac{\pi}{2} - \tan x\right)`

    :math:`\Rightarrow \cot x = n\pi + \left(\frac{\pi}{2} - \tan x\right)`

    :math:`\Rightarrow \tan x + \cot x = n\pi + \frac{\pi}{2}`

    :math:`\Rightarrow \frac{\sin^2x + \cos^2x}{\sin x + \cos x} = (2n + 1)\pi/2`

    :math:`\Rightarrow \frac{1}{\sin2x} = (2n + 1)\pi/4 \Rightarrow \sin2x = \frac{4}{(2n + 1)\pi}`

60. We have :math:`a\tan z+ b\sec z = c`

    :math:`\Rightarrow c - a\tan z = b\sec z \Rightarrow (c - a\tan z)^2 = b^2sec^2z`

    :math:`\Rightarrow (a^2 - b^2)\tan^2x -2ac\tan z + (c^2 - b^2) = 0`

    Given that :math:`x` and :math:`y` are roots of original equation so :math:`\tan x` and :math:`\tan y` will be roots of last
    equation.

    :math:`\Rightarrow \tan x + \tan y = \frac{2ac}{a^2 - b^2}` and :math:`\tan x\tan y = \frac{c^2 - b^2}{a^2 - b^2}`

    :math:`\Rightarrow \tan(x + y) = \frac{\tan x + \tan y}{1 - \tan x\tan y} = \frac{2ac}{a^2 - c^2}`

61. Given :math:`\sin(\pi\cos x) = \cos(\pi\sin x)`

    :math:`\Rightarrow \pi\cos x = \frac{\pi}{2} - \pi\sin x`

    :math:`\Rightarrow \sin x + \cos x = \frac{1}{2}`

    1. Fividing both sides by :math:`\sqrt{2}`

       :math:`\Rightarrow \frac{\sin x}{\sqrt{2}} + \frac{\cos x}{\sqrt{2}} = \frac{1}{2\sqrt{2}}`

       :math:`\cos\left(x \pm \frac{\pi}{4}\right) = \frac{1}{2\sqrt{2}}`

    2. Squaring both sides

       :math:`\Rightarrow \sin^2x + \cos^2x + 2\sin x\cos x = \frac{1}{4}`

       :math:`\Rightarrow \sin 2x = -\frac{3}{4}`

62. Given equation is :math:`\tan(x + 100^\circ) = \tan(x + 50^\circ).\tan x.\tan(x - 50^\circ)`

    :math:`\Rightarrow \frac{\tan(x+100^\circ)}{\tan x} = \tan(x+50^\circ)\tan(x-50^\circ)`

    :math:`\Rightarrow \frac{\sin(x+100^\circ)\cos x}{\cos(x + 100^\circ)\sin x} =
    \frac{\sin(x+50^\circ)\sin(x-50^\circ)}{\cos(x+50^\circ)\cos(x-50^\circ)}`

    Appplying componendo and dividendo

    :math:`\Rightarrow \frac{\sin(x + 100^\circ)\cos x + \cos(x + 100^\circ)\sin x}{\sin(x + 100^\circ)\cos x - \cos(x +
    100^\circ)\sin x} = \frac{\sin(x+50^\circ)\sin(x-50^\circ) + \cos(x+50^\circ)\cos(x-50^\circ)}{\sin(x+50^\circ)\sin(x-50^\circ)
    -\cos(x+50^\circ)\cos(x-50^\circ)}`

    :math:`\Rightarrow \frac{\sin 2x + 100^\circ}{\sin100^\circ} = \frac{\cos100^\circ}{-\cos 2x}`

    :math:`\Rightarrow -2\sin(2x + 100^\circ)\cos2x = 2\sin100^\circ\cos100^\circ`

    :math:`\Rightarrow -\sin(4x + 100^\circ) - \sin100^\circ = \sin200^\circ`

    :math:`\Rightarrow \sin(4x + 100^\circ) = -2\sin1506\circ.\cos50^\circ = -\cos50^\circ = \sin220^\circ`

    Thus, minimum value of :math:`x` is :math:`30^\circ.`

63. We have to find :math:`x` for which :math:`\tan^2x + \sec 2x = 1`

    :math:`\Rightarrow \tan^2x + \frac{1 + \tan2x}{1 - \tan^2x} = 1`

    :math:`\Rightarrow \tan^2x - \tan^4x + 1 + \tan^2x = 1 - \tan^2x`

    :math:`\Rightarrow \tan^4x - 3\tan^2x = 0`

    :math:`\Rightarrow \tan^2x(\tan^2x - 3) = 0`

    If :math:`\tan^2x = 0 \Rightarrow x = n\pi`

    If :math:`\tan^2x = 3\Rightarrow x = n\pi\pm\frac{\pi}{3}`

    Clearly, for all these values :math:`\tan x` and :math:`\sec 2x` are defined.

64. Given equation is :math:`\sec x - \cosec x = \frac{4}{3}`

    :math:`\Rightarrow \frac{1}{\cos x}- \frac{1}{\sin x} = \frac{4}{3}`

    :math:`\Rightarrow 3(\sin x - \cos x) = 4\sin x\cos x`

    Squaring both sides

    :math:`\Rightarrow 9(\sin^2x + \cos^2x - 2\sin x\cos x) = 16\sin^2x\cos^2x`

    :math:`\Rightarrow 9(1 - \sin2x) = 4\sin^22x`

    :math:`\Rightarrow 4\sin^22x + 9\sin2x - 9 = 0`

    :math:`\Rightarrow (\sin2x + 3)(4\sin2x - 3) = 0`

    :math:`\sin2x \neq 3\therefore 4\sin2x = 3 \Rightarrow x = \frac{n\pi}{2} + (-1)^n/2.\sin^{-1}\frac{3}{4}`

65. Given equation is :math:`\sin2x - 12(\sin x - \cos x) + 12 = 0.`

    :math:`\Rightarrow 1 - \sin2x + 12(\sin x - \cos x) - 13 = 0`

    :math:`\Rightarrow (\sin x - \cos x)^2 + 12(\sin x - \cos x) - 13 = 0`

    :math:`\Rightarrow (\sin x - \cos x - 1)(\sin  x - \cos x + 13) = 0`

    Clearly, :math:`\sin x - \cos x + 13 \neq 0`

    :math:`\therefore \sin x - \cos x = 1`

    :math:`\Rightarrow \frac{1}{\sqrt{2}}\sin x - \frac{1}{\sqrt{2}}\cos x = \frac{1}{\sqrt{2}}`

    :math:`\Rightarrow \sin\left(x - \frac{\pi}{4}\right) = \sin\frac{\pi}{4}`

    :math:`\Rightarrow x = n\pi + (-1)^n\frac{\pi}{4} + \frac{\pi}{4}`

66. Given equation is :math:`\cos(p\sin x) = \sin(p\cos x)`

    :math:`\Rightarrow p\sin x = 2n\pi \pm \left(\frac{\pi}{2} - p\cos x\right)`

    Taking positive sign

    :math:`p\sin x = 2n\pi + \frac{\pi}{2} - p\cos x`

    :math:`\Rightarrow p(\sin x + \cos x) = (4n + 1)\frac{\pi}{2}`

    :math:`\Rightarrow \sin x + \cos x = \frac{(4n + 1)\pi}{2p}`

    :math:`\Rightarrow \frac{1}{\sqrt{2}}\sin x + \frac{1}{\sqrt{2}}\cos x = \frac{(4n + 1)\pi}{2\sqrt{2}p}`

    :math:`\Rightarrow \sin(x + \pi/4) = \frac{(4n + 1)p}{2\sqrt{2}p}`

    Clealry, :math:`\left|\frac{(4n + 1)\pi}{2\sqrt{2}p}\right|\leq 1`

    :math:`\Rightarrow p \geq \frac{(4n + 1)\pi}{2\sqrt{2}}`

    For smallest positive value :math:`n = 0 \therefore p = \frac{\pi}{2\sqrt{2}}`

    Taking negative sing

    :math:`p\sin x = 2n\pi - \frac{\pi}{2} + p\cos x`

    :math:`\Rightarrow p(\cos x - \sin x) = -2n\pi + \frac{\pi}{2}`

    Proceeding similarly, :math:`p \geq \frac{(-4n + 1)\pi}{2\sqrt{2}}`

    Smallest positive value of :math:`p = \frac{\pi}{2\sqrt{2}}`

67. Given equation is :math:`\cos x + \sqrt{3}\sin x = 2\cos2x`

    :math:`\Rightarrow \frac{\cos x}{2} + \frac{\sqrt{3}\sin x}{2} = \cos 2x`

    :math:`\Rightarrow \cos \left(x - \frac{\pi}{3}\right) = \cos 2x`

    :math:`\Rightarrow x - \frac{\pi}{3} = 2n\pi \pm 2x`

    Taking positive sign, :math:`x = -2n\pi - \frac{\pi}{3}`

    Taking negative sing :math:`x = \frac{2n\pi}{3} + \frac{\pi}{9}`

68. Given equation is :math:`\tan x+ \sec x = \sqrt{3}`

    :math:`\Rightarrow \frac{\sin x}{\cos x} + \frac{1}{\cos x} = \sqrt{3}`

    :math:`\Rightarrow \sqrt{3}\cos x - \sin x = 1`

    Dividing both sides by :math:`2,` we get

    :math:`\frac{\sqrt{3}}{2}\cos x - \frac{1}{2}\sin x = \frac{1}{2}`

    :math:`\Rightarrow \cos\left(x + \frac{\pi}{6}\right) = \cos \frac{\pi}{3}`

    :math:`\Rightarrow x + \frac{\pi}{6} = 2n\pi \pm \frac{\pi}{3}`

    Taking positive sign

    :math:`x = 2n\pi + \frac{\pi}{6}`

    Taking negative sign

    :math:`x = (4n - 1)\frac{\pi}{2}`

    Values of :math:`x` between :math:`0` and :math:`2\pi` are :math:`\frac{\pi}{6}, \frac{3\pi}{2}`

    However, when :math:`x = \frac{3\pi}{2}, \cos x = 0` which will be rejected.

    :math:`\therefore x = \frac{\pi}{6}`

69. Given equation is :math:`1 + \sin^3x + \cos^3x = \frac{3}{2}\sin2x`

    :math:`\Rightarrow 1 + \sin^3x + \cos^3x = 3\sin x\cos x`

    :math:`\Rightarrow 1 + \sin^3x + \cos^3x - 3\sin x\cos x = 0`

    :math:`\Rightarrow (1 + \sin x+\cos x[(1 - \sin x)^2 + (\sin x - \cos x)^2 + (\cos x - 1)^2] = 0[\because a^3 + b^3 + c^3 -
    3abc = (a + b + c).\frac{1}{2}[(a - b)^2 + (b - c)^2 + (c - a)^3]]`

    If :math:`1 + \sin x + \cos x = 0 \Rightarrow \cos x + \sin x = -1`

    :math:`\Rightarrow \frac{1}{\sqrt{2}}\cos x + \frac{1}{\sqrt{2}}\sin x = \frac{-1}{\sqrt{2}}`

    :math:`\Rightarrow \cos\left(x - \frac{\pi}{4}\right) = \cos\frac{3\pi}{4}`

    :math:`\Rightarrow x - \frac{\pi}{4} = 2n\pi \pm\frac{3\pi}{4} \Rightarrow x = 2n\pi + \frac{\pi}{4}\pm \frac{3\pi}{4}`

    else :math:`\sin x = 1, \sin x = \cos x, \cos x = 1` which is not possible.

70. Given equation is :math:`(2 + \sqrt{3})\cos x = 1 - \sin x`

    :math:`\Rightarrow \frac{1 - \sin x}{\cos x} = 2 + \sqrt{3}`

    :math:`\Rightarrow \frac{1 - \sin x}{\cos x}.\frac{1 + \sin x}{1 + \sin x} = (2 + \sqrt{3}).\frac{2 - \sqrt{3}}{2 - \sqrt{3}}`

    :math:`\Rightarrow \frac{\cos x}{1 + \sin x} = \frac{1}{2 - \sqrt{3}}` [note that we have cancelled :math:`\cos x` here]

    :math:`\Rightarrow \frac{1 + \sin x}{\cos x} = 2 - \sqrt{3}`

    :math:`\Rightarrow \frac{1 + \sin x + 1 - \sin x}{\cos x} = 2 + \sqrt{3} + 2 - \sqrt{3}`

    :math:`\Rightarrow \frac{2}{\cos x} = 4 \Rightarrow \cos x = \frac{1}{2} \Rightarrow x = 2n\pi \pm \frac{\pi}{3}`

    Since we have cancelled :math:`\cos x` one of the possible solutions is :math:`\cos x = 0 \Rightarrow x = 2n\pi + \frac{\pi}{2}`

71. Given equation is :math:`\tan\left(\frac{\pi}{2}\sin x\right) = \cot\left(\frac{\pi}{2}\cos x\right)`

    :math:`\Rightarrow \frac{\pi}{2}\sin x = \frac{\pi}{2} - \frac{\pi}{2}\cos x`

    :math:`\Rightarrow \sin x = 1 - \cos x`

    :math:`\Rightarrow \sin x + \cos x = 1`

    :math:`\Rightarrow \frac{1}{\sqrt{2}}\sin x + \frac{1}{\sqrt{2}}\cos x = \frac{1}{\sqrt{2}}`

    :math:`\Rightarrow \cos(x - \frac{\pi}{4}) = \cos \frac{\pi}{4}`

    :math:`\Rightarrow x - \frac{\pi}{4} = 2n\pi \pm \frac{\pi}{4}`

    Taking positive sign :math:`x = 2n\pi + \pi/2`

    Taking negative sign :math:`x = 2n\pi`

72. Given equation is :math:`8\cos x\cos2x\cos4x = \frac{\sin6x}{\sin x}`

    :math:`\Rightarrow 8\sin x\cos x\cos2x\cos4x = \sin6x`

    :math:`\Rightarrow 4\sin2x\cos2x\cos4x = \sin6x`

    :math:`\Rightarrow 2\sin4x\cos4x = \sin6x \Rightarrow \sin8x = \sin6x`

    :math:`\Rightarrow 2\cos7x\sin x = 0`

    If :math:`\cos7x = 0 \Rightarrow 7x = (2n + 1)\frac{\pi}{2}\Rightarrow x = (2n + 1)\frac{\pi}{14}`

    :math:`\sin x` cannot be zeor as it is in denominator.

73. Given equation is :math:`3 - 2\cos x - 4\sin x -\cos 2x + \sin 2x = 0`

    :math:`\Rightarrow 3 - 2\cos x - 4\sin x -(1 - 2\sin^2) + 2\sin x\cos x = 0`

    :math:`\Rightarrow 2(\sin^2x - 2\sin x + 1) + 2\cos x(\sin x -1) = 0`

    :math:`\Rightarrow (\sin x- 1)(2\cos x + 2\sin x - 2) = 0`

    If :math:`\sin x - 1 = 0 \Rightarrow x = n\pi + (-1)^n\frac{\pi}{2}`

    If :math:`\sin x + \cos x = 1`

    Like previous examples :math:`x = 2n\pi, 2n\pi + \frac{\pi}{2}`

74. Given equation is :math:`\sin x - 3\sin 2x + \sin 3x = \cos x - 3\cos 2x + \cos 3x`

    :math:`\Rightarrow 2\sin2x\cos x - 3\sin 2x = 2\cos2x\cos x - 3\cos 2x`

    :math:`\Rightarrow \sin2x(2\cos x - 3) = \cos2x(2\cos x - 3)`

    :math:`\because 2\cos x \neq 3 \therefore \sin 2x = \cos 2x`

    :math:`\Rightarrow \frac{1}{\sqrt{2}}\cos2x - \frac{1}{\sqrt{2}}\sin2x = 0`

    :math:`\Rightarrow 2x + \pi/4 = n\pi \Rightarrow x = n\pi/2 + \pi/8`

75. Given equation is :math:`\sin^2x\tan x + \cos^2x\cot x - \sin 2x = 1 + \tan x + \cot x`

    :math:`\Rightarrow \frac{\sin^3x}{\cos x} + \frac{\cos^3x}{\sin x} - \sin 2x = 1 + \frac{\sin x}{\cos x} + \frac{\cos x}{\sin
    x}`

    :math:`\Rightarrow \frac{\sin^4x + \cos^4x}{\sin x\cos x} - \sin2x = \frac{\sin x\cos x + \sin^2x + \cos^2x}{\sin x\cos x}`

    :math:`\Rightarrow \frac{1 - 2\sin^2x\cos^2x}{\sin x\cos x} - \sin2x = 1 + \frac{1}{\sin x\cos x}`

    :math:`\Rightarrow -2\sin x\cos x - \sin 2x = 1`

    :math:`\Rightarrow \sin 2x = -1/2 \Rightarrow 2x = n\pi + (-1)^{n + 1}\frac{\pi}{6}`

    :math:`\Rightarrow x = \frac{n\pi}{2} + (-1)^{n + 1}\frac{\pi}{12}`

76. :math:`\sin x = -\frac{1}{2} \Rightarrow x = \frac{7\pi}{6}, \frac{11\pi}{6}`

    :math:`\tan x = \frac{1}{\sqrt{3}}\Rightarrow x = \frac{\pi}{6}, \frac{7\pi}{6}`

    So common value is :math:`\frac{7\pi}{6}`

    Period of :math:`\sin x` is :math:`2\pi` and period of :math:`\tan x` is :math:`n\pi` so common period is :math:`2n\pi`

    Thus, most general value of :math:`x` is :math:`2n\pi +\frac{7\pi}{6}`

77. :math:`\tan(x - y) = 1 \Rightarrow x - y = \frac{\pi}{4}, \frac{5\pi}{4}`

    :math:`\sec(x + y) = \frac{2}{\sqrt{3}}\Rightarrow x + y = \frac{\pi}{6}, \frac{11\pi}{6}`

    Since :math:`x` and :math:`y` are positve so :math:`x + y > x - y`

    When :math:`x - y = \frac{\pi}{4}` and :math:`x + y = \frac{11\pi}{6}`

    :math:`x = \frac{25\pi}{24} y = \frac{19\pi}{24}`

    When :math:`x - y = \frac{5\pi}{5}` and :math:`x + y = \frac{11\pi}{6}`

    :math:`x = \frac{37\pi}{24}, y = \frac{7\pi}{24}`

    General Solution:

    :math:`\tan(x - y) = 1 \Rightarrow x - y = m\pi + \frac{\pi}{4}`

    :math:`\sec(x + y) = \frac{2}{\sqrt{3}} \Rightarrow x + y = 2n\pi \pm \frac{\pi}{6}`

    :math:`x = (2m + n)\frac{\pi}{2} + \frac{\pi}{8}\pm \frac{\pi}{12}`

    :math:`y = (2m - n)\frac{\pi}{2} - \frac{pi}{8}\pm \frac{\pi}{12}`

78. Given curves are :math:`y = \cos x` and :math:`y = \sin 3x`

    For intersection point both the equations must be satisfied, thus

    :math:`\cos x = \sin 3x = \cos\left(\frac{\pi}{2} - 3x\right)`

    :math:`\Rightarrow x = 2n\pi \pm \left(\frac{\pi}{2} - 3x\right)`

    :math:`\Rightarrow x = \frac{n\pi}{2} + \frac{\pi}{8}, n\pi + \frac{\pi}{4}`

    So in the given interval values of :math:`x` are :math:`\frac{\pi}{8}, -\frac{3\pi}{8}, \frac{\pi}{4}.`

79. From first equation :math:`r\sin x = \sqrt{3} \Rightarrow r = \frac{\sqrt{3}}{\sin x}`

    Substituting this value in the second equagtion, we get

    :math:`\frac{\sqrt{3}}{\sin x} + 4\sin x = 2(\sqrt{3} + 1)`

    :math:`\Rightarrow 4\sin^2x - 2\sqrt{3}\sin x - 2\sin x + \sqrt{3} = 0`

    :math:`\Rightarrow (2\sin x - \sqrt{3})(2\sin x - 1) = 0`

    If :math:`2\sin x - \sqrt{3} = 0 \Rightarrow x = n\pi + (-1)^n\frac{\pi}{3}`

    If :math:`2\sin x - 1 = 0 \Rightarrow x = n\pi + (-1)^n\frac{\pi}{6}`

    Thus, for :math:`o\leq x\leq 2\pi, x = \frac{\pi}{6}, \frac{\pi}{3}, \frac{2\pi}{3}, \frac{5\pi}{6}`

80. Given :math:`x - y = \frac{\pi}{4}` and :math:`\cot x + \cot y = 2`

    From second equation :math:`\frac{\cos x}{\sin x} + \frac{\cos y}{\sin y} = 2`

    :math:`\Rightarrow \sin(x + y) = 2\sin x\sin y = \cos(x - y) - \cos(x + y) = \cos \frac{\pi}{4} - \cos(x + y)`

    :math:`\Rightarrow \sin(x + y) + \cos (x + y) = \cos\frac{\pi}{4}`

    :math:`\Rightarrow \frac{1}{\sqrt{2}}\sin(x + y) + \frac{1}{\sqrt{2}}\cos(x + y) = \frac{1}{2} = \cos\frac{\pi}{3}`

    :math:`\Rightarrow \cos(x + y - \pi/4) = \cos\frac{\pi}{3}`

    :math:`\Rightarrow x + y - \frac{\pi}{4} = 2n\pi\pm \frac{\pi}{3}`

    :math:`x + y = 2n\pi \pm \frac{\pi}{3} + \frac{\pi}{4}`

    For :math:`n = 0, x + y = \frac{7\pi}{12}[\because x, y > 0]`

    :math:`\Rightarrow x = \frac{5\pi}{12}, y = \frac{\pi}{6}`

81. Given equations are :math:`x - y = \frac{\pi}{4}` and :math:`\cot x + \cot y = 2`
