Trigonometrical Identities Solutions
************************************
1. :math:`\because A + B + C = \pi \therefore A + B = \pi - C`

   :math:`\Rightarrow \cos(A + B) = \cos(\pi - C) = \cos C \Rightarrow \sin A\sin B - \cos C = \cos A\cos B`

   :math:`\Rightarrow (\sin A\sin B - \cos C)^2 = \cos^2A\cos^2B`

   :math:`\Rightarrow \sin^2A\sin^2B + \cos^2C - 2\sin A\sin B\cos C = (1 - \sin^2A)(1 - \sin^2B)`

   :math:`\Rightarrow \sin^A + \sin^2B + \cos^2C - 1 = 2\sin A\sin B\cos C`

   :math:`\Rightarrow \sin^2A + \sin^2B - \cos^2C = 2\sin A\sin B\cos C`

2. :math:`A + B + C = 180^\circ \Rightarrow \frac{A}{2} + \frac{B}{2} + \frac{C}{2} = 90^\circ \Rightarrow \frac{A}{2} +
   \frac{B}{2} = 90^\circ - \frac{C}{2}`

   :math:`\Rightarrow \cos\left(\frac{A}{2} + \frac{B}{2}\right) = \cos\left(90^\circ - \frac{C}{2}\right)`

   :math:`\Rightarrow \cos\frac{A}{2}\cos\frac{B}{2} - \sin\frac{A}{2}\sin\frac{B}{2} = \sin\frac{C}{2}`

   :math:`\Rightarrow \sin\frac{C}{2} + \sin\frac{A}{2}\sin\frac{B}{2} = \cos\frac{A}{2}\cos\frac{B}{2}`

   :math:`\Rightarrow \left(\sin\frac{C}{2} + \sin\frac{A}{2}\sin\frac{B}{2}\right)^2 = \cos^2\frac{A}{2}\cos^2\frac{B}{2}`

   :math:`\Rightarrow \sin^2\frac{C}{2} + \sin^2\frac{A}{2}\sin^2\frac{B}{2} + 2\sin\frac{A}{2}\sin\frac{B}{2}\sin\frac{C}{2} = \left(1 -
   \cos^2\frac{A}{2}\right)\left(1 - \cos^2\frac{B}{2}\right)`

   :math:`\sin^2\frac{A}{2} + \sin^2\frac{B}{2} + \sin^2\frac{C}{2} = 1 - 2\sin\frac{A}{2}\sin\frac{B}{2}\sin\frac{C}{2}`

3. Let :math:`A + B = C \Rightarrow \cos(A + B) = \cos C`

   :math:`\Rightarrow \sin A\sin B + \cos C = \cos A\cos B \Rightarrow (\sin A\sin B + \cos C)^2 = \cos^2A\cos^2B`

   :math:`\Rightarrow \sin^2A\sin^2B + \cos^2C + 2\sin A\sin B\cos C = (1 - \sin^2A)(1 - \sin^2B)`

   :math:`\Rightarrow \sin^2A + \sin^2B + 2\sin A\sin B\cos C = \sin^2C`

   :math:`\Rightarrow \sin^2A + \sin^2B + 2\sin A\sin B\cos(A + B) = \sin^2(A + B)`

4. Given, :math:`A + B + C = 180^\circ \Rightarrow A + B = 180^\circ - C \Rightarrow \cos(A + B) = -\cos C`

   :math:`\Rightarrow \cos A\cos B + \cos C = \sin A\sin B \Rightarrow (\cos A\cos B + \cos C)^2 = \sin^2A\sin^2B`

   :math:`\Rightarrow \cos^2A\cos^2B + \cos^2C + 2\cos A\cos B\cos C = (1 - \cos^2A)(1 - \cos^2B)`

   :math:`\Rightarrow \cos^2A + \cos^2B + \cos^2C + 2\cos A\cos B\cos C = 1`

5. We have just proved that :math:`\cos^2A + \cos^2B + \cos^2C + 2\cos A\cos B\cos C = 1`

   :math:`\Rightarrow 3 - \sin^2A - \sin^2B - \sin^2C + 2\cos A\cos B\cos C = 1`

   :math:`\Rightarrow \sin^2A + \sin^2B + \sin^2C = 2(1 + \cos A\cos B\cos C)`

6. Given, :math:`A + B + C = 180^\circ \Rightarrow A + B = 180^\circ - C \Rightarrow \cos(A + B) = -\cos C`

   :math:`\Rightarrow \cos A\cos B = \sin A\sin B - \cos C \Rightarrow \cos^2A\cos^2B = \sin^2A\sin^2B + \cos^2C - 2\sin A\sin
   B\cos C`

   :math:`\Rightarrow \cos^2A\cos^2B = (1 - \cos^2A)(1 - \cos^2B) + \cos^2C - 2\sin A\sin B\cos C`

   :math:`\Rightarrow \cos^2A + \cos^2B - \cos^2C = 1 - 2\sin A\sin B\cos C`

7. Given, :math:`A + B + C = 180^\circ \Rightarrow \frac{A + B + C}{2} = 90^\circ`

   :math:`\Rightarrow \cos\left(\frac{A}{2} + \frac{B}{2}\right) = \sin\frac{C}{2}`

   :math:`\Rightarrow \cos\frac{A}{2}\cos\frac{B}{2} - \sin\frac{C}{2} = \sin\frac{A}{2}\sin\frac{B}{2}`

   :math:`\Rightarrow \cos^2\frac{A}{2}\cos^2\frac{B}{2} + \sin^2\frac{C}{2} - 2\cos\frac{A}{2}\cos\frac{B}{2}\sin\frac{C}{2} =
   \left(1 - \cos^2\frac{A}{2}\right)\left(1 - \cos^2\frac{B}{2}\right)`

   :math:`\Rightarrow \cos^2\frac{A}{2} + \cos^2\frac{B}{2} - \cos^2\frac{C}{2} = 2\cos\frac{A}{2}\cos\frac{B}{2}\sin\frac{C}{2}`

8. Given, :math:`A + B + C = 180^\circ \Rightarrow \frac{A + B + C}{2} = 90^\circ`

   :math:`\Rightarrow \cos\left(\frac{A}{2} + \frac{B}{2}\right) = \sin\frac{C}{2}`

   :math:`\Rightarrow \cos\frac{A}{2}\cos\frac{B}{2} = \sin\frac{A}{2}\sin\frac{B}{2} + \sin\frac{C}{2}`

   :math:`\Rightarrow \cos^2\frac{A}{2}\cos^2\frac{B}{2} = \sin^2\frac{A}{2}\sin^2\frac{B}{2} + \sin^2\frac{C}{2} +
   2\sin\frac{A}{2}\sin\frac{B}{2}\sin\frac{C}{2}`

   :math:`\Rightarrow \cos^2\frac{A}{2}\cos^2\frac{B}{2} = \left(1 - \cos^2\frac{A}{2}\right)\left(1 - \cos^2\frac{B}{2}\right) +
   \sin^2\frac{C}{2} + 2\sin\frac{A}{2}\sin\frac{B}{2}\sin\frac{C}{2}`

   :math:`\cos^2\frac{A}{2} + \cos^2\frac{B}{2} + \cos^2\frac{C}{2} = 2 + 2\sin\frac{A}{2}\sin\frac{B}{2}\sin\frac{C}{2}`

9. Given, :math:`A + B + C = \frac{\pi}{2} \Rightarrow A + B = \frac{\pi}{2} - C \Rightarrow \cos(A + B) = \sin C`

   :math:`\Rightarrow \cos A\cos B = \sin A\sin B + \sin C`

   :math:`\Rightarrow \cos^2A\cos^2B = \sin^2A\sin^2B + \sin^2C + 2\sin A\sin B\sin C`

   :math:`\Rightarrow (1 - \sin^2A)(1 - \sin^2B) = \sin^2A\sin^2B + \sin^2C + 2\sin A\sin B\sin C`

   :math:`\Rightarrow \sin^2A + \sin^2B + \sin^2C = 1 - 2\sin A\sin B\sin C`

10. We have just proven that :math:`\sin^2A + \sin^2B + \sin^2C = 1 - 2\sin A\sin B\sin C` in previous problem.

    :math:`\Rightarrow 1 - \cos^2A + 1 - \cos^2B + 1 - \cos^2C = 1 - 2\sin A\sin B\sin C`

    :math:`\Rightarrow \cos^2A + \cos^2B + \cos^2C = 2 + 2\sin A\sin B\sin C`

11. Givem :math:`A + B + C = 2\pi \Rightarrow A + B = 2\pi - C \Rightarrow \cos(A + B) = \cos C`

    :math:`\Rightarrow \cos A\cos B - \cos C = \sin A\sin B`

    :math:`\Rightarrow \cos^2A\cos^2B + \cos^2C - 2\cos A\cos B\cos C = \sin^2A\sin^2B = (1 - \cos^2A)(1 - \cos^2B)`

    :math:`\Rightarrow \cos^2A + \cos^2B + \cos^2C - 2\cos A\cos B\cos C = 1`

12. Given :math:`A + B = C \Rightarrow \cos(A + B) = \cos C`

    :math:`\Rightarrow \cos A\cos B - \cos C = \sin A\sin B`

    :math:`\Rightarrow \cos^2A\cos^2B + \cos^2C - 2\cos A\cos B\cos C = \sin^2A\sin^2B`

    :math:`\Rightarrow \cos^2A\cos^2B + \cos^2C - 2\cos A\cos B\cos C = (1 - \cos^2A)(1 - \cos^2B)`

    :math:`\Rightarrow \cos^2A + \cos^2B + \cos^2C - 2\cos A\cos B\cos C = 1`

13. Given :math:`A + B = \frac{\pi}{3} \Rightarrow \cos(A + B) = \cos\frac{\pi}{3} = \frac{1}{2}`

    :math:`\Rightarrow \cos A\cos B - \frac{1}{2} = \sin A\sin B`

    :math:`\Rightarrow \cos^2A\cos^2B - \cos A\cos B + \frac{1}{4} = \sin^2A\sin^2B = (1 - \cos^2A)(1 - \cos^2B)`

    :math:`\Rightarrow \cos^2A + \cos^2B - \cos A\cos B = \frac{3}{4}`

14. From problem 12 we have :math:`A + B = C` and :math:`\cos^2A + \cos^2B + \cos^2C - 2\cos A\cos B\cos C = 1`

    Substituting :math:`C = A + B` we get :math:`\cos^2A + \cos^2B + \cos^2(A + B) - 2\cos A\cos B\cos(A + B) = 1`

    :math:`\Rightarrow \cos^2B + \cos^2(A + B) - 2\cos A\cos B\cos(A + B) = 1 - \cos^2A = \sin^2A` which is independent of
    :math:`B`

15. Given :math:`A + B + C = \pi` and :math:`A + B = 2C \Rightarrow C = \frac{\pi}{3} \Rightarrow A + B = \pi - \frac{pi}{3}`

    :math:`\cos(A + B) = -\cos\frac{\pi}{3}\Rightarrow \cos A\cos B = \sin A\sin B - \frac{1}{2}`

    :math:`\Rightarrow \cos^2A\cos^2B = \sin^2A\sin^2B - \sin A\sin B + \frac{1}{4}`

    :math:`\Rightarrow (1 - \sin^2A)(1 - \sin^2B) = \sin^2A\sin^2B - \sin A\sin B + \frac{1}{4}`

    :math:`\Rightarrow 4(\sin^2A + \sin^2B - \sin A\sin B) = 3`

16. Given :math:`A + B + C = 2\pi \Rightarrow \cos(B + C) = \cos(2\pi - A) = \cos A`

    :math:`\Rightarrow \cos B\cos C - \cos A = \sin B\sin C`

    :math:`\Rightarrow \cos^B\cos^2C + \cos^2A - 2\cos A\cos B\cos C = \sin^2B\sin^2C = (1 - \cos^2B)(1 - \cos^2C)`

    :math:`\Rightarrow \cos^2B + \cos^2C - \sin^2A - 2\cos A\cos B\cos C = 0`

17. Given :math:`A + B + C = 0 \Rightarrow \cos(A + B) = \cos C`

    :math:`\Rightarrow \cos A\cos B - \cos C = \sin A\sin B`

    :math:`\Rightarrow \cos^2A\cos^2B + \cos^2C - 2\cos A\cos B\cos C = \sin^2A\sin^2B = (1 - \cos^2A)(1 - \cos^2B)`

    :math:`\Rightarrow \cos^2A + \cos^2B + \cos^2C = 1 + 2\cos A\cos B\cos C`

18. Putting :math:`A = B - C, B = C - A` and :math:`C = A - B` in 17 we can obtain the desired result.

19. Given :math:`A + B + C = \pi,` we have to prove that :math:`\sin A\cos B\cos C + \sin B\cos C\cos A + \sin C\cos A\cos B= \sin
    A\sin B\sin C`

    Dividing both sides by :math:`\sin A\sin B\sin C,` we get

    :math:`\cot B\cot C + \cot C\cot A + \cot A\cot B = 1`

    :math:`A + B = \pi - C\Rightarrow \cot(A + B) = -\cot C`

    :math:`\Rightarrow \frac{\cot A\cot B - 1}{\cot A + \cot B} = -\cot C`

    :math:`\Rightarrow \cot B\cot C + \cot C\cot A + \cot A\cot B = 1`

20. Given, :math:`A + B + C = \pi \Rightarrow A + B = \pi - C`

    :math:`\Rightarrow \tan(A + B) = \tan(\pi - C) = -\tan C`

    :math:`\Rightarrow \frac{\tan A + \tan B}{1 - \tan A\tan B} = -\tan C`

    :math:`\Rightarrow \tan A + \tan B + \tan C = \tan A\tan B\tan C`

21. Given :math:`A + B + C = \pi \Rightarrow \frac{A + B}{2} = \frac{\pi - C}{2}`

    :math:`\Rightarrow \tan\frac{A + B}{2} = \tan\frac{\pi - C}{2}`

    :math:`\Rightarrow \frac{\tan\frac{A}{2} + \tan\frac{B}{2}}{1 - \tan\frac{A}{2}\tan\frac{B}{2}} = \cot\frac{C}{2} =
    \frac{1}{\tan\frac{C}{2}}`

    :math:`\Rightarrow \tan\frac{A}{2}\tan\frac{B}{2} + \tan\frac{B}{2}\tan\frac{C}{2} + \tan\frac{C}{2}\tan\frac{A}{2} = 1`

22. Let :math:`B + C - A = \alpha, C + A - B = \beta, A + B - C = \gamma`

    :math:`\alpha + \beta + \gamma = A + B + C = \pi`

    We have just proven that if :math:`A + B + C = \pi` then :math:`\Rightarrow \tan A + \tan B + \tan C = \tan A\tan B\tan C`

    Thus, substituting we get, :math:`\Rightarrow \tan\alpha + \tan\beta + \tan\gamma = \tan\alpha\tan\beta\tan\gamma`

    :math:`\Rightarrow \tan(B + C - A) + \tan(C + A - B) + \tan(A + B - C) = \tan(B + C - A)\tan(C + A -
    B)\tan(A + B - C)`

23. Given :math:`A + B + C = \pi\Rightarrow  A + B = \pi - C \Rightarrow \cot(A + B) = \cot(\pi - C)`

    :math:`\Rightarrow \frac{\cot A\cot B - 1}{\cot A + \cot B} = -\cot C`

    :math:`\Rightarrow \cot B\cot C + \cot C\cot A + \cot A\cot B = 1`

24. From previosu problem if :math:`A + B + C = \pi` then :math:`\Rightarrow \cot B\cot C + \cot C\cot A + \cot A\cot B = 1`

    Given :math:`\cot A + \cot B + \cot C = \sqrt{3}`

    :math:`\Rightarrow \cot^2A + \cot^2B + \cot^2C + 2(\cot A\cot B + \cot B\cot C + \cot C\cot A) = 3`

    :math:`\cot^2A + \cot^2B + \cot^2C = 1`

    :math:`2\cot^2A + 2\cot^2B + 2\cot^2C - 2 = 0`

    :math:`2\cot^2A + 2\cot^2B + 2\cot^2C - 2(\cot A\cot B + \cot B\cot C + \cot C\cot A) = 0`

    :math:`(\cot A - \cot B)^2 + (\cot B - \cot C)^2 + (\cot C - \cot A)^2 = 0`

    This is possible only if :math:`\cot A - \cot B = 0` i.e. :math:`\cot A = \cot B,` :math:`\cot B - \cot C = 0` i.e. :math:`\cot
    B = \cot C` and :math:`\cot C - \cot A = 0` i.e. :math:`\cot C = \cot A`

    :math:`\therefore \cot A = \cot B = \cot C \Rightarrow A = B = C`

25. :math:`\because A + B + C + D = 2\pi \Rightarrow A + B = 2\pi - C - D`

    :math:`\Rightarrow \tan(A + B) = -\tan(C + D)`

    :math:`\Rightarrow \frac{\tan A + \tan B}{1 - \tan A\tan B} = -\frac{\tan C + \tan D}{1 - \tan C\tan D}`

    :math:`\Rightarrow (\tan A + \tan B)(1 - \tan C\tan D) = -(1 - \tan A\tan B)(\tan C + \tan D)`

    :math:`\Rightarrow \tan A + \tan B + \tan C + \tan D = \tan A\tan B\tan C + \tan A\tan C\tan D + \tan A\tan B\tan D + \tan
    B\tan C\tan D`

    Dividing both sides by :math:`\tan A\tan B\tan C\tan D,` we get

    :math:`\frac{\tan A + \tan B + \tan C + \tan D}{\tan A\tan B\tan C\tan D} = \frac{1}{\tan A} + \frac{1}{\tan B} + \frac{1}{\tan
    C} + \frac{1}{\tan D}`

    :math:`\Rightarrow \frac{\tan A + \tan B + \tan C + \tan D}{\cot A + \cot B + \cot C + \cot D} = \tan A\tan B\tan C\tan D`

26. Given :math:`A + B + C = \frac{\pi}{2}\Rightarrow A + B = \frac{\pi}{2} - C`

    :math:`\Rightarrow \cot(A + B) = \cot\left(\frac{\pi}{2} - C\right)`

    :math:`\Rightarrow \frac{\cot A\cot B - 1}{\cot A + \cot B} = \tan C = \frac{1}{\cot C}`

    :math:`\Rightarrow \cot A + \cot B + \cot C = \cot A\cot B\cot C`

27. We have just proven in 26 that :math:`\Rightarrow \cot A + \cot B + \cot C = \cot A\cot B\cot C`

    Dividing both sides by :math:`\cot A\cot B\cot C,` we get

    :math:`\tan A\tan B + \tan B\tan C + \tan C\tan A = 1`

28. Given :math:`A + B + C = \pi \Rightarrow 3(A + B + C) = 3\pi \Rightarrow 3A + 3B = 3\pi - 3C`

    :math:`\Rightarrow \tan(3A + 3B) = \tan(3\pi - 3C) = -\tan3C`

    :math:`\Rightarrow \frac{\tan 3A + \tan 3B}{1 - \tan3A\tan3B} = -\tan3C`

    :math:`\Rightarrow \tan 3A + \tan 3B + \tan 3C = \tan 3A\tan 3B\tan 3C`

29. Given :math:`A + B + C = \pi \Rightarrow \frac{A + B}{2} = \frac{\pi - C}{2}`

    :math:`\Rightarrow \cot\frac{A + B}{2} = \cot\frac{\pi - C}{2}`

    :math:`\Rightarrow \frac{\cot\frac{A}{2}\cot\frac{B}{2} - 1}{\cot\frac{A}{2} + \cot\frac{B}{2}} = \tan\frac{C}{2} =
    \frac{1}{\cot\frac{C}{2}}`

    :math:`\Rightarrow \cot \frac{A}{2} + \cot \frac{B}{2} + \cot \frac{C}{2} = \cot \frac{A}{2}\cot
    \frac{B}{2}\cot \frac{C}{2}`

30. We have to prove that :math:`\frac{\cot A + \cot B}{\tan A + \tan B} + \frac{\cot B + \cot C}{\tan B + \tan C}
    + \frac{\cot C + \cot A}{\tan C + \tan A} = 1`

    Putting :math:`\tan A = \frac{1}{\cot A}, \tan B = \frac{1}{\cot B}, \tan C = \frac{1}{\cot C},` we get

    :math:`\cot A\cot B + \cot B\cot C + \cot C\cot A = 1`

    We have already proven above in problem 19.

31. Let :math:`A - B = \alpha, B - C = \beta, C - A = \gamma,` then

    :math:`\alpha + \beta + \gamma = 0`

    :math:`\Rightarrow \tan(\alpha + \beta) = -\tan\gamma`

    :math:`\Rightarrow \frac{\tan\alpha + \tan\beta}{1 - \tan\alpha\tan\beta} = -\tan\gamma`

    :math:`\tan\alpha + \tan\beta + \tan\gamma = \tan\alpha\tan\beta\tan\gamma`

    Substituting back the values, we get

    :math:`\tan(A - B) + \tan(B - C) + \tan(C - A) = \tan(A - B)\tan(B - C)\tan(C - A)`

32. We have already proven in problem 19 that if :math:`A + B + C = 0,` then

    :math:`\cot A\cot B + \cot B\cot C + \cot C\cot A = 1`

    Let :math:`A = x + y - z, B = z + x - y, C = y + z - x,` then

    :math:`A + B + C = x + y + z = 0`

    :math:`\Rightarrow \cot A\cot B + \cot B\cot C + \cot C\cot A = 1`

    Substituting back the values, we get

    :math:`\cot(x + y - z)\cot(z + x - y) + \cot(x + y - z)\cot(y + z - x) + \cot(y + z - x)\cot(z + x - y) = 1`

33. Given :math:`A + B + C= n\pi \Rightarrow \tan(A + B) = \tan(n\pi - C) = -\tan C`

    :math:`\Rightarrow \frac{\tan A + \tan B}{1 - \tan A\tan B} = -\tan C`

    :math:`\Rightarrow \tan A + \tan B + \tan C = \tan A\tan B\tan C`
