Trigonometrical Ratios Solutions
********************************
Go through the list of relationship between trigonometrical ratios as the problems are centered around those.

1. L.H.S. :math:`= \sqrt{\frac{1- \cos A}{1 + \cos A}}`

   Multiplying and dividing with :math:`1 - \cos A,` we get

   :math:`= \sqrt{\frac{(1 - \cos A)^2}{1 - \cos^2 A}}`

   :math:`= \sqrt{\left(\frac{1 - \cos A}{\sin A}\right)^2}`

   :math:`= \frac{1 - \cos A}{\sin A} = \cosec A - \cot A =` R.H.S.

2. L.H.S. :math:`\sqrt{1 + \tan^2A + 1 + \cot^2A}` [:math:`\because \sec^2A = 1 + \tan^2A` and :math:`\cosec^2A = 1 + \cot^2 A` ]

   :math:`= \sqrt{\tan^2A + 2\tan A\cot A + \cot^2A}` [:math:`\tan A\cot A = 1` ]

   :math:`= \sqrt{(\tan A + \cot A)^2} =` R.H.S.

3. L.H.S :math:`= \left(\frac{1 - \sin^2 A}{\sin A}\right)\left(\frac{1 - \cos^2 A}{\cos A}\right)\left(\frac{\sin^2A +
   \cos^2A}{\sin A \cos A}\right)`

   :math:`= \frac{\cos^2A}{\sin A}\frac{\sin^2 A}{\cos A}\frac{1}{\sin A \cos A} = 1`

4. L.H.S. :math:`= \cos^4A - \sin^4A  + 1= (\cos^2A + \sin^2A)(\cos^2A - \sin^2A) + 1`

   :math:`= \cos^2A - \sin^2A + 1 = 2\cos^2A`

5. L.H.S. :math:`= (\sin A + \cos A)(1 - \sin A\cos A) = (\sin A + \cos A)(\sin^2A + \cos^2A - \sin A\cos A)`

   :math:`= \sin^3A + \cos^3A =` R.H.S.

6. L.H.S :math:`= \frac{\sin A}{1 + \cos A}+\frac{1 + \cos A}{\sin A} = \frac{\sin^2A + (1 + \cos A)^2}{\sin A(1 + \cos A)}`

   :math:`= \frac{\sin^2A + 1 + 2\cos A + \cos^2A}{\sin A(1 + \cos A)} = \frac{1 + 1 + 2\cos A}{(\sin A)(1 + \cos A))}`

   :math:`= \frac{2}{\sin A} = 2\cosec A =` R.H.S.

7. L.H.S. :math:`= \sin^6A - cos^6A = (\sin^2A + \cos^2A)^3 - 3\cos^4A\sin^2A - 3\cos^2A\sin^4A`

   :math:`= 1 - 3\sin^2A\cos^2A(\cos^2A + \sin^2A) = 1 - 3\sin^2A\cos^2A =` R.H.S.

8. L.H.S. :math:`= \sqrt{\frac{1 - \sin A}{1 + \sin A}}`

   Multiplying and dividing with :math:`1 - \sin A,` we get

   :math:`= \sqrt{\frac{(1 - \sin A)^2}{1 - \sin^2A}} = \sqrt{\frac{(1 - \sin A)^2}{\cos^2A}} = \sqrt{\left(\frac{1 - \sin A}{\cos
   A}\right)^2}`

   :math:`= \frac{1 - \sin A}{\cos A} = \sec A - \tan A`

9. L.H.S. :math:`= \frac{\cosec A}{\cosec A - 1} + \frac{\cosec A}{\cosec A + 1} = \frac{\frac{1}{\sin A}}{\frac{1}{\sin A} - 1} +
   \frac{\frac{1}{\sin A}}{\frac{1}{\sin A} + 1}`

   :math:`= \frac{1}{1 - \sin A} + \frac{1}{1 + \sin A} = \frac{1}{(1 - \sin A)(1 + \sin A)} = \frac{1}{\cos^2A} = \sec^2A =`
   R.H.S.

10. L.H.S. :math:`= \frac{\cosec A}{\tan A + \cot A} = \frac{\frac{1}{\sin A}}{\frac{\sin A}{\cos A} + \frac{\cos A}{\sin A}}`

    :math:`= \frac{\frac{1}{\sin A}}{\frac{\sin^2A + \cos^2A}{\sin A\cos A}} = \frac{\frac{1}{\sin A}}{\frac{1}{\sin A\cos A}} =
    \cos A =` R.H.S.

11. L.H.S. :math:`= (\sec A + \cos A)(\sec A - \cos A) = \sec^2A - \cos^2A = 1 + \tan^2A - 1 + \sin^2A = \tan^2A + \sin^2A =`
    R.H.S.

12. L.H.S. :math:`= \frac{1}{\tan A + \cot A} = \frac{1}{\frac{\sin A}{\cos A} + \frac{\cos A}{\sin A}} = \frac{1}{\frac{\sin^2A +
    \cos^2A}{\sin A\cos A}} = \sin A\cos A =` R.H.S.

13. L.H.S :math:`= \frac{1 - \tan A}{1 + \tan A} = \frac{1 - \frac{1}{\cot A}}{1 + \frac{1}{\cot A}} = \frac{\cot A - 1}{\cot A +
    1} =` R.H.S.

14. L.H.S. :math:`= \frac{1 + \tan^2A}{1 + \cot^2A} = \frac{1 + \frac{\sin^2A}{\cos^2A}}{1 + \frac{\cos^2A}{\sin^A}}`

    :math:`= \frac{\frac{\cos^2A + \sin^2A}{\cos^2A}}{\frac{\sin^2A + \cos^2A}{\sin^2A}} = \frac{\sin^2A}{\cos^2A} =` R.H.S.

15. L.H.S. :math:`= \frac{\sec A - \tan A}{\sec A + \tan A}`

    Multiplying and dividing with :math:`\sec A - \tan A,` we get

    :math:`\frac{(\sec A - \tan A)^2}{\sec^2A - \tan^2A} = \sec^2A - 2\tan A\sec A + \tan^A = 1 + \tan^2A - 2\tan A\sec A +
    \tan^2A`

    :math:`= 1 - 2\tan A\sec A + 2\tan^2A =` R.H.S.

16. L.H.S. :math:`= \frac{1}{\sec A - \tan A}`

    Multiplying and dividing with :math:`\sec A + \tan A,` we get

    :math:`= \frac{\sec A + \tan A}{\sec^2A = \tan^2A} = \sec A + \tan A =` R.H.S.

17. L.H.S. :math:`= \frac{\tan A}{1 - \cot A} + \frac{\cot A}{1 - \tan A}`

    :math:`= \frac{\frac{\sin A}{\cos A}}{1 - \frac{\cos A}{\sin A}} + \frac{\frac{\cos A}{\sin A}}{1 - \frac{\sin A}{\cos A}}`

    :math:`= \frac{\sin^2A}{\cos A(\sin A - \cos A)} + \frac{\cos^2A}{\sin A(\cos A - \sin A)}`

    :math:`= \frac{\sin^3A - \cos^3A}{\sin A\cos A(\sin A - \cos A)} = \frac{\sin^2A + \cos^2A + \sin A\cos A}{\sin A\cos A}`

    :math:`= \frac{1 + \sin A \cos A}{\sin A\cos A} = 1 + \cosec A\sec A =` R.H.S.

18. L.H.S. :math:`= \frac{\cos A}{1 - \tan A} + \frac{\sin A}{1 - \cot A} = \frac{\cos A}{1 - \frac{\sin A}{\cos A}} + \frac{\sin
    A}{1 - \frac{\cos A}{\sin A}}`

    :math:`= \frac{\cos^2A}{\cos A - \sin A} + \frac{\sin^2A}{\sin A - \cos A} = \frac{\cos^2A - \sin^2A}{\cos A - \sin A}`

    :math:`= \cos A + \sin A =` R.H.S.

19. L.H.S. :math:`= (\sin A + \cos A)(\tan A + \cot A) = (\sin A + \cos A)(\frac{\sin A}{\cos A} + \frac{\cos A}{\sin A})`

    :math:`= (\sin A + \cos A)\frac{\sin^2A + \cos^2A}{\sin A\cos A} = \frac{\sin A + \cos A}{\sin A\cos A} = \sec A + \cosec A =`
    R.H.S.

20. L.H.S. :math:`= \sec^4A - \sec^2A = (1 + \tan^2A) - 1 - \tan^2A = 1 + 2\tan^2A + \tan^4A - 1 - \tan^2A = \tan^4A + \tan^2A =`
    R.H.S.

21. L.H.S. :math:`= \cot^4A + \cot^2A = (\cosec^2A - 1)^1 + \cosec^2A - 1 = \cosec^4A - 2\cosec^2A + 1 + \cosec^2A -1 = \cosec^4A -
    \cosec^2A =` R.H.S.

22. L.H.S. :math:`= \sqrt{\cosec^2A - 1} = \sqrt{\cot^2A} = \cot A = \frac{\cos A}{\sin A} = \cos A \cosec A =` R.H.S.

23. L.H.S. :math:`= \sec^2A\cosec^2A = (1 + \tan^2A)(1 + \cot^2A) = 1 + \tan^2A + \cot^2A + \tan^2A\cos^2A = 2 + \tan^2A + \cot^2A
    =` R.H.S.

24. L.H.S. :math:`= \tan^2A - \sin^2A = \frac{\sin^2A}{\cos^2A} - \sin^2A = \frac{\sin^2A - \sin^2A\cos^2A}{\cos^2A} = \sin^2A(1 -
    \cos^2A)\sec^2A = \sin^4A\sec^2A =` R.H.S.

25. L.H.S. :math:`= (1 + \cot A - \cosec A)(1 + \tan A + \sec A) = \left(1 + \frac{\cos A}{\sin A} - \frac{1}{\sin A}\right)\left(1
    + \frac{\sin A}{\cos A} + \frac{1}{\cos A}\right)`

    :math:`= \frac{(\sin A + \cos A - 1)(\sin A + \cos A + 1)}{\sin A\cos A} = \frac{(\sin A + \cos A)^2 - 1}{\sin A\cos A}`

    :math:`= \frac{\sin^2A + \cos^2A + \sin A\cos A - 1 }{\sin A\cos A} = \frac{1 + 2\sin A\cos A - 1}{\sin A\cos A} = 2=` R.H.S.

26. L.H.S. :math:`= \frac{\cot A\cos A}{\cot A + \cos A} = \frac{\frac{\cos^2 A}{\sin A}}{\frac{\cos A}{\sin A} + \cos A}`

    :math:`= \frac{\cos^2A}{\sin A}{\frac{\sin A}{\cos A(1 + \sin A)}} = \frac{\cos A}{1 + \sin A}`

    Proceeding in same way for R.H.S. we obtain :math:`\frac{1 - \sin A}{\cos A}`

    :math:`\frac{\cos A}{1 + \sin A} = \frac{\cos A(1 - \sin A)}{1 - \sin^2A} = \frac{1 - \sin A}{\cos A} =` R.H.S.

27. L.H.S. :math:`= \frac{\cot A + \tan B}{\cot B + \tan A} = \frac{\frac{1}{\tan A} + \tan B}{\frac{1}{\tan B} + \tan A}`

    :math:`\frac{\frac{1 + \tan A\tan B}{\tan A}}{\frac{1 + \tan A\tan B}{\tan B}} = \frac{\tan B}{\tan A} = \cot A\tan B =` R.H.S.

28. L.H.S. :math:`= \left(\frac{1}{\sec^2 A - \cos^2A} + \frac{1}{\cosec^2A - \sin^2A}\right)\cos^2A\sin^2A`

    :math:`= \left(\frac{1}{\frac{1}{\cos^2A} - \cos^2A} + \frac{1}{\frac{1}{\sin^2A} - \sin^2A}\right)\cos^2A\sin^2A`

    :math:`= \left(\frac{\cos^2A}{1 - \cos^4A} + \frac{\sin^2A}{1 - \sin^4}\right)\cos^2A\sin^2A`

    :math:`= \left(\frac{\cos^2A}{(1 - \cos^2A)(1 + \cos^2A)} + \frac{\sin^2A}{(1 - \sin^2A)(1 + \sin^2A)}\right)\cos^2A\sin^2A`

    :math:`= \left(\frac{\cos^2A}{\sin^2A(1 + \cos^2A)} + \frac{\sin^2A}{\cos^2A(1 + \sin^2A)}\right)\cos^2A\sin^2A`

    :math:`= \left(\frac{\cos^4A(1 + \sin^2A) + \sin^4A(1 + \cos^2A)}{\sin^2A\cos^2A(1 + \cos^2A))(1 +
    \sin^2A)}\right)\cos^2A\sin^2A`

    :math:`= \left(\frac{\cos^4A + \sin^4A + \cos^2A\sin^2A(\cos^2A + \sin^2A)}{(1 +\cos^2A)(1 + \sin^2A)}\right)`

    :math:`= \left(\frac{(\cos^2A + \sin^2A)^2 - \cos^2A\sin^2A}{1 + \sin^2A + \cos^2A + \sin^2A\cos^2A}\right)`

    :math:`= \frac{1 - \sin^2A\cos^2A}{2 + \sin^2A\cos^2A} =` R.H.S.

29. L.H.S. :math:`= \sin^8A - \cos^8A = (\sin^4A - \cos^4A)(\sin^4A + \cos^4A)`

    :math:`= (\sin^2A + \cos^2A)(\sin^2A - \cos^2A)((\sin^2A + \cos^2A)^2 - 2\sin^2A\cos^2A)`

    :math:`= (\sin^2A - \cos^2A)(1 - 2\sin^2A\cos^2A) =` R.H.S.

30. L.H.S. :math:`= \frac{\cos A\cosec A - \sin A\sec A}{\cos A + \sin A} = \frac{\frac{\cos A}{\sin A} - \frac{\sin A}{\cos
    A}}{\cos A + \sin A}`

    :math:`= \frac{\cos^2A - \sin^2A}{\sin A\cos A(\cos A + \sin A)} = \frac{\cos A  \sin A}{\sin A\cos A} = \cosec A - \sec A =`
    R.H.S.

31. Given, :math:`\frac{1}{\cosec A - \cot A} - \frac{1}{\sin A} = \frac{1}{\sin A} - \frac{1}{\cosec A + \cot A}`

    Therefore alternatively we can prove that :math:`\frac{1}{\cosec A - \cot A} + \frac{1}{\cosec A + \cot A} = \frac{2}{\sin A}`

    L.H.S. :math:`= \frac{1}{\frac{1}{\sin A} - \frac{\cos A}{\sin A}} + \frac{1}{\frac{1}{\sin A} + \frac{\cos A}{\sin A}}`

    :math:`= \frac{\sin A}{1 - \cos A} - \frac{\sin A}{1 + \cos A} = \frac{\sin A(1 + \cos A + 1 - \cos A)}{1 - \cos^2 A} =
    \frac{2\sin A}{\sin^2A} = \frac{2}{\sin A} =` R.H.S.

32. L.H.S. :math:`= \frac{\tan A + \sec A - 1}{\tan A - \sec A + 1} = \frac{\frac{\sin A + 1 - \cos A}{\cos A}}{\frac{\sin A + \cos
    A - 1)}{\cos A}}`

    :math:`= \frac{1 + \sin A - \cos A}{\sin A + \cos A - 1} = \frac{(1 + \sin A - \cos A)(\sin A + \cos A - 1)}{(\sin A + \cos A -
    1)^2}`

    Solving this yields :math:`= \frac{1 + \sin A}{\cos A} =` R.H.S.

33. L.H.S. :math:`= (\tan A + \cosec B)^2 - (\cot B - \sec A)^2 = \tan^2A + \cosec^2B + 2\tan A\cosec B - \cot^2B - \sec^2A+ 2\sec
    A\cot B`


    :math:`= (\cosec^2B - \cot^2B) - (sec^2A - tan^2A) + 2\tan A\cot B\left(\frac{\cosec B}{\cot B} + \frac{\sec A}{\tan A}\right)`

    :math:`= 1 - 1 + 2\tan A\cot B\left(\sec B + \cosec A\right)  =` R.H.S.

34. L.H.S. :math:`= 2\sec^2 A - \sec^4A - 2\cosec^2A + \cosec^4A = 2(1 + \tan^2A) - (1 + \tan^2A)^2 - 2(1 + \cot^2A) + (1 +
    \cot^2A)^2`

    :math:`= 2 + 2\tan^2A - 1 - 2\tan^2A + \tan^4A - 2 - 2\cot^2A + 1 + 2\cot^2A + \cot^4A = \cot^4A - \tan^4A =` R.H.S.

35. L.H.S. :math:`= (\sin A + \cosec A)^2 + (\cos A + \sec A)^2 = \sin^2A + \cosec^2A + 2\sin A\cosec A + \cos^2A + \sec^2A + 2\sec
    A\cosec A`

    :math:`= (\sin^2A + \cos^2A) + 4 + \cosec^2A + \sec^2A = 1 + 4 + 1 + \cot^2A + 1 + \tan^2A = \cot^2A + \tan^2A + 7 =` R.H.S.

36. L.H.S :math:`= (\cosec A + \cot A)(1 - \sin A) - (\sec A + \tan A)(1 - \cos A)`

    :math:`= \left(\frac{1}{\sin A} + \frac{\cos A}{\sin A}\right)(1 - \sin A) - \left(\frac{1}{\cos A} + \frac{\sin A}{\cos
    A}\right)(1 - \cos A)`

    :math:`= \frac{(1 + \cos A)(1 - \sin A)}{\sin A} - \frac{(1 + \sin A)(1 - \cos A)}{\cos A}`

    :math:`= \frac{\cos A(1 + \cos A - \sin A - \cos A\sin A) -\sin A(1 + \sin A - \cos A - \sin A\cos A)}{\sin A\cos A}`

    :math:`= \frac{(1 - \sin A\cos A)(\cos A - \sin A) + (\cos A - \sin A)(\cos A + \sin A)}{\sin A\cos A}`

    :math:`= \frac{(\cos A - \sin A)(1 - \cos A\sin A + \cos A + \sin A)}{\sin A\cos A}`

    :math:`= \left(\frac{(\cos A - \sin A)}{\sin A\cos A}\right)(2 - 1 - \cos A\sin A + \cos A + \sin A)`

    :math:`= (\cosec A - \sec A)(2 - (1 - \cos A)(1 - \sin A)) =` R.H.S.

37. L.H.S :math:`= (1 + \cot A + \tan A)(\sin A - \cos A) = \left(1 + \frac{\cosec A}{\sec A} + \frac{\sec A}{\cosec
    A}\right)\left(\frac{1}{\cosec A} - \frac{1}{\sec A}\right)`

    :math:`= \left(\frac{\sec A\cosec A + \sec A | \cosec A}{\sec A\cosec A}\right)\left(\frac{\sec A - \cosec A}{\sec A\cosec
    a}\right)`

    :math:`= \frac{\sec^3A - \cosec^3A}{\sec^2A\cosec^2A} = \frac{\sec A}{\cosec^2A} - \frac{\cosec A}{\sec^2A} =` R.H.S.

38. Given, :math:`\frac{1}{\sec A - \tan A} - \frac{1}{\cos A} = \frac{1}{\cos A} - \frac{1}{\sec A + \tan A}`

    So alternatively we can prove that :math:`\frac{1}{\sec A - \tan A} + \frac{1}{\sec A + \tan A} = \frac{2}{\cos A}`

    L.H.S. :math:`= \frac{\sec A + \tan A + \sec A - \tan A}{\sec^2A - tan^2A} = 2\sec A = \frac{2}{\cos A} =` R.H.S.

39. L.H.S. :math:`= 3(\sin A - \cos A)^4 + 4(\sin^6 A + \cos^6 A) + 6(\sin A + \cos A)^2`

    :math:`= 3[(\sin A - \cos A)^2]^2 + 4[(\sin^2A)^3 + (\cos^2A)^3] + 6(\sin^2A + \cos^2A + 2\cos A\sin A)`

    :math:`= 3[(\sin^2A + \cos^2A - 2\sin A\cos A)]^2 + 4(\sin^2A + \cos^2A)(\sin^4A + \cos^4A - \sin^2A\cos^2A) + 6(1 + 2\cos A\sin
    A)`

    :math:`= 3(1 - 2\sin A\cos A)^2 + 4(\sin^4A + \cos^4A - \sin^2A\cos^2A) + 6(1 + 2\cos A\sin A)`

    :math:`= 3(1 + 4\sin^2A\cos^2A - 4\cos A\sin A) + 4[(\sin^2A + \cos^2A)^2 - 2\sin^2A\cos^2A - \sin^2A\cos^2A] + 6(1 + 2\sin
    A\cos A)`

    :math:`= 3 + 12\sin^2A\cos^2A -12\cos A\sin A + 4(1 - 3\sin^2A\cos^2A) + 6 + 12\sin A\cos A`

    :math:`= 13 =` R.H.S.

40. L.H.S. :math:`= \sqrt{\frac{1 + \cos A}{1 - \cos A}}`

    Multiplying and dividing with :math:`1 + \cos A,` we get

    :math:`= \sqrt{\frac{(1 + \cos A)^2}{1 - \cos^2A}} = \sqrt{\left(\frac{1 + \cos A}{\sin A}\right)^2} = \cosec A + \cot A =`
    R.H.S.

41. L.H.S. :math:`= \frac{\cos A}{1 + \sin A} + \frac{\cos A}{1 - \sin A}`

    :math:`\frac{\cos A(1 - \sin A) + \cos A(1 + \sin A)}{1 - \sin^2A}`

    :math:`= \frac{2\cos A}{\cos^2A} = 2\sec A =` R.H.S.

42. L.H.S. :math:`= \frac{\tan A}{\sec A - 1} + \frac{\tan A}{\sec A + 1}`

    :math:`= \frac{\tanA\sec A + \tan A + \tan A\sec A - \tan A}{(\sec^2A - 1)}`

    :math:`= \frac{2\tan A\sec A}{\tan^2 A} = 2\cosec A =` R.H.S.

43. L.H.S. :math:`= \frac{1}{1 - \sin A} - \frac{1}{1 + \sin A}`

    :math:`= \frac{1 + \sin A - 1 + \sin A}{1 - \sin^2A} = \frac{2\sin A}{\cos^2A} = 2\sec A\tan A =` R.H.S.

44. L.H.S. :math:`= \frac{1 + \tan^2 A}{1 + \cot^2 A} = \frac{1 + \frac{\sin^2A}{\cos^2A}}{1 + \frac{\cos^2A}{\sin^2A}}`

    :math:`= \frac{\frac{\sin^2A + \cos^2A}{\cos^2A}}{\frac{\sin^2A + \cos^2A}{\sin^2A}} = \frac{\sin^2A}{\cos^2A} = \tan^2A`

    R.H.S. :math:`= \left(\frac{1 - \tan A}{1 - \cot A}\right)^2 = \left(\frac{1 - \frac{\sin A}{\cos A}}{1 - \frac{\cos A}{\sin A}}\right)`

    :math:`= \left(\frac{\frac{\cos A - sin A}{\cos A}}{\frac{\sin A - \cos A}{\sin A}}\right)^2`

    :math:`= \frac{\sin^2A}{\cos^2A} = \tan^2A`

    Hence, L.H.S. = R.H.S.

45. L.H.S. :math:`= 1 + \frac{2\tan^2 A}{\cos^2 A} = 1 + \frac{2\sin^2A}{\cos^4A} = \frac{\cos^4A + 2\sin^2A}{\cos^4A}`

    :math:`= \frac{(1 - \sin^2A)^2 + 2\sin^2A}{\cos^4A} = \frac{1 - 2\sin^2A + \sin^4A + 2\sin^2A}{\cos^4A}`

    :math:`= \tan^4A + sec^4A =` R.H.S.

46. L.H.S. :math:`= (1 - \sin A - \cos A)^2 = 1 - 2\cos A - 2\sin A + 2\sin A\cos A + \sin^2A + \cos^2A`

    :math:`= 2 - 2\cos A - 2\sin A + 2\sin A\cos A = 2(1 - \cos A)(1 - \sin A) =` R.H.S.

47. L. H. S. :math:`= \frac{\cot A + \cosec A - 1}{\cot A - \cosec A + 1}`

    :math:`= \frac{\cos A + 1 - \sin A}{\cos A + \sin A - 1}`

    Multiplying and dividing with :math:`\cos A - (1 - \sin A),` we get

    :math:`= \frac{\cos^2A - 1 + 2\sin A - \sin^2A}{\cos^2A + \sin^2A + 1 - 2\cos A - 2\sin A + 2\sin A\cos A}`

    :math:`= \frac{2\sin A - 2\sin^2A}{2(1 - \cos A)(1 - \sin A)} = \frac{\sin A}{1 - \cos A}`

    Multiplyig numerator and denominator with :math:`1 + \cos A,` we get

    :math:`= \frac{\sin A(1 + \cos A)}{1 - \cos^2A} = \frac{1 + \cos A}{\sin A} =` R.H.S.

48. L.H.S. :math:`= (\sin A + \sec A)^2 + (\cos A + \cosec A)^2`

    :math:`= \left(\frac{\sin A\cos A + 1}{\cos A}\right)^2 + \left(\frac{\cos A\sin A + 1}{\sin A}\right)^2`

    :math:`= (1 + \sin A\cos A)^2 \left(\frac{1}{\cos^2A} + \frac{1}{\sin^2A}\right)`

    :math:`= (1 + \sin A\cos A)^2\left(\frac{\sin^2A + \cos^2A}{\sin^2A\cos^2A}\right)`

    :math:`= \left(\frac{1 + \sin A\cos A}{\sin A\cos A}\right)^2 = (1 + \sec A\cosec A)^2 =` R.H.S.

49. L.H.S. :math:`= \frac{2\sin A\tan A(1 - \tan A) + 2\sin A\sec^2A}{(1 + \tan A)^2}`

    :math:`= \frac{2\sin A(\tan A - \tan^2A + \sec^2A)}{(1 + \tan A)^2} = \frac{2\sin A(1 + \tan A)}{(1 + \tan A)^2}`

    :math:`= \frac{2\sin A}{1 + \tan A} =` R.H.S.

50. Given, :math:`2\sin A = 2 - \cos A`

    :math:`\cos A = 2 - 2\sin A,` squaring both sides we, get :math:`\cos^2A = 4 - 8\sin A + 4\sin^2A`

    :math:`1 - \sin^2A = 4 - 8\sin A + 4\sin^2A \Rightarrow 5\sin^2A - 8\sin A + 3 = 0`

    :math:`5\sin^2A - 5\sin A - 3\sin A + 3 = 0 \Rightarrow \sin A = 1, \frac{3}{5}`

51. Given :math:`8\sin A = 4 + \cos A \Rightarrow 8\sin A - 4 = \cos A`

    Squaring both sides, we get

    :math:`64\sin^2A - 64\sin A + 16 = \cos^2A = 1 - \sin^2A`

    :math:`65\sin^2A - 64\sin A + 15 = 0`

    :math:`65\sin^2A - 39\sin A - 25\sin A + 15 = 0`

    :math:`\sin A = \frac{3}{5}, \frac{5}{13}`

52. Given, :math:`\tan A + \sec A = 1.5`

    :math:`\Rightarrow 1 + \sin A = 1.5 \cos A \Rightarrow 2 + 2\sin A = 3\cos A`

    Squaring both sides, we get

    :math:`4 + 8\sin A + 4\sin^2A = 9 - 9\sin^2A`

    :math:`13\sin^2A + 8\sin A - 5 =0`

    :math:`\sin A = -1, \frac{5}{13}`

53. Given, :math:`\cot A + \cosec A = 5 \Rightarrow 1 + \cos A = 5\sin A`

    Squarig both sides, we get

    :math:`1 + 2\cos A + \cos^2A = 25\sin^2A = 25(1 - \cos^2A)`

    :math:`26\cos^2A + 2\cos A - 24 = 0`

    :math:`26\cos^2A + 26\cos A - 24\cos A - 24 = 0`

    :math:`\cos A= -1, \frac{12}{13}`

54. :math:`3\sec^4 A + 8 = 10\sec^2A \Rightarrow 3(sec^2A)^2 + 8 = 10(1 + \tan^2A)`

    :math:`\Rightarrow 3(1 + \tan^2A)^2 + 8 = 10 + 10\tan^2A`

    :math:`3 + 6\tan^2A + 3\tan^4A + 8 = 10 + 10\tan^2A`

    :math:`3\tan^4A - 4\tan^2A + 1 = 0`

    :math:`\tan A = \pm1, \pm\frac{1}{\sqrt{3}}`

55. Given, :math:`\tan^2A + \sec A = 5 \Rightarrow \sec^2A - 1 + \sec A = 5`

    :math:`\sec^2A + \secA - 6 = 0`

    :math:`\sec A = -3, 2\Rightarrow \cos A = -\frac{1}{3}, \frac{1}{2}`

56. Given :math:`\tan A + \cot A = 2 \Rightarrow \tan A + \frac{1}{\tan A} = 2`

    :math:`\tan^2A - 2\tan A + 1 = 0`

    :math:`\tan A = 1 \Rightarrow \sin A = \frac{1}{\sqrt{2}}`

57. Given, :math:`\sec^2A = 2 + 2\tan A \Rightarrow \tan^2A + 1 = 2 + 2\tan A`

    :math:`\tan^2A - 2\tanA - 1 = 0`

    :math:`tan A = \frac{2 \pm \sqrt{4 + 4}}{2} = 1 \pm \sqrt{2}`

58.
