Trigonometrical Identities
**************************
In this chapter we will have only problems and we will use the theory we have learned till now.

1. If :math:`A + B + C = \pi,` prove that :math:`\sin^2A + \sin^2B - \sin^2C = 2\sin A\sin B\sin C`

2. If :math:`A + B + C = 180^\circ,` prove that :math:`\sin^2\frac{A}{2} + \sin^2\frac{B}{2} + \sin^2\frac{C}{2} = 1 - 2\sin
   \frac{A}{2}\sin \frac{B}{2}\sin \frac{C}{2}`

3. Show that :math:`\sin^2A + \sin^2B + 2\sin A\sin B\cos(A + B) = \sin^2(A + B)`

4. If :math:`A + B + C = 180^\circ,` prove that :math:`\cos^2A + \cos^2B + \cos^2C + 2\cos A\cos B\cos C = 1`

5. If :math:`A + B + C = 180^\circ,` prove that :math:`\sin^2A + \sin^2B + \sin^2C = 2(1 + \cos A \cos B \cos C)`

6. If :math:`A + B + C = 180^\circ,` prove that :math:`\cos^2A + \cos^2B - \cos^2C = 1 - 2\sin A\sin B\sin C`

7. If :math:`A + B + C = 180^\circ,` prove that :math:`\cos^2\frac{A}{2} + \cos^2\frac{B}{2} - \cos^2\frac{C}{2} =
   2\cos\frac{A}{2}\cos\frac{B}{2}\sin\frac{C}{2}`

8. If :math:`A + B + C = 180^\circ,` prove that :math:`\cos^2\frac{A}{2} + \cos^2\frac{B}{2} + \cos^2\frac{C}{2} = 2 +
   2\sin\frac{A}{2}\sin\frac{B}{2}\sin\frac{C}{2}`

9. If :math:`A + B + C = \frac{\pi}{2},` prove that :math:`\sin^2A + \sin^2B + \sin^2C = 1 - 2\sin A\sin B\sin C`

10. If :math:`A + B + C = \frac{\pi}{2},` prove that :math:`\cos^2A + \cos^2B + \cos^2C = 2 + 2\sin A\sin B\sin C`

11. If :math:`A + B + C = 2\pi,` prove that :math:`\cos^2A + \cos^2B + \cos^2C - 2\cos A\cos B\cos C = 1`

12. If :math:`A + B = C,` prove that :math:`\cos^2A + \cos^2B + \cos^2C - 2\cos A\cos B\cos C = 1`

13. If :math:`A + B = \frac{\pi}{3},` prove that :math:`\cos^2A + \cos^2B - \cos A\cos B = \frac{3}{4}`

14. Show that :math:`\cos^2B + \cos^2(A + B) - 2\cos A\cos B\cos(A + B)` is independent of :math:`B.`

15. If :math:`A + B + C = \pi` and :math:`A + B = 2C,` prove that :math:`4(\sin^2A + \sin^2B - \sin A\sin B) = 3`

16. If :math:`A + B + C = 2\pi,` prove that :math:`\cos^2B + \cos^2C - \sin^2A - 2\cos A\cos B\cos C = 0`

17. If :math:`A + B + C = 0,` prove that :math:`\cos^2A + \cos^2B + \cos^2C = 1 + 2\cos A\cos B\cos C`

18. Prove that :math:`\cos^2(B - C) + \cos^2(C - A) + \cos^2(A - B) = 1 + 2\cos(B - C)\cos(C - A)\cos(A - B)`

19. If :math:`A + B + C = \pi,` prove that :math:`\sin A\cos B\cos C + \sin B\cos C\cos A + \sin C\cos A\cos B= \sin A\sin B\sin C`

20. If :math:`A + B + C = \pi,` prove that :math:`\tan A + \tan B + \tan C = \tan A\tan B\tan C`

21. If :math:`A + B + C = \pi,` prove that :math:`\tan\frac{A}{2}\tan\frac{B}{2} + \tan\frac{B}{2}\tan\frac{C}{2} +
    \tan\frac{C}{2}\tan\frac{A}{2} = 1`

22. If :math:`A + B + C = \pi,` prove that :math:`\tan(B + C - A) + \tan(C + A - B) + \tan(A + B - C) = \tan(B + C - A)\tan(C + A -
    B)\tan(A + B - C)`

23. If :math:`A + B + C = \pi,` prove that :math:`\cot B\cot C + \cot C\cot A + \cot A\cot B = 1`

24. In a :math:`\triangle ABC,` if :math:`\cot A + \cot B + \cot C = \sqrt{3},` prove that the triangle is equilateral.

25. If :math:`A, B, C, D` are angles of a quadrilateral, prove that :math:`\frac{\tan A + \tan B + \tan C + \tan D}{\cot A + \cot B
    + \cot C + \cot D} = \tan A\tan B\tan C\tan D`

26. If :math:`A + B + C = \frac{\pi}{2},` show that :math:`\cot A + \cot B + \cot C = \cot A\cot B\cot C`

27. If :math:`A + B + C = \frac{\pi}{2},` show that :math:`\tan A\tan B + \tan B\tan C + \tan C\tan A = 1`

28. If :math:`A + B + C = \pi,` prove that :math:`\tan 3A + \tan 3B + \tan 3C = \tan 3A\tan 3B\tan 3C`

29. If :math:`A + B + C = \pi,` prove that :math:`\cot \frac{A}{2} + \cot \frac{B}{2} + \cot \frac{C}{2} = \cot \frac{A}{2}\cot
    \frac{B}{2}\cot \frac{C}{2}`

30. If :math:`A + B + C = \pi,` prove that :math:`\frac{\cot A + \cot B}{\tan A + \tan B} + \frac{\cot B + \cot C}{\tan B + \tan C}
    + \frac{\cot C + \cot A}{\tan C + \tan A} = 1`

31. Prove that :math:`\tan(A - B) + \tan(B - C) + \tan(C - A) = \tan(A - B)\tan(B - C)\tan(C - A)`

32. If :math:`x + y + z = 0,` show that :math:`\cot(x + y - z)\cot(z + x - y) + \cot(x + y - z)\cot(y + z - x) + \cot(y + z -
    x)\cot(z + x - y) = 1`

33. If :math:`A + B + C = n\pi(n` being zero or an integer :math:`),` show that :math:`\tan A + \tan B + \tan C = \tan A\tan B\tan
    C`

34. If :math:`A + B + C = \pi,` prove that :math:`\sin 2A + \sin 2B + \sin 2C = 4\sin A\sin B\sin C`

35. If :math:`A + B + C = \pi,` prove that :math:`\cos A + \cos B + \cos C - 1 = 4\sin \frac{A}{2}\sin \frac{B}{2}\sin \frac{C}{2}`

36. Prove that :math:`\frac{\sin 2A + \sin 2B + \sin 2C}{\cos A + \cos B + \cos C - 1} =
    8\cos\frac{A}{2}\cos\frac{B}{2}\cos\frac{C}{2}`

37. If :math:`A + B + C = \pi,` prove that :math:`\cos\frac{A}{2} + \cos\frac{B}{2} + \cos\frac{C}{2} = 4\cos\frac{\pi -
    A}{4}\cos\frac{\pi - B}{4}\cos\frac{\pi - C}{4}`

38. If :math:`A + B + C = \pi,` prove that :math:`\sin \frac{A}{2} + \sin \frac{B}{2} + \sin \frac{C}{2} = 1 + 4\sin \frac{B +
    C}{4}\sin \frac{C + A}{4}\sin \frac{A + B}{4}`

39. If :math:`A + B + C = \pi,` prove that :math:`\sin^2\frac{A}{2} + \sin^2\frac{B}{2} - \sin^2\frac{C}{2} = 1 - 2\cos
    \frac{A}{2}\cos \frac{B}{2}\cos \frac{C}{2}`

40. Prove that :math:`1 + \cos 56^\circ + \cos 58^\circ - \cos 66^\circ = 4\cos28^\circ\cos29^\circ\sin 33^\circ`

41. If :math:`A + B + C = \pi,` prove that :math:`\cos 2A + \cos 2B - \cos 2C = 1 - 4\sin A\sin B\cos C`

42. If :math:`A + B + C = \pi,` prove that :math:`\sin 2A + \sin 2B - \sin 2C = 4\cos A\cos B\sin C`

43. If :math:`A + B + C = \pi,` prove that :math:`\sin A + \sin B + \sin C = 4\cos \frac{A}{2}\cos \frac{B}{2}\cos \frac{C}{2}`

44. If :math:`A + B + C = \pi,` prove that :math:`\cos A + \cos B - \cos C = 4\cos \frac{A}{2}\cos \frac{B}{2}\sin \frac{C}{2} - 1`

45. If :math:`A + B + C = \pi,` prove that :math:`\sin(B + C - A) + \sin(C + A - B) + \sin(A + B - C) = 4\sin A\sin B\sin C`

46. If :math:`A + B + C = \pi,` prove that :math:`\frac{\cos A}{\sin B\sin C} + \frac{\cos B}{\sin C\sin A} + \frac{\cos C}{\sin
    A\sin B} = 2`

47. If :math:`A + B + C = \pi,` prove that :math:`\frac{\sin 2A + \sin 2B + \sin 2C}{\sin A + \sin B + \sin C} = 8\sin \frac{A}{2}\
    \sin \frac{B}{2}\sin \frac{C}{2}`

48. If :math:`x + y + z = \frac{\pi}{2},` prove that :math:`\cos(x - y - z) + \cos(y - z - x) + \cos(z - x - y) - 4\cos x\cos y\cos
    z = 0`

49. Show that :math:`\sin(x - y) + \sin(y - z) + \sin(z - x) + 4\sin\frac{x - y}{2}\sin\frac{y - z}{2}\sin \frac{z - x}{2} = 0`

50. If :math:`A + B + C = 180^\circ,` prove that :math:`\sin(B + 2C) + \sin(C + 2A) + \sin(A + 2B) = 4\sin\frac{B - C}{2}
    \sin\frac{C - A}{2}\sin\frac{A - B}{2}`

51. If :math:`A + B + C = \pi,` prove that :math:`\sin\frac{B + C}{2} + \sin \frac{C + A}{2} + \sin \frac{A + B}{2} =
    4\cos\frac{\pi - A}{4}\cos\frac{\pi - B}{4}\cos\frac{\pi - C}{4}`

52. If :math:`xy + yz + zx = 1,` prove that :math:`\frac{x}{1 - x^2} + \frac{y}{1 - y^2} + \frac{z}{1 - z^2} = \frac{4xyz}{(1 -
    x^2)(1 - y^2)(1 - z^2)}`

53. If :math:`x + y + z = xyz,` show that :math:`\frac{3x - x^3}{1 - 3x^2} + \frac{3y - y^3}{1 - 3y^2} + \frac{3z - z^3}{1 - 3z^2}
    = \frac{3x - x^3}{1 - 3x^2}.\frac{3y - y^3}{1 - 3y^2}.\frac{3z - z^3}{1 - 3z^2}`

54. If :math:`x + y + z = xyz,` prove that :math:`\frac{2x}{1 - x^2} + \frac{2y}{1 - y^2} + \frac{2z}{1 - z^2} = \frac{2x}{1 -
    x^2}.\frac{2y}{1 - y^2}.\frac{2z}{1 - z^2}`

55. If :math:`x + y + z = xyz,` prove that :math:`x(1 - y^2)(1 - z^2) + y(1 - z^2)(1 - x^2) + z(1 - x^2)(1 - y^2) = 4xyz`

56. If :math:`A + B + C + D = 2\pi,` prove that :math:`\cos A + \cos B + \cos C + \cos D = 4\cos\frac{A + B}{2}\cos\frac{B +
    C}{2}\cos\frac{C + A}{2}`

57. If :math:`A + B + C = 2S,` prove that :math:`\cos^2S + \cos^2(S - A) + \cos^2(S - B) + \cos^2(S - C) = 2 + 2\cos A\cos B\cos C`

58. If :math:`A + B + C = \pi,` prove that :math:`\tan^2\frac{A}{2} + \tan^2\frac{B}{2} + \tan^2\frac{C}{2}\geq 1`

59. If :math:`A + B + C = \pi,` prove that :math:`(\tan A + \tan B + \tan C)(\cot A + \cot B + \cot C) = 1 + \sec A\sec B\sec C`

60. If :math:`A + B + C = \pi,` prove that :math:`(\cot B + \cot C)(\cot C + \cot A)(\cot A + \cot C) = \cosec A\cosec B\cosec C`

61. If :math:`A + B + C = \pi,` prove that :math:`\frac{1}{2}\sum \sin^2A(\sin 2B + \sin 2C) = 3\sin A\sin B\sin C`

62. If :math:`A + B + C + D = 2\pi,` prove that :math:`\cos A - \cos B + \cos C - \cos D = 4\sin\frac{A + B}{2}\sin\frac{A +
    D}{2}\cos \frac{A + C}{2}`

63. If :math:`A, B, C, D` be the angles of a cyclic quadrilateral, prove that :math:`\cos A + \cos B + \cos C + \cos D = 0`

64. If :math:`A + B + C = \pi,` prove that :math:`\cot^2A + \cot^2B + \cot^2C \geq 1`

65. If :math:`A + B + C = \pi,` prove that :math:`\cos \frac{A}{2}\cos\frac{B - C}{2} + \cos\frac{B}{2}\cos\frac{C - A}{2} + \cos
    \frac{C}{2}\cos\frac{A -B}{2} = \sin A + \sin B + \sin C`

66. In a :math:`\triangle ABC,` prove that :math:`\sin 3A\sin(B - C) + \sin 3B\sin(C - A) + \sin3C\sin(A - B) = 0`
