Trigonometrical Equations and their General Solutions
*****************************************************

Trigonometrical Equation
========================
An equation involving one or more trigonometrical ratios of unknown angle is called trigonometrical equation.

Ex. :math:`\cos^2x - 4\sin x = 1`

A trigonometrical identity is satisfied for every value of the unknown angle whereas trigonometrical equation is satisfied for
only some values of unknown angle. For example, :math:`1 - \cos^2x = \sin^2x` is a trigonometrical identity because it is satisfied
for every value of :math:`x.`

Solution of a Trigonometrical Equation
======================================
A value of the unknown angle which satisfies the given trigonometrical equation is called a solution or root of the equation.

For example, :math:`2\sin\theta = 1 \Rightarrow \theta = 30^\circ, 150^\circ` which are two solutions between :math:`0` and
:math:`2\pi.`

General Solution
================
Some trigonometrical functions are periodic functions, therefore, solutions of trigonometrical equations can be generalized with
the help of periodicirty of trigonometrical functions. The solution consisting of all possible solutions of a trigonometrical
equation is called its general solution.

For example, :math:`\sin\theta = 0` has a genral solution which is :math:`n\pi` where :math:`n\in I.`

Similarly, fo :math:`\cos\theta = 0,` the general solution is :math:`(2n + 1)\frac{\pi}{2},` where :math:`n\in I` and for
:math:`\tan\theta = 0` the solution is again :math:`n\pi.`

General Solution of :math:`\sin\theta = \sin\alpha`
---------------------------------------------------
Given, :math:`\sin\theta = \sin\alpha \Rightarrow \sin\theta - \sin\alpha = 0`

:math:`\Rightarrow 2\cos\frac{\theta + \alpha}{2}\sin\frac{\theta - \alpha}{2} = 0`

**Case I** :math:`\cos\frac{\theta + \alpha}{2} = 0`

:math:`\Rightarrow \theta + \alpha = (2m + 1)\pi, m\in I`

**Case II** :math:`\sin\frac{\theta - \alpha}{2} = 0`

:math:`\Rightarrow \theta - \alpha = 2m\pi \Rightarrow \theta = 2m\pi + \alpha`

Thus, :math:`\theta = n\pi + (-1)^n\alpha, n\in I`

General Solution of :math:`\cos\theta = \cos\alpha`
---------------------------------------------------
Given, :math:`\cos\theta = \cos\alpha \Rightarrow \cos\theta - \cos\alpha = 0`


:math:`\Rightarrow 2\sin\frac{\alpha + \theta}{2}\sin\frac{\theta - \alpha}{2} = 0`

**Case I:** :math:`\sin\frac{\alpha + \theta}{2} = 0`
